renaming to HolBA and HolBIR

bir_immScript.sml
@@ -1,23 +1,15 @@
-(* ========================================================================= *)
-(* FILE          : bil_immScript.sml                                             *)
-(* DESCRIPTION   : A model of immediates from BAP Intermediate Language.     *)
-(* AUTHOR        : (c) Thomas Tuerk <tuerk@kth.se> based on previous work    *)
-(*                 by Roberto Metere, KTH - Royal Institute of Technology    *)
-(* DATE          : 2017                                                      *)
-(* ========================================================================= *)
-
 open HolKernel Parse boolLib bossLib;
 open wordsTheory bitstringTheory;
-open bil_auxiliaryTheory;
+open bir_auxiliaryTheory;
 
-val _ = new_theory "bil_imm";
+val _ = new_theory "bir_imm";
 
 (* ------------------------------------------------------------------------- *)
 (*  Immediates                                                               *)
 (* ------------------------------------------------------------------------- *)
 
-(* Bil immediates can be words of various sizes *)
-val _ = Datatype `bil_imm_t =
+(* Immediates can be words of various sizes *)
+val _ = Datatype `bir_imm_t =
     Imm1  bool[1]
   | Imm8  bool[8]
   | Imm16 bool[16]
@@ -27,7 +19,7 @@ val _ = Datatype `bil_imm_t =
 
 
 (* It is handy to keep track of the size via both a special datatype and a number *)
-val _ = Datatype `bil_immtype_t =
+val _ = Datatype `bir_immtype_t =
   | Bit1
   | Bit8
   | Bit16
@@ -35,24 +27,24 @@ val _ = Datatype `bil_immtype_t =
   | Bit64
 `;
 
-val bil_imm_ss = rewrites ((type_rws ``:bil_imm_t``) @ (type_rws ``:bil_immtype_t``));
+val bir_imm_ss = rewrites ((type_rws ``:bir_imm_t``) @ (type_rws ``:bir_immtype_t``));
 
-val type_of_bil_imm_def = Define `
-  (type_of_bil_imm (Imm1  _) = Bit1) /\
-  (type_of_bil_imm (Imm8  _) = Bit8) /\
-  (type_of_bil_imm (Imm16 _) = Bit16) /\
-  (type_of_bil_imm (Imm32 _) = Bit32) /\
-  (type_of_bil_imm (Imm64 _) = Bit64)`;
+val type_of_bir_imm_def = Define `
+  (type_of_bir_imm (Imm1  _) = Bit1) /\
+  (type_of_bir_imm (Imm8  _) = Bit8) /\
+  (type_of_bir_imm (Imm16 _) = Bit16) /\
+  (type_of_bir_imm (Imm32 _) = Bit32) /\
+  (type_of_bir_imm (Imm64 _) = Bit64)`;
 
-val size_of_bil_immtype_def = Define `
-  (size_of_bil_immtype Bit1  = 1) /\
-  (size_of_bil_immtype Bit8  = 8) /\
-  (size_of_bil_immtype Bit16 = 16) /\
-  (size_of_bil_immtype Bit32 = 32) /\
-  (size_of_bil_immtype Bit64 = 64)`
+val size_of_bir_immtype_def = Define `
+  (size_of_bir_immtype Bit1  = 1) /\
+  (size_of_bir_immtype Bit8  = 8) /\
+  (size_of_bir_immtype Bit16 = 16) /\
+  (size_of_bir_immtype Bit32 = 32) /\
+  (size_of_bir_immtype Bit64 = 64)`
 
-val bil_immtype_of_size_def = Define `
-  bil_immtype_of_size n = (
+val bir_immtype_of_size_def = Define `
+  bir_immtype_of_size n = (
          if n = 1  then SOME Bit1
     else if n = 8  then SOME Bit8
     else if n = 16 then SOME Bit16
@@ -60,38 +52,38 @@ val bil_immtype_of_size_def = Define `
     else if n = 64 then SOME Bit64
     else NONE)`;
 
-val is_valid_bil_immtype_size_def = Define `
-  is_valid_bil_immtype_size n = ?b. n = size_of_bil_immtype b`;
+val is_valid_bir_immtype_size_def = Define `
+  is_valid_bir_immtype_size n = ?b. n = size_of_bir_immtype b`;
 
 (* A few sanity checks *)
-val size_of_bil_immtype_INJ = store_thm ("size_of_bil_immtype_INJ",
-  ``!b1 b2. (size_of_bil_immtype b1 = size_of_bil_immtype b2) <=> (b1 = b2)``,
-Cases >> Cases >> SIMP_TAC (std_ss++bil_imm_ss) [size_of_bil_immtype_def]);
+val size_of_bir_immtype_INJ = store_thm ("size_of_bir_immtype_INJ",
+  ``!b1 b2. (size_of_bir_immtype b1 = size_of_bir_immtype b2) <=> (b1 = b2)``,
+Cases >> Cases >> SIMP_TAC (std_ss++bir_imm_ss) [size_of_bir_immtype_def]);
 
-val size_of_bil_immtype_NEQ_0 = store_thm ("size_of_bil_immtype_NEQ_0",
-  ``!b. size_of_bil_immtype b <> 0``,
-Cases >> SIMP_TAC arith_ss [size_of_bil_immtype_def])
+val size_of_bir_immtype_NEQ_0 = store_thm ("size_of_bir_immtype_NEQ_0",
+  ``!b. size_of_bir_immtype b <> 0``,
+Cases >> SIMP_TAC arith_ss [size_of_bir_immtype_def])
 
-val is_valid_bil_immtype_size_REWRS = save_thm ("is_valid_bil_immtype_size_REWRS",
-  SIMP_RULE (std_ss++DatatypeSimps.expand_type_quants_ss [``:bil_immtype_t``]) [size_of_bil_immtype_def] is_valid_bil_immtype_size_def);
+val is_valid_bir_immtype_size_REWRS = save_thm ("is_valid_bir_immtype_size_REWRS",
+  SIMP_RULE (std_ss++DatatypeSimps.expand_type_quants_ss [``:bir_immtype_t``]) [size_of_bir_immtype_def] is_valid_bir_immtype_size_def);
 
-val is_valid_bil_immtype_size_IMP = save_thm ("is_valid_bil_immtype_size_IMP",
-  snd (EQ_IMP_RULE (SPEC_ALL is_valid_bil_immtype_size_REWRS)));
+val is_valid_bir_immtype_size_IMP = save_thm ("is_valid_bir_immtype_size_IMP",
+  snd (EQ_IMP_RULE (SPEC_ALL is_valid_bir_immtype_size_REWRS)));
 
-val is_valid_bil_immtype_size_IS_SOME = store_thm ("is_valid_bil_immtype_size_IS_SOME",
-  ``!n. is_valid_bil_immtype_size n <=> IS_SOME (bil_immtype_of_size n)``,
-SIMP_TAC std_ss [is_valid_bil_immtype_size_REWRS, bil_immtype_of_size_def] >>
+val is_valid_bir_immtype_size_IS_SOME = store_thm ("is_valid_bir_immtype_size_IS_SOME",
+  ``!n. is_valid_bir_immtype_size n <=> IS_SOME (bir_immtype_of_size n)``,
+SIMP_TAC std_ss [is_valid_bir_immtype_size_REWRS, bir_immtype_of_size_def] >>
 METIS_TAC[optionTheory.IS_SOME_DEF]);
 
-val bil_immtype_of_num_inv = store_thm ("bil_immtype_of_num_inv",
-  ``(!brt. bil_immtype_of_size (size_of_bil_immtype brt) = SOME brt) /\
-    (!n brt. (bil_immtype_of_size n = SOME brt) ==>
-             (size_of_bil_immtype brt = n))``,
+val bir_immtype_of_num_inv = store_thm ("bir_immtype_of_num_inv",
+  ``(!brt. bir_immtype_of_size (size_of_bir_immtype brt) = SOME brt) /\
+    (!n brt. (bir_immtype_of_size n = SOME brt) ==>
+             (size_of_bir_immtype brt = n))``,
 REPEAT CONJ_TAC >| [
-  Cases >> SIMP_TAC std_ss [size_of_bil_immtype_def, bil_immtype_of_size_def],
+  Cases >> SIMP_TAC std_ss [size_of_bir_immtype_def, bir_immtype_of_size_def],
 
-  SIMP_TAC (std_ss++boolSimps.LIFT_COND_ss) [bil_immtype_of_size_def, DISJ_IMP_THM, FORALL_AND_THM,
-    COND_EXPAND_OR, LEFT_AND_OVER_OR, size_of_bil_immtype_def]
+  SIMP_TAC (std_ss++boolSimps.LIFT_COND_ss) [bir_immtype_of_size_def, DISJ_IMP_THM, FORALL_AND_THM,
+    COND_EXPAND_OR, LEFT_AND_OVER_OR, size_of_bir_immtype_def]
 ]);
 
 
@@ -130,10 +122,10 @@ val n2b_fixed_DEFS = save_thm ("n2b_fixed_DEFS",
     LIST_CONJ [n2b_1_def, n2b_8_def, n2b_16_def, n2b_32_def, n2b_64_def]);
 
 val b2n_n2bs = store_thm ("b2n_n2bs",
-  ``!bt n. b2n (n2bs n bt) = MOD_2EXP (size_of_bil_immtype bt) n``,
+  ``!bt n. b2n (n2bs n bt) = MOD_2EXP (size_of_bir_immtype bt) n``,
 Cases >> (
   SIMP_TAC (std_ss++wordsLib.WORD_ss) [b2n_def, n2bs_def, w2n_n2w,
-    size_of_bil_immtype_def, bitTheory.MOD_2EXP_def]
+    size_of_bir_immtype_def, bitTheory.MOD_2EXP_def]
 ));
 
 val b2n_n2b_fixed = store_thm ("b2n_n2b_fixed",
@@ -142,15 +134,15 @@ val b2n_n2b_fixed = store_thm ("b2n_n2b_fixed",
     (!n. b2n (n2b_16 n) = n MOD 2**16) /\
     (!n. b2n (n2b_32 n) = n MOD 2**32) /\
     (!n. b2n (n2b_64 n) = n MOD 2**64) /\
-    (!n bt. b2n (n2bs n bt) = n MOD 2**(size_of_bil_immtype bt))``,
+    (!n bt. b2n (n2bs n bt) = n MOD 2**(size_of_bir_immtype bt))``,
 
-SIMP_TAC std_ss [n2b_fixed_DEFS, b2n_n2bs, size_of_bil_immtype_def,
+SIMP_TAC std_ss [n2b_fixed_DEFS, b2n_n2bs, size_of_bir_immtype_def,
   bitTheory.MOD_2EXP_def]);
 
 val n2bs_b2n = store_thm ("n2bs_b2n",
-  ``!b s. (s = type_of_bil_imm b) ==> (n2bs (b2n b) s = b)``,
+  ``!b s. (s = type_of_bir_imm b) ==> (n2bs (b2n b) s = b)``,
 Cases >> (
-  SIMP_TAC std_ss [b2n_def, n2bs_def, type_of_bil_imm_def, n2w_w2n]
+  SIMP_TAC std_ss [b2n_def, n2bs_def, type_of_bir_imm_def, n2w_w2n]
 ));
 
 
@@ -158,37 +150,37 @@ val w2n_lt_trans = prove (``!w:'a word. dimword (:'a) <= m ==> (w2n w < m)``,
 METIS_TAC[w2n_lt, arithmeticTheory.LESS_LESS_EQ_TRANS]);
 
 val b2n_lt = store_thm ("b2n_lt",
-  ``!b. b2n b < 2 ** (size_of_bil_immtype (type_of_bil_imm b))``,
+  ``!b. b2n b < 2 ** (size_of_bir_immtype (type_of_bir_imm b))``,
 Cases >> (
-  SIMP_TAC std_ss [b2n_def, type_of_bil_imm_def, size_of_bil_immtype_def] >>
+  SIMP_TAC std_ss [b2n_def, type_of_bir_imm_def, size_of_bir_immtype_def] >>
   MATCH_MP_TAC w2n_lt_trans >>
   SIMP_TAC (std_ss++wordsLib.SIZES_ss) []
 ));
 
 
 val b2n_lt_REWRS = save_thm ("b2n_lt_REWRS",
-SIMP_RULE (std_ss++DatatypeSimps.expand_type_quants_ss[``:bil_imm_t``]) [
-  type_of_bil_imm_def, size_of_bil_immtype_def] b2n_lt);
+SIMP_RULE (std_ss++DatatypeSimps.expand_type_quants_ss[``:bir_imm_t``]) [
+  type_of_bir_imm_def, size_of_bir_immtype_def] b2n_lt);
 
 
 val b2n_MOD_2EXP = store_thm ("b2n_MOD_2EXP",
-  ``!i n. ((size_of_bil_immtype (type_of_bil_imm i)) = n) ==>
+  ``!i n. ((size_of_bir_immtype (type_of_bir_imm i)) = n) ==>
           (MOD_2EXP n (b2n i) = b2n i)``,
 SIMP_TAC std_ss [bitTheory.MOD_2EXP_def, b2n_lt]);
 
 
 val type_of_n2bs = store_thm ("type_of_n2bs",
-``!s n. type_of_bil_imm (n2bs n s) = s``,
-Cases >> SIMP_TAC std_ss [n2bs_def, type_of_bil_imm_def]);
+``!s n. type_of_bir_imm (n2bs n s) = s``,
+Cases >> SIMP_TAC std_ss [n2bs_def, type_of_bir_imm_def]);
 
 
 val type_of_n2b_fixed = save_thm ("type_of_n2b_fixed",
-SIMP_RULE (std_ss++DatatypeSimps.expand_type_quants_ss [``:bil_immtype_t``]) [
+SIMP_RULE (std_ss++DatatypeSimps.expand_type_quants_ss [``:bir_immtype_t``]) [
   GSYM n2b_fixed_DEFS] type_of_n2bs);
 
 
-val type_of_bil_imm_n2bs_INTRO = store_thm ("type_of_bil_imm_n2bs_INTRO",
-  ``!s b. (type_of_bil_imm b = s) <=> (?n. b = n2bs n s)``,
+val type_of_bir_imm_n2bs_INTRO = store_thm ("type_of_bir_imm_n2bs_INTRO",
+  ``!s b. (type_of_bir_imm b = s) <=> (?n. b = n2bs n s)``,
 
 REPEAT GEN_TAC >> EQ_TAC >> STRIP_TAC >| [
   Q.EXISTS_TAC `b2n b` >>
@@ -225,7 +217,7 @@ SIMP_TAC std_ss [w2bs_def,n2bs_def, w2w_def]);
 
 
 val w2bs_b2w = store_thm ("w2bs_b2w",
-  ``!b s. ((s = type_of_bil_imm b) /\ size_of_bil_immtype (type_of_bil_imm b) <= dimindex (:'a)) ==>
+  ``!b s. ((s = type_of_bir_imm b) /\ size_of_bir_immtype (type_of_bir_imm b) <= dimindex (:'a)) ==>
           (w2bs ((b2w b):'a word) s = b)``,
 SIMP_TAC std_ss [w2bs_def, b2w_def, w2n_n2w] >>
 REPEAT STRIP_TAC >>
@@ -233,14 +225,14 @@ REPEAT STRIP_TAC >>
   MATCH_MP_TAC arithmeticTheory.LESS_MOD >>
   ASSUME_TAC (Q.SPEC `b` b2n_lt) >>
   FULL_SIMP_TAC arith_ss [dimword_def] >>
-  `2 ** size_of_bil_immtype (type_of_bil_imm b) <= 2 ** dimindex (:'a)` by
+  `2 ** size_of_bir_immtype (type_of_bir_imm b) <= 2 ** dimindex (:'a)` by
      METIS_TAC[bitTheory.TWOEXP_MONO2] >>
   DECIDE_TAC
 ) >>
 ASM_SIMP_TAC std_ss [n2bs_b2n])
 
 val type_of_w2bs = store_thm ("type_of_w2bs",
-``!s w. type_of_bil_imm (w2bs w s) = s``,
+``!s w. type_of_bir_imm (w2bs w s) = s``,
 SIMP_TAC std_ss [w2bs_def, type_of_n2bs]);
 
 
@@ -251,7 +243,7 @@ SIMP_TAC std_ss [w2bs_def, type_of_n2bs]);
 val b2bool_def = Define `b2bool bi = (b2n bi <> 0)`;
 
 val b2bool_REWRS = save_thm ("b2bool_REWRS",
-  SIMP_RULE (std_ss++DatatypeSimps.expand_type_quants_ss[``:bil_imm_t``]) [
+  SIMP_RULE (std_ss++DatatypeSimps.expand_type_quants_ss[``:bir_imm_t``]) [
     b2n_def, w2n_eq_0]
     b2bool_def);
 
@@ -270,8 +262,8 @@ FULL_SIMP_TAC (std_ss++wordsLib.WORD_ss) [] >>
 ));
 
 val type_of_bool2b = store_thm ("type_of_bool2b",
-  ``!b. type_of_bil_imm (bool2b b) = Bit1``,
-Cases >> SIMP_TAC std_ss [bool2b_def, type_of_bil_imm_def]);
+  ``!b. type_of_bir_imm (bool2b b) = Bit1``,
+Cases >> SIMP_TAC std_ss [bool2b_def, type_of_bir_imm_def]);
 
 
 (* ------------------------------------------------------------------------- *)
@@ -281,7 +273,7 @@ Cases >> SIMP_TAC std_ss [bool2b_def, type_of_bil_imm_def]);
 val v2bs_def = Define `v2bs v s = n2bs (v2n v) s`;
 
 val v2bs_REWRS = save_thm ("v2bs_REWRS",
-  SIMP_RULE (std_ss++DatatypeSimps.expand_type_quants_ss[``:bil_immtype_t``]) [
+  SIMP_RULE (std_ss++DatatypeSimps.expand_type_quants_ss[``:bir_immtype_t``]) [
     n2bs_def, FORALL_AND_THM, n2w_v2n] v2bs_def);
 
 val b2v_def = Define `
@@ -293,11 +285,11 @@ val b2v_def = Define `
 `;
 
 val b2v_LENGTH = store_thm ("b2v_LENGTH",
-  ``!r. LENGTH (b2v r) = size_of_bil_immtype (
-        type_of_bil_imm r)``,
+  ``!r. LENGTH (b2v r) = size_of_bir_immtype (
+        type_of_bir_imm r)``,
 Cases >> (
-  SIMP_TAC (std_ss++wordsLib.WORD_ss) [b2v_def, type_of_bil_imm_def,
-    size_of_bil_immtype_def, length_w2v]
+  SIMP_TAC (std_ss++wordsLib.WORD_ss) [b2v_def, type_of_bir_imm_def,
+    size_of_bir_immtype_def, length_w2v]
 ));
 
 val v2n_w2v = store_thm ("v2n_w2v",
@@ -316,7 +308,7 @@ Cases >> (
 
 
 val type_of_v2bs = store_thm ("type_of_v2bs",
-``!s v. type_of_bil_imm (v2bs v s) = s``,
+``!s v. type_of_bir_imm (v2bs v s) = s``,
 SIMP_TAC std_ss [v2bs_def, type_of_n2bs]);
 
 
@@ -331,12 +323,12 @@ METIS_TAC[v2w_fixwidth]);
 
 
 val v2bs_fixwidth = store_thm ("v2bs_fixwidth",
-``!v vty w. (size_of_bil_immtype vty <= w) ==>
+``!v vty w. (size_of_bir_immtype vty <= w) ==>
             (v2bs (fixwidth w v) vty = v2bs v vty)``,
 
 GEN_TAC >> Cases >>
 SIMP_TAC (std_ss++wordsLib.WORD_ss) [v2bs_def, n2bs_def, n2w_v2n,
-  v2w_fixwidth_imp, size_of_bil_immtype_def]);
+  v2w_fixwidth_imp, size_of_bir_immtype_def]);
 
 val v2bs_n2v = store_thm ("v2bs_n2v",
   ``!n. v2bs (n2v n) = n2bs n``,
