birScript.sml
@@ -1,9 +1,11 @@
-open HolKernel Parse boolTheory boolLib pairTheory
-
-open HolBASimps birTheory;
+open HolKernel Parse boolLib bossLib;
+open wordsTheory bitstringTheory;
 open bir_auxiliaryTheory bir_immTheory bir_valuesTheory;
 open bir_imm_expTheory bir_mem_expTheory bir_envTheory;
 open bir_expTheory bir_programTheory bir_typingTheory;
+open wordsLib;
+
+val _ = new_theory "bir";
 
 
-val _ = Process.exit Process.success;
+val _ = export_theory();
