bir_expScript.sml
@@ -1,0 +1,428 @@
+open HolKernel Parse boolLib bossLib;
+open wordsTheory bitstringTheory;
+open bir_auxiliaryTheory bir_immTheory bir_valuesTheory;
+open bir_imm_expTheory bir_mem_expTheory bir_envTheory;
+
+val _ = new_theory "bir_exp";
+
+val bir_imm_ss = rewrites ((type_rws ``:bir_imm_t``) @ (type_rws ``:bir_immtype_t``));
+val bir_type_ss = rewrites ((type_rws ``:bir_type_t``));
+
+
+(* ------------------------------------------------------------------------- *)
+(*  Datatypes                                                                *)
+(* ------------------------------------------------------------------------- *)
+
+val _ = Datatype `bir_exp_t =
+    BExp_Const             bir_imm_t
+  | BExp_Den               bir_var_t
+
+  | BExp_Cast              bir_cast_t bir_exp_t bir_immtype_t
+
+  | BExp_UnaryExp          bir_unary_exp_t bir_exp_t
+  | BExp_BinExp            bir_bin_exp_t bir_exp_t bir_exp_t
+  | BExp_BinPred           bir_bin_pred_t bir_exp_t bir_exp_t
+
+    (* For some reason if-then-else officially misses in BAP documentation *)
+  | BExp_IfThenElse        bir_exp_t bir_exp_t bir_exp_t
+
+  | BExp_Load              bir_exp_t bir_exp_t bir_endian_t bir_immtype_t
+  | BExp_Store             bir_exp_t bir_exp_t bir_endian_t bir_exp_t
+`;
+
+
+(* ------------------------------------------------------------------------- *)
+(*  Semantics of expressions                                                 *)
+(* ------------------------------------------------------------------------- *)
+
+val bir_eval_cast_def = Define `
+  (bir_eval_cast ct (BVal_Imm bi) ty = BVal_Imm (bir_gencast ct bi ty)) /\
+  (bir_eval_cast _ _ _ = BVal_Unknown)`;
+
+val bir_eval_unary_exp_def = Define `
+  (bir_eval_unary_exp et (BVal_Imm bi) = BVal_Imm (bir_unary_exp et bi)) /\
+  (bir_eval_unary_exp _ _ = BVal_Unknown)`;
+
+val bir_eval_bin_exp_def = Define `
+  (bir_eval_bin_exp et (BVal_Imm bi1) (BVal_Imm bi2) =
+     if (type_of_bir_imm bi1 <> type_of_bir_imm bi2) then BVal_Unknown else
+     BVal_Imm (bir_bin_exp et bi1 bi2)) /\
+  (bir_eval_bin_exp _ _ _ = BVal_Unknown)`;
+
+val bir_eval_bin_pred_def = Define `
+  (bir_eval_bin_pred pt (BVal_Imm bi1) (BVal_Imm bi2) =
+     if (type_of_bir_imm bi1 <> type_of_bir_imm bi2) then BVal_Unknown else
+     BVal_Imm (bool2b (bir_bin_pred pt bi1 bi2))) /\
+  (bir_eval_bin_pred _ _ _ = BVal_Unknown)`;
+
+val bir_eval_ifthenelse_def = Define `
+  (bir_eval_ifthenelse (BVal_Imm (Imm1 cw)) e1 e2 =
+     if (cw = 1w) then e1 else e2) /\
+  (bir_eval_ifthenelse _ _ _ = BVal_Unknown)`;
+
+val bir_eval_load_def = Define `
+  (bir_eval_load (BVal_Mem ta tv mmap) (BVal_Imm a) en t =
+     if ((type_of_bir_imm a) = ta) then
+        (case (bir_load_from_mem tv t mmap en (b2n a)) of
+           NONE => BVal_Unknown
+         | SOME i => BVal_Imm i)
+     else BVal_Unknown) /\
+  (bir_eval_load _ _ _ _ = BVal_Unknown)`;
+
+val bir_eval_store_def = Define `
+  (bir_eval_store (BVal_Mem ta tv mmap) (BVal_Imm a) en (BVal_Imm v) =
+     if ((type_of_bir_imm a) = ta) then
+        (case (bir_store_in_mem tv v mmap en (b2n a)) of
+           NONE => BVal_Unknown
+         | SOME mmap' => BVal_Mem ta tv mmap')
+     else BVal_Unknown) /\
+  (bir_eval_store _ _ _ _ = BVal_Unknown)`;
+
+
+
+val bir_eval_exp_def = Define `
+  (bir_eval_exp (BExp_Const n) env = BVal_Imm n) /\
+
+  (bir_eval_exp (BExp_Den v) env = bir_env_read v env) /\
+
+  (bir_eval_exp (BExp_Cast ct e ty) env = (
+     bir_eval_cast ct (bir_eval_exp e env) ty)) /\
+
+  (bir_eval_exp (BExp_UnaryExp et e) env = (
+     bir_eval_unary_exp et (bir_eval_exp e env))) /\
+
+  (bir_eval_exp (BExp_BinExp et e1 e2) env = (
+     bir_eval_bin_exp et (bir_eval_exp e1 env) (bir_eval_exp e2 env))) /\
+
+  (bir_eval_exp (BExp_BinPred pt e1 e2) env = (
+     bir_eval_bin_pred pt (bir_eval_exp e1 env) (bir_eval_exp e2 env))) /\
+
+  (bir_eval_exp (BExp_IfThenElse c et ef) env =
+     bir_eval_ifthenelse (bir_eval_exp c env) (bir_eval_exp et env) (bir_eval_exp ef env)
+  ) /\
+
+  (bir_eval_exp (BExp_Load mem_e a_e en ty) env =
+     bir_eval_load (bir_eval_exp mem_e env) (bir_eval_exp a_e env) en ty) /\
+
+  (bir_eval_exp (BExp_Store mem_e a_e en v_e) env =
+     bir_eval_store (bir_eval_exp mem_e env) (bir_eval_exp a_e env) en (bir_eval_exp v_e env))
+`;
+
+
+
+
+(* ------------------------------------------------------------------------- *)
+(*  Rewrite theorems for eval                                                *)
+(* ------------------------------------------------------------------------- *)
+
+val bir_eval_cast_REWRS = store_thm ("bir_eval_cast_REWRS",
+``(!ct bi ty. (bir_eval_cast ct (BVal_Imm bi) ty = BVal_Imm (bir_gencast ct bi ty))) /\
+  (!ct ty. bir_eval_cast ct BVal_Unknown ty = BVal_Unknown) /\
+  (!ct at vt mmap ty. bir_eval_cast ct (BVal_Mem at vt mmap) ty = BVal_Unknown)``,
+SIMP_TAC std_ss [bir_eval_cast_def]);
+
+val bir_eval_unary_exp_REWRS = store_thm ("bir_eval_unary_exp_REWRS",
+ ``(!et bi. (bir_eval_unary_exp et (BVal_Imm bi) = BVal_Imm (bir_unary_exp et bi))) /\
+   (!et. bir_eval_unary_exp et BVal_Unknown = BVal_Unknown) /\
+   (!et at vt mmap. bir_eval_unary_exp et (BVal_Mem at vt mmap) = BVal_Unknown)``,
+SIMP_TAC std_ss [bir_eval_unary_exp_def]);
+
+
+val bir_eval_bin_exp_REWRS = store_thm ("bir_eval_bin_exp_REWRS",
+``(!et bi1 bi2. bir_eval_bin_exp et (BVal_Imm bi1) (BVal_Imm bi2) =
+     if (type_of_bir_imm bi1 <> type_of_bir_imm bi2) then BVal_Unknown else
+     BVal_Imm (bir_bin_exp et bi1 bi2)) /\
+  (!et v. bir_eval_bin_exp et BVal_Unknown v = BVal_Unknown) /\
+  (!et v. bir_eval_bin_exp et v BVal_Unknown = BVal_Unknown) /\
+  (!et at vt mmap v. bir_eval_bin_exp et (BVal_Mem at vt mmap) v = BVal_Unknown) /\
+  (!et at vt mmap v. bir_eval_bin_exp et v (BVal_Mem at vt mmap) = BVal_Unknown)``,
+SIMP_TAC std_ss [bir_eval_bin_exp_def] >>
+CONJ_TAC >| [
+  Cases_on `v` >> SIMP_TAC std_ss [bir_eval_bin_exp_def],
+  Cases_on `v` >> SIMP_TAC std_ss [bir_eval_bin_exp_def]
+]);
+
+val bir_eval_bin_pred_REWRS = store_thm ("bir_eval_bin_pred_REWRS",
+``(!et bi1 bi2. bir_eval_bin_pred et (BVal_Imm bi1) (BVal_Imm bi2) =
+     if (type_of_bir_imm bi1 <> type_of_bir_imm bi2) then BVal_Unknown else
+     BVal_Imm (bool2b (bir_bin_pred et bi1 bi2))) /\
+  (!et v. bir_eval_bin_pred et BVal_Unknown v = BVal_Unknown) /\
+  (!et v. bir_eval_bin_pred et v BVal_Unknown = BVal_Unknown) /\
+  (!et at vt mmap v. bir_eval_bin_pred et (BVal_Mem at vt mmap) v = BVal_Unknown) /\
+  (!et at vt mmap v. bir_eval_bin_pred et v (BVal_Mem at vt mmap) = BVal_Unknown)``,
+SIMP_TAC std_ss [bir_eval_bin_pred_def] >>
+CONJ_TAC >| [
+  Cases_on `v` >> SIMP_TAC std_ss [bir_eval_bin_pred_def],
+  Cases_on `v` >> SIMP_TAC std_ss [bir_eval_bin_pred_def]
+]);
+
+
+val bir_eval_ifthenelse_REWRS = store_thm ("bir_eval_ifthenelse_REWRS",
+``(!c e1 e2. bir_eval_ifthenelse (BVal_Imm c) e1 e2 =
+     if (type_of_bir_imm c = Bit1) then (
+       if (c = Imm1 1w) then e1 else e2
+     ) else BVal_Unknown) /\
+  (!c e1 e2. bir_eval_ifthenelse BVal_Unknown e1 e2 = BVal_Unknown) /\
+  (!at vt mmap e1 e2. bir_eval_ifthenelse (BVal_Mem at vt mmap) e1 e2 = BVal_Unknown)``,
+SIMP_TAC std_ss [bir_eval_ifthenelse_def] >>
+Cases_on `c` >> (
+  SIMP_TAC (std_ss++bir_imm_ss) [type_of_bir_imm_def, bir_eval_ifthenelse_def]
+));
+
+val bir_eval_ifthenelse_REWRS_Unknown = store_thm ("bir_eval_ifthenelse_REWRS_Unknown",
+``(!ec e1 e2.
+     (type_of_bir_val ec <> SOME (BType_Imm Bit1)) ==>
+     (bir_eval_ifthenelse ec e1 e2 = BVal_Unknown))``,
+
+Cases_on `ec` >> (
+  SIMP_TAC (std_ss++bir_type_ss++bir_imm_ss) [type_of_bir_imm_def, type_of_bir_val_def,
+    bir_eval_ifthenelse_REWRS]
+));
+
+val bir_eval_ifthenelse_TF_EQ = store_thm ("bir_eval_ifthenelse_TF_EQ",
+``!c e.
+     bir_eval_ifthenelse c e e =
+     if (bir_val_is_Bool c) then e else BVal_Unknown``,
+Cases_on `c` >> (
+  SIMP_TAC (std_ss++bir_imm_ss++bir_type_ss) [type_of_bir_imm_def, bir_eval_ifthenelse_REWRS,
+    bir_val_checker_REWRS]
+));
+
+
+val bir_eval_load_Unknown_REWRS1 = prove (
+  ``(!mem en t. bir_eval_load mem BVal_Unknown en t = BVal_Unknown) /\
+    (!mem en t aty vty mmap. bir_eval_load mem (BVal_Mem aty vty mmap) en t = BVal_Unknown)``,
+
+SIMP_TAC std_ss [bir_eval_load_def] >>
+REPEAT CONJ_TAC >>
+Cases_on `mem` >> SIMP_TAC std_ss [bir_eval_load_def]);
+
+val bir_eval_load_Unknown_REWRS2 = prove (
+  ``(!a en t. bir_eval_load BVal_Unknown a en t = BVal_Unknown) /\
+    (!a en t i. bir_eval_load (BVal_Imm i) a en t = BVal_Unknown)``,
+
+SIMP_TAC std_ss [bir_eval_load_def]);
+
+val bir_eval_load_Unknown_REWRS3 = prove (
+  ``!a en t i aty vty mmap.
+      (type_of_bir_imm i <> aty) ==>
+      (bir_eval_load (BVal_Mem aty vty mmap) (BVal_Imm i) en t = BVal_Unknown)``,
+
+SIMP_TAC std_ss [bir_eval_load_def]);
+
+
+val bir_eval_load_Unknown_REWRS4 = prove (
+  ``!a en t i aty vty mmap.
+      (t <> vty) ==>
+      (bir_eval_load (BVal_Mem aty vty mmap) (BVal_Imm i) BEnd_NoEndian t = BVal_Unknown)``,
+
+SIMP_TAC std_ss [bir_eval_load_def] >>
+REPEAT STRIP_TAC >>
+COND_CASES_TAC >> SIMP_TAC std_ss [] >>
+ASM_SIMP_TAC std_ss [bir_load_from_mem_NO_ENDIAN]);
+
+val bir_eval_load_Unknown_REWRS5 = prove (
+  ``!a en t i aty vty mmap en.
+      (bir_number_of_mem_splits vty t = NONE) ==>
+      (bir_eval_load (BVal_Mem aty vty mmap) (BVal_Imm i) en t = BVal_Unknown)``,
+
+SIMP_TAC std_ss [bir_eval_load_def] >>
+REPEAT STRIP_TAC >>
+COND_CASES_TAC >> SIMP_TAC std_ss [] >>
+ASM_SIMP_TAC std_ss [bir_load_from_mem_def]);
+
+
+val bir_eval_load_Unknown_REWRS = save_thm ("bir_eval_load_Unknown_REWRS",
+  REWRITE_RULE [GSYM CONJ_ASSOC] (
+  LIST_CONJ [bir_eval_load_Unknown_REWRS1, bir_eval_load_Unknown_REWRS2,
+             bir_eval_load_Unknown_REWRS3, bir_eval_load_Unknown_REWRS4,
+             bir_eval_load_Unknown_REWRS5]));
+
+
+val bir_eval_load_SINGLE_REWR = store_thm ("bir_eval_load_SINGLE_REWR",
+  ``!a en t i aty vty mmap en.
+      (bir_eval_load (BVal_Mem aty vty mmap) (BVal_Imm i) en vty) =
+      ((if (type_of_bir_imm i = aty) then (BVal_Imm (n2bs (mmap (b2n i)) vty))
+       else BVal_Unknown))``,
+
+SIMP_TAC arith_ss [bir_eval_load_def, bir_load_from_mem_SINGLE]);
+
+
+val bir_eval_load_BASIC_REWR = store_thm ("bir_eval_load_BASIC_REWR",
+  ``!a en t i aty vty ty mmap en.
+      (bir_eval_load (BVal_Mem aty vty mmap) (BVal_Imm i) en ty) =
+      (if type_of_bir_imm i = aty then
+        case bir_load_from_mem vty ty mmap en (b2n i) of
+          NONE => BVal_Unknown
+        | SOME i => BVal_Imm i
+       else BVal_Unknown)``,
+SIMP_TAC arith_ss [bir_eval_load_def]);
+
+
+val bir_eval_load_FULL_REWRS = save_thm ("bir_eval_load_FULL_REWRS",
+let
+  val thm_prune0 = prove (``(!ta a.
+      (type_of_bir_imm a <> ta) ==>
+      (bir_eval_load (BVal_Mem ta tv mmap) (BVal_Imm a) en tr = BVal_Unknown)) /\
+      (!tr tv.
+      (tr <> tv) ==> (bir_number_of_mem_splits tv tr <> NONE) ==>
+      (bir_eval_load (BVal_Mem ta tv mmap) (BVal_Imm i) BEnd_NoEndian tr = BVal_Unknown)) /\
+      (!tr tv.
+      (bir_number_of_mem_splits tv tr = NONE) ==>
+      (bir_eval_load (BVal_Mem ta tv mmap) (BVal_Imm i) en tr = BVal_Unknown))``,
+   SIMP_TAC std_ss [bir_eval_load_Unknown_REWRS])
+
+  val thm_prune1 = SIMP_RULE (std_ss ++ bir_imm_ss ++ DatatypeSimps.expand_type_quants_ss [``:bir_immtype_t``, ``:bir_imm_t``]) [bir_number_of_mem_splits_REWRS, type_of_bir_imm_def] thm_prune0
+
+  val thm_prune2 = SIMP_RULE std_ss [FORALL_AND_THM, GSYM CONJ_ASSOC] (GEN_ALL thm_prune1)
+
+
+  val thm0 = bir_eval_load_BASIC_REWR
+
+  val thm1 = SIMP_RULE (list_ss ++ bir_imm_ss ++ DatatypeSimps.expand_type_quants_ss [``:bir_immtype_t``, ``:bir_imm_t``, ``:bir_endian_t``]) [ type_of_bir_imm_def, size_of_bir_immtype_def, bir_number_of_mem_splits_REWRS, bir_load_from_mem_REWRS, thm_prune2]
+     thm0
+
+  val thm2 = Ho_Rewrite.REWRITE_RULE [fold_bir_endian_THM] thm1
+
+  val thm3 = SIMP_RULE (list_ss) [
+     FORALL_AND_THM, b2n_MOD_2EXP, type_of_bir_imm_def, size_of_bir_immtype_def]
+     thm2
+
+  val thm4 = REWRITE_RULE [b2n_def, GSYM CONJ_ASSOC] (CONJ thm3 thm_prune2)
+in thm4
+end);
+
+
+
+val bir_eval_store_Unknown_REWRS1 = prove (
+  ``(!mem en v. bir_eval_store mem BVal_Unknown en v = BVal_Unknown) /\
+    (!mem en v aty vty mmap. bir_eval_store mem (BVal_Mem aty vty mmap) en v = BVal_Unknown)``,
+
+SIMP_TAC std_ss [bir_eval_store_def] >>
+REPEAT CONJ_TAC >>
+Cases_on `mem` >> SIMP_TAC std_ss [bir_eval_store_def]);
+
+val bir_eval_store_Unknown_REWRS2 = prove (
+  ``(!a en v. bir_eval_store BVal_Unknown a en v = BVal_Unknown) /\
+    (!a en v i. bir_eval_store (BVal_Imm i) a en v = BVal_Unknown)``,
+
+SIMP_TAC std_ss [bir_eval_store_def]);
+
+
+val bir_eval_store_Unknown_REWRS3 = prove (
+  ``(!a en mem. bir_eval_store mem a en BVal_Unknown = BVal_Unknown) /\
+    (!a en mem ta tv mmap. bir_eval_store mem a en (BVal_Mem ta tv mmap) = BVal_Unknown)``,
+
+REPEAT CONJ_TAC >>
+Cases_on `mem` >> Cases_on `a` >> SIMP_TAC std_ss [bir_eval_store_def]);
+
+
+val bir_eval_store_Unknown_REWRS4 = prove (
+  ``!en v i aty vty mmap.
+      (type_of_bir_imm i <> aty) ==>
+      (bir_eval_store (BVal_Mem aty vty mmap) (BVal_Imm i) en v = BVal_Unknown)``,
+Cases_on `v` >>
+SIMP_TAC std_ss [bir_eval_store_def]);
+
+
+val bir_eval_store_Unknown_REWRS5 = prove (
+  ``!a en v aty vty mmap.
+      (type_of_bir_imm v <> vty) ==>
+      (bir_eval_store (BVal_Mem aty vty mmap) a BEnd_NoEndian (BVal_Imm v) = BVal_Unknown)``,
+
+Cases_on `a` >> SIMP_TAC std_ss [bir_eval_store_def] >>
+REPEAT STRIP_TAC >>
+COND_CASES_TAC >> SIMP_TAC std_ss [] >>
+ASM_SIMP_TAC std_ss [bir_store_in_mem_NO_ENDIAN]);
+
+
+val bir_eval_store_Unknown_REWRS6 = prove (
+  ``!a en v aty vty mmap en.
+      (bir_number_of_mem_splits vty (type_of_bir_imm v) = NONE) ==>
+      (bir_eval_store (BVal_Mem aty vty mmap) a en (BVal_Imm v) = BVal_Unknown)``,
+
+Cases_on `a` >> SIMP_TAC std_ss [bir_eval_store_def, LET_DEF] >>
+REPEAT STRIP_TAC >>
+COND_CASES_TAC >> SIMP_TAC std_ss [] >>
+ASM_SIMP_TAC std_ss [bir_store_in_mem_def, LET_DEF]);
+
+
+val bir_eval_store_Unknown_REWRS = save_thm ("bir_eval_store_Unknown_REWRS",
+  SIMP_RULE std_ss [GSYM CONJ_ASSOC] (
+  LIST_CONJ [bir_eval_store_Unknown_REWRS1, bir_eval_store_Unknown_REWRS2,
+             bir_eval_store_Unknown_REWRS3, bir_eval_store_Unknown_REWRS4,
+             bir_eval_store_Unknown_REWRS5, bir_eval_store_Unknown_REWRS6]));
+
+val bir_eval_store_SINGLE_REWR = store_thm ("bir_eval_store_SINGLE_REWR",
+  ``!a en t i aty v vty mmap en.
+      ((type_of_bir_imm i = aty) /\ (type_of_bir_imm v = vty)) ==>
+      (bir_eval_store (BVal_Mem aty vty mmap) (BVal_Imm i) en (BVal_Imm v) =
+      (BVal_Mem aty vty ((b2n i =+ b2n v) mmap)))``,
+
+SIMP_TAC arith_ss [bir_eval_store_def, bir_store_in_mem_SINGLE]);
+
+
+
+val bir_eval_store_BASIC_REWR = store_thm ("bir_eval_store_BASIC_REWR",
+  ``!a en t i aty v vty mmap en.
+      (bir_eval_store (BVal_Mem aty vty mmap) (BVal_Imm i) en (BVal_Imm v) =
+      (if type_of_bir_imm i = aty then
+         case bir_store_in_mem vty v mmap en (b2n i) of
+           NONE => BVal_Unknown
+         | SOME mmap' => BVal_Mem aty vty mmap'
+       else BVal_Unknown))``,
+
+SIMP_TAC arith_ss [bir_eval_store_def]);
+
+
+val bir_eval_store_FULL_REWRS = save_thm ("bir_eval_store_FULL_REWRS",
+let
+  val thm_prune0 = prove (``(!ta a.
+      (type_of_bir_imm a <> ta) ==>
+      (bir_eval_store (BVal_Mem ta tv mmap) (BVal_Imm a) en v = BVal_Unknown)) /\
+      (!i tv.
+      (type_of_bir_imm i <> tv) ==> (bir_number_of_mem_splits tv (type_of_bir_imm i) <> NONE) ==>
+      (bir_eval_store (BVal_Mem ta tv mmap) a BEnd_NoEndian (BVal_Imm i) = BVal_Unknown)) /\
+      (!i tv.
+      (bir_number_of_mem_splits tv (type_of_bir_imm i) = NONE) ==>
+      (bir_eval_store (BVal_Mem ta tv mmap) a en (BVal_Imm i) = BVal_Unknown))``,
+   SIMP_TAC std_ss [bir_eval_store_Unknown_REWRS])
+
+  val thm_prune1 = SIMP_RULE (std_ss ++ bir_imm_ss ++ DatatypeSimps.expand_type_quants_ss [``:bir_immtype_t``, ``:bir_imm_t``]) [bir_number_of_mem_splits_REWRS, type_of_bir_imm_def] thm_prune0
+
+  val thm_prune2 = SIMP_RULE std_ss [FORALL_AND_THM, GSYM CONJ_ASSOC] (GEN_ALL thm_prune1)
+
+
+  val thm0 = SIMP_RULE (std_ss) [bir_eval_store_Unknown_REWRS, FORALL_AND_THM] bir_eval_store_BASIC_REWR
+
+  val thm1 = SIMP_RULE (list_ss++ bir_imm_ss ++ DatatypeSimps.expand_type_quants_ss [``:bir_immtype_t``, ``:bir_imm_t``, ``:bir_endian_t``]) [ type_of_bir_imm_def, size_of_bir_immtype_def, bir_number_of_mem_splits_REWRS, bir_store_in_mem_REWRS, thm_prune2]
+     thm0
+
+  val thm2 = Ho_Rewrite.REWRITE_RULE [fold_bir_endian_THM] thm1
+
+  val thm3 = SIMP_RULE (list_ss) [
+     FORALL_AND_THM, type_of_bir_imm_def, size_of_bir_immtype_def]
+     thm2
+
+  val thm4 = REWRITE_RULE [b2n_def, GSYM CONJ_ASSOC] (CONJ thm3 thm_prune2)
+in thm4
+end);
+
+
+(* ------------------------------------------------------------------------- *)
+(*  Boolean Expressions                                                      *)
+(* ------------------------------------------------------------------------- *)
+
+val bir_dest_bool_val_def = Define `
+  (bir_dest_bool_val (BVal_Imm (Imm1 w)) = SOME (w = 1w)) /\
+  (bir_dest_bool_val _ = NONE)`
+
+val bir_dest_bool_val_EQ_NONE = store_thm ("bir_dest_bool_val_EQ_NONE",
+  ``!v. (bir_dest_bool_val v = NONE) <=> ~(bir_val_is_Bool v)``,
+Cases >> SIMP_TAC std_ss [bir_val_checker_REWRS, bir_dest_bool_val_def] >>
+Cases_on `b` >> SIMP_TAC (std_ss++bir_imm_ss) [bir_val_checker_REWRS, bir_dest_bool_val_def,
+  type_of_bir_imm_def]);
+
+
+
+val _ = export_theory();
