bir_mem_expScript.sml
@@ -1,0 +1,802 @@
+open HolKernel Parse boolLib bossLib;
+open wordsTheory bitstringTheory;
+open bir_auxiliaryTheory bir_immTheory;
+
+val _ = new_theory "bir_mem_exp";
+
+val bir_imm_ss = rewrites ((type_rws ``:bir_imm_t``) @ (type_rws ``:bir_immtype_t``));
+
+
+(* ------------------------------------------------------------------------- *)
+(* Endian for memory                                                         *)
+(* ------------------------------------------------------------------------- *)
+
+val _ = Datatype `bir_endian_t =
+  | BEnd_BigEndian
+  | BEnd_LittleEndian
+  | BEnd_NoEndian`
+
+val bir_endian_ss = rewrites (type_rws ``:bir_endian_t``);
+
+val fold_bir_endian_THM = store_thm ("fold_bir_endian_THM", 
+  ``!P. (P BEnd_BigEndian /\ P BEnd_LittleEndian /\ P BEnd_NoEndian) <=> (!en. P en)``,
+    SIMP_TAC (std_ss++DatatypeSimps.expand_type_quants_ss [``:bir_endian_t``]) []);
+
+
+(* ------------------------------------------------------------------------- *)
+(*  How many splits are needed                                               *)
+(* ------------------------------------------------------------------------- *)
+
+(* given a value- and a result_type, compute how many values are needed to
+   form a result. If the length of the result is not devidable by the value size
+   return NONE. *)
+val bir_number_of_mem_splits_def = Define `bir_number_of_mem_splits
+   (value_ty : bir_immtype_t) (result_ty : bir_immtype_t) =
+   if ((size_of_bir_immtype result_ty) MOD (size_of_bir_immtype value_ty) = 0) then
+      SOME ((size_of_bir_immtype result_ty) DIV (size_of_bir_immtype value_ty))
+   else NONE`;
+
+val bir_number_of_mem_splits_REWRS = save_thm ("bir_number_of_mem_splits_REWRS",
+  SIMP_RULE (std_ss++DatatypeSimps.expand_type_quants_ss [``:bir_immtype_t``]) [
+    size_of_bir_immtype_def, GSYM CONJ_ASSOC]
+     bir_number_of_mem_splits_def)
+
+val bir_number_of_mem_splits_NEQ_SOME0 = store_thm ("bir_number_of_mem_splits_NEQ_SOME0",
+  ``!vt rt. bir_number_of_mem_splits vt rt <> SOME 0``,
+Cases >> Cases >> SIMP_TAC std_ss [bir_number_of_mem_splits_def, size_of_bir_immtype_def]);
+
+val bir_number_of_mem_splits_ID = store_thm ("bir_number_of_mem_splits_ID",
+  ``!r. bir_number_of_mem_splits r r = SOME 1``,
+Cases >> SIMP_TAC std_ss [bir_number_of_mem_splits_REWRS]);
+
+
+val bir_number_of_mem_splits_EQ_SOME1 = store_thm ("bir_number_of_mem_splits_EQ_SOME1",
+  ``!vt rt. (bir_number_of_mem_splits vt rt = SOME 1) <=> (vt = rt)``,
+Cases >> Cases >> SIMP_TAC (std_ss++bir_imm_ss) [bir_number_of_mem_splits_REWRS]);
+
+
+
+
+(* ------------------------------------------------------------------------- *)
+(*  Loading                                                                  *)
+(* ------------------------------------------------------------------------- *)
+
+val bir_mem_concat_def = Define `bir_mem_concat vl rty = v2bs (FLAT vl) rty`
+
+val type_of_bir_mem_concat = store_thm ("type_of_bir_mem_concat",
+  ``!vl ty. type_of_bir_imm (bir_mem_concat vl ty) = ty``,
+SIMP_TAC std_ss [bir_mem_concat_def, type_of_v2bs]);
+
+val bir_load_bitstring_from_mmap_def = Define `
+  bir_load_bitstring_from_mmap value_ty mmap a =
+    fixwidth (size_of_bir_immtype value_ty) (n2v (mmap a))`
+
+val bir_load_bitstring_from_mmap_w2v = store_thm ("bir_load_bitstring_from_mmap_w2v",
+  ``!value_ty mmap a. (size_of_bir_immtype value_ty = dimindex (:'a)) ==>
+      (bir_load_bitstring_from_mmap value_ty mmap a =
+       (w2v ((n2w (mmap a)):'a word)))``,
+SIMP_TAC std_ss [bir_load_bitstring_from_mmap_def, GSYM w2v_v2w, v2w_n2v]);
+
+
+val bir_load_bitstring_from_mmap_w2v_THMS = store_thm ("bir_load_bitstring_from_mmap_w2v_THMS",
+``(!mmap a. (bir_load_bitstring_from_mmap Bit1  mmap a = (w2v ((n2w (mmap a)):word1)))) /\
+  (!mmap a. (bir_load_bitstring_from_mmap Bit8  mmap a = (w2v ((n2w (mmap a)):word8)))) /\
+  (!mmap a. (bir_load_bitstring_from_mmap Bit16 mmap a = (w2v ((n2w (mmap a)):word16)))) /\
+  (!mmap a. (bir_load_bitstring_from_mmap Bit32 mmap a = (w2v ((n2w (mmap a)):word32)))) /\
+  (!mmap a. (bir_load_bitstring_from_mmap Bit64 mmap a = (w2v ((n2w (mmap a)):word64))))``,
+
+REPEAT STRIP_TAC >> (
+  MATCH_MP_TAC bir_load_bitstring_from_mmap_w2v >>
+  SIMP_TAC (std_ss++wordsLib.WORD_ss) [size_of_bir_immtype_def]
+));
+
+
+val bir_load_from_mem_def = Define `bir_load_from_mem
+  (value_ty : bir_immtype_t) (result_ty : bir_immtype_t) (mmap : num -> num) (en: bir_endian_t) (a:num) =
+
+   case (bir_number_of_mem_splits value_ty result_ty) of
+    | NONE => NONE
+    | SOME (n:num) => (
+        let vs = MAP (\n. bir_load_bitstring_from_mmap value_ty mmap (a+n)) (COUNT_LIST n) in
+        let vs' = (case en of BEnd_LittleEndian => SOME (REVERSE vs)
+                          |  BEnd_BigEndian => SOME vs
+                          |  BEnd_NoEndian => if (n = 1) then SOME vs else NONE) in
+        case vs' of NONE => NONE
+                 |  SOME vs'' => SOME (bir_mem_concat vs'' result_ty)
+   )`;
+
+val bir_load_from_mem_SINGLE = store_thm ("bir_load_from_mem_SINGLE",
+  ``!en a vty mmap. bir_load_from_mem vty vty mmap en a =
+    SOME (n2bs (mmap a) vty)``,
+
+SIMP_TAC list_ss [bir_load_from_mem_def, bir_number_of_mem_splits_ID, LET_THM,
+  rich_listTheory.count_list_sub1, rich_listTheory.COUNT_LIST_def] >>
+Cases_on `en` >> (
+  SIMP_TAC (list_ss++bir_endian_ss) [bir_mem_concat_def, v2bs_fixwidth,
+    v2bs_n2v, bir_load_bitstring_from_mmap_def]
+));
+
+
+val bir_load_from_mem_NO_ENDIAN = store_thm ("bir_load_from_mem_NO_ENDIAN",
+  ``!a vty rty mmap. bir_load_from_mem vty rty mmap BEnd_NoEndian a =
+    (if vty = rty then
+      SOME (n2bs (mmap a) vty)
+     else NONE)``,
+
+REPEAT GEN_TAC >>
+Cases_on `vty = rty` >> (
+  ASM_SIMP_TAC std_ss [bir_load_from_mem_SINGLE]
+) >>
+`bir_number_of_mem_splits vty rty <> SOME 1` by (
+  Cases_on `vty` >> Cases_on `rty` >>
+  FULL_SIMP_TAC std_ss [bir_number_of_mem_splits_REWRS]
+) >>
+Cases_on `bir_number_of_mem_splits vty rty` >> (
+  FULL_SIMP_TAC (std_ss++bir_endian_ss) [bir_load_from_mem_def, LET_DEF]
+));
+
+
+val bir_load_from_mem_EQ_NONE = store_thm ("bir_load_from_mem_EQ_NONE",
+  ``!a en vty rty mmap. (bir_load_from_mem vty rty mmap en a = NONE) <=>
+      ((bir_number_of_mem_splits vty rty = NONE) \/
+      ((vty <> rty) /\ (en = BEnd_NoEndian)))``,
+
+REPEAT GEN_TAC >>
+ASM_REWRITE_TAC [GSYM bir_number_of_mem_splits_EQ_SOME1] >>
+Cases_on `bir_number_of_mem_splits vty rty` >> (
+  ASM_SIMP_TAC std_ss [bir_load_from_mem_def, LET_DEF]
+) >>
+Cases_on `en` >> (
+  ASM_SIMP_TAC (std_ss++bir_endian_ss) []
+) >>
+Cases_on `x=1` >> ASM_SIMP_TAC std_ss []);
+
+
+val bir_load_from_mem_EQ_NONE_IMP = store_thm ("bir_load_from_mem_EQ_NONE_IMP",
+  ``!a en vty rty mmap. 
+      ((bir_number_of_mem_splits vty rty = NONE) \/
+      ((vty <> rty) /\ (en = BEnd_NoEndian))) ==>
+      (bir_load_from_mem vty rty mmap en a = NONE)``,
+METIS_TAC[bir_load_from_mem_EQ_NONE]);
+
+
+val bir_load_from_mem_EQ_SOME = store_thm ("bir_load_from_mem_EQ_SOME",
+  ``!a en vty rty mmap res. (bir_load_from_mem vty rty mmap en a = SOME res) <=>
+      (?n vs vs'. (bir_number_of_mem_splits vty rty = SOME n) /\
+                  (vs = MAP (\n. bir_load_bitstring_from_mmap vty mmap (a+n)) (COUNT_LIST n)) /\
+                  ((en = BEnd_BigEndian) /\ (vs' = vs) \/
+                   (en = BEnd_LittleEndian) /\ (vs' = REVERSE vs) \/
+                   (en = BEnd_NoEndian) /\ (n = 1) /\ (vs' = vs)) /\
+                   (res = bir_mem_concat vs' rty))``,
+
+SIMP_TAC std_ss [bir_load_from_mem_def] >>
+REPEAT GEN_TAC >>
+Cases_on `bir_number_of_mem_splits vty rty` >> (
+  ASM_SIMP_TAC std_ss [LET_DEF]
+) >>
+Cases_on `en` >> (
+  ASM_SIMP_TAC (std_ss++bir_endian_ss++boolSimps.EQUIV_EXTRACT_ss) []
+) >>
+Cases_on `x=1` >>
+ASM_SIMP_TAC (std_ss++boolSimps.EQUIV_EXTRACT_ss) []);
+
+
+
+val type_of_bir_load_from_mem = store_thm ("type_of_bir_load_from_mem",
+  ``!a en vty rty mmap res. (bir_load_from_mem vty rty mmap en a = SOME res) ==>
+      (type_of_bir_imm res = rty)``,
+
+SIMP_TAC std_ss [bir_load_from_mem_EQ_SOME, GSYM LEFT_FORALL_IMP_THM,
+  type_of_bir_mem_concat]);
+
+
+val bir_load_from_mem_NONE_REWRS = save_thm ("bir_load_from_mem_NONE_REWRS",
+let
+  val thm0 = bir_load_from_mem_EQ_NONE_IMP
+
+  val thm1 = SIMP_RULE (list_ss++DatatypeSimps.expand_type_quants_ss [``:bir_immtype_t``]) [
+    bir_number_of_mem_splits_REWRS] thm0
+
+  val thm2 = SIMP_RULE (std_ss++bir_imm_ss) [GSYM CONJ_ASSOC, FORALL_AND_THM] thm1
+in thm2 end);
+
+
+(* One first rewrite *)
+val bir_load_from_mem_REWRS0 = save_thm ("bir_load_from_mem_REWRS0",
+let
+  val thm0 = bir_load_from_mem_def
+
+  val thm1 = SIMP_RULE (list_ss++DatatypeSimps.expand_type_quants_ss [``:bir_immtype_t``]) [
+    bir_number_of_mem_splits_REWRS, rich_listTheory.count_list_sub1, rich_listTheory.COUNT_LIST_def, bir_load_bitstring_from_mmap_w2v_THMS] thm0
+
+  val thm2 = SIMP_RULE (list_ss++bir_endian_ss++(DatatypeSimps.expand_type_quants_ss [``:bir_endian_t``])) [LET_DEF] thm1
+
+  val thm3 = Ho_Rewrite.REWRITE_RULE [fold_bir_endian_THM] thm2
+
+  val thm4 = SIMP_RULE std_ss [GSYM CONJ_ASSOC, FORALL_AND_THM] thm3
+
+in thm4
+end)
+
+(* And a fancier one *)
+val bir_load_from_mem_REWRS = save_thm ("bir_load_from_mem_REWRS",
+let
+  val thm0 = bir_load_from_mem_REWRS0
+  val thm1 = SIMP_RULE (list_ss) [bir_mem_concat_def, v2bs_def, n2bs_def] thm0
+  val thm2 = SIMP_RULE std_ss [GSYM listTheory.APPEND_ASSOC] thm1
+  val thm3 = REWRITE_RULE [w2v_word_concat_SYM_REWRS] thm2
+  val thm4 = REWRITE_RULE [n2w_v2n, v2w_w2v] thm3
+in
+  thm4
+end);
+
+
+(* Important addresses *)
+val bir_load_from_mem_used_addrs_def = Define
+  `bir_load_from_mem_used_addrs tv tr en a =
+   case (bir_number_of_mem_splits tv tr) of
+    | NONE => {}
+    | SOME (n:num) => (if (n <> 1) /\ (en = BEnd_NoEndian) then {} else
+        set (MAP (\n. a + n) (COUNT_LIST n)))`
+
+val bir_load_from_mem_used_addrs_THM = store_thm ("bir_load_from_mem_used_addrs_THM",
+  ``!vt rt mmap mmap' en a.
+      (!addr. addr IN (bir_load_from_mem_used_addrs vt rt en a) ==>
+              (mmap addr = mmap' addr)) ==>
+      (bir_load_from_mem vt rt mmap en a =
+       bir_load_from_mem vt rt mmap' en a)``,
+
+SIMP_TAC std_ss [bir_load_from_mem_def, bir_load_from_mem_used_addrs_def] >>
+REPEAT GEN_TAC >>
+Cases_on `bir_number_of_mem_splits vt rt` >- (
+  ASM_SIMP_TAC std_ss []
+) >>
+ASM_SIMP_TAC std_ss [] >>
+COND_CASES_TAC >- (
+  FULL_SIMP_TAC (list_ss++bir_endian_ss) [LET_DEF]
+) >>
+POP_ASSUM (K ALL_TAC) >>
+STRIP_TAC >>
+`MAP (\n. bir_load_bitstring_from_mmap vt mmap (a + n)) (COUNT_LIST x) =
+ MAP (\n. bir_load_bitstring_from_mmap vt mmap' (a + n)) (COUNT_LIST x)` suffices_by (
+  ASM_SIMP_TAC std_ss []
+) >>
+
+FULL_SIMP_TAC list_ss [listTheory.MAP_EQ_f, listTheory.MEM_MAP,
+  GSYM LEFT_FORALL_IMP_THM, bir_load_bitstring_from_mmap_def]);
+
+
+val bir_load_from_mem_used_addrs_REWRS = save_thm ("bir_load_from_mem_used_addrs_REWRS",
+let
+  val thm0 = bir_load_from_mem_used_addrs_def
+
+  val thm1 = SIMP_RULE (list_ss++DatatypeSimps.expand_type_quants_ss [``:bir_immtype_t``]) [
+bir_number_of_mem_splits_REWRS, rich_listTheory.count_list_sub1, rich_listTheory.COUNT_LIST_def,
+   GSYM CONJ_ASSOC] thm0
+in thm1
+end);
+
+
+val bir_load_from_mem_used_addrs_FINITE = store_thm ("bir_load_from_mem_used_addrs_FINITE",
+  ``!tv tr en a.
+      FINITE (bir_load_from_mem_used_addrs tv tr en a)``,
+REPEAT GEN_TAC >>
+SIMP_TAC std_ss [bir_load_from_mem_used_addrs_def] >>
+Cases_on `bir_number_of_mem_splits tv tr` >> ASM_SIMP_TAC std_ss [pred_setTheory.FINITE_EMPTY] >>
+COND_CASES_TAC >> ASM_SIMP_TAC std_ss [pred_setTheory.FINITE_EMPTY, listTheory.FINITE_LIST_TO_SET]);
+
+
+val bir_load_from_mem_used_addrs_EMPTY = store_thm ("bir_load_from_mem_used_addrs_EMPTY",
+  ``!mmap tv tr en a.
+      (bir_load_from_mem_used_addrs tv tr en a = {}) <=>
+      (bir_load_from_mem tv tr mmap en a = NONE)``,
+
+REPEAT GEN_TAC >>
+SIMP_TAC std_ss [bir_load_from_mem_EQ_NONE, bir_load_from_mem_used_addrs_def,
+  GSYM bir_number_of_mem_splits_EQ_SOME1] >>
+Cases_on `bir_number_of_mem_splits tv tr` >> ASM_SIMP_TAC std_ss [] >>
+COND_CASES_TAC >> ASM_SIMP_TAC std_ss [] >>
+POP_ASSUM (K ALL_TAC) >>
+Cases_on `x` >- (
+  FULL_SIMP_TAC std_ss [bir_number_of_mem_splits_NEQ_SOME0]
+) >>
+SIMP_TAC list_ss [rich_listTheory.COUNT_LIST_def]);
+
+
+val bir_load_from_mem_used_addrs_NoEndian = store_thm ("bir_load_from_mem_used_addrs_NoEndian",
+  ``!tv tr a.
+      (bir_load_from_mem_used_addrs tv tr BEnd_NoEndian a = {}) \/
+      (bir_load_from_mem_used_addrs tv tr BEnd_NoEndian a = {a})``,
+
+REPEAT GEN_TAC >>
+SIMP_TAC std_ss [bir_load_from_mem_EQ_NONE, bir_load_from_mem_used_addrs_def] >>
+Cases_on `bir_number_of_mem_splits tv tr` >> ASM_SIMP_TAC std_ss [] >>
+COND_CASES_TAC >> ASM_SIMP_TAC std_ss [] >>
+SIMP_TAC list_ss [rich_listTheory.count_list_sub1,
+  rich_listTheory.COUNT_LIST_def])
+
+
+
+
+(* ------------------------------------------------------------------------- *)
+(*  Storing                                                                  *)
+(* ------------------------------------------------------------------------- *)
+
+
+(* =============== *)
+(* bitstring_split *)
+(* =============== *)
+
+val bitstring_split_aux_defn = Hol_defn "bitstring_split_aux"
+ `(bitstring_split_aux 0 acc bs = ARB) /\
+  (bitstring_split_aux n acc [] = REVERSE acc) /\
+  (bitstring_split_aux n acc bs =
+     bitstring_split_aux n ((TAKE n bs)::acc) (DROP n bs))`
+
+(* Defn.tgoal bitstring_split_aux_defn *)
+val (bitstring_split_aux_def, bitstring_split_aux_ind) = Defn.tstore_defn (bitstring_split_aux_defn,
+  WF_REL_TAC `measure (\ (_, _, l). LENGTH l)` >>
+  SIMP_TAC list_ss []);
+
+val bitstring_split_def = Define `bitstring_split n bs = bitstring_split_aux n [] bs`
+
+val bitstring_split_aux_REWR1 = SIMP_RULE std_ss [] (prove (``!n (_ : 'a list list) bs.
+  (!acc. (n <> 0) ==> (bitstring_split_aux n acc (bs:'a list) =
+         (REVERSE acc) ++ (bitstring_split_aux n [] bs)))``,
+
+HO_MATCH_MP_TAC bitstring_split_aux_ind >>
+REWRITE_TAC [numTheory.NOT_SUC] >>
+REPEAT STRIP_TAC >| [
+  SIMP_TAC list_ss [bitstring_split_aux_def],
+
+  REWRITE_TAC [bitstring_split_aux_def] >>
+  ONCE_ASM_REWRITE_TAC[] >>
+  SIMP_TAC list_ss []
+]));
+
+
+val bitstring_split_aux_REWR2 = prove (``!n acc x xs.
+  (bitstring_split_aux (SUC n) acc (x::xs) =
+  (bitstring_split_aux (SUC n) ((TAKE (SUC n) (x::xs))::acc) (DROP (SUC n) (x::xs))))``,
+REWRITE_TAC[bitstring_split_aux_def]);
+
+
+val bitstring_split_REWRS = store_thm ("bitstring_split_REWRS",
+  ``(!n. n <> 0 ==> (bitstring_split n [] = [])) /\
+    (!n bs. n <> 0 /\ bs <> [] ==> (bitstring_split n bs = (TAKE n bs) :: (bitstring_split n (DROP n bs))))``,
+
+SIMP_TAC std_ss [bitstring_split_def] >>
+CONJ_TAC >- (
+  Cases >> REWRITE_TAC [bitstring_split_aux_def, listTheory.REVERSE_DEF]
+) >>
+Cases >> Cases >> SIMP_TAC list_ss [bitstring_split_aux_REWR2] >>
+SIMP_TAC list_ss [Once bitstring_split_aux_REWR1]);
+
+
+val bitstring_split_REWRS_LENGTH = store_thm ("bitstring_split_REWRS_LENGTH",
+  ``(!n bs. n <> 0 /\ (LENGTH bs = 0) ==> (bitstring_split n bs = [])) /\
+    (!n bs. n <> 0 /\ 0 < LENGTH bs ==> (bitstring_split n bs = (TAKE n bs) :: (bitstring_split n (DROP n bs))))``,
+
+REPEAT STRIP_TAC >> (
+  Cases_on `bs` >>
+  FULL_SIMP_TAC list_ss [bitstring_split_REWRS]
+));
+
+
+val bitstring_split_INDUCT = store_thm ("bitstring_split_INDUCT",
+``!n P. (n <> 0 /\
+        (P [] /\ (!l. (l <> [] /\ P (DROP n l)) ==> P l))) ==>
+        (!l. P l)``,
+
+REPEAT STRIP_TAC >>
+completeInduct_on `LENGTH l` >>
+Cases_on `v` >> Cases_on `l` >> ASM_SIMP_TAC list_ss []
+)
+
+val bitstring_split_FLAT = store_thm ("bitstring_split_FLAT",
+  ``!n. n <> 0 ==> !bs. (FLAT (bitstring_split n bs) = bs)``,
+
+GEN_TAC >> STRIP_TAC >>
+HO_MATCH_MP_TAC (Q.SPEC `n` bitstring_split_INDUCT) >>
+ASM_SIMP_TAC list_ss [bitstring_split_REWRS]);
+
+
+val bitstring_split_LENGTHS = store_thm ("bitstring_split_LENGTHS",
+  ``!n m bs. n <> 0 /\ (LENGTH bs = m*n) ==> (
+      (EVERY (\l. LENGTH l = n) (bitstring_split n bs)) /\
+      (LENGTH (bitstring_split n bs) = m))``,
+
+GEN_TAC >>
+Induct >- (
+  Cases >> SIMP_TAC list_ss [bitstring_split_REWRS]
+) >>
+SIMP_TAC list_ss [arithmeticTheory.MULT_SUC] >>
+GEN_TAC >> STRIP_TAC >>
+`bs <> []` by (
+  REPEAT STRIP_TAC >>
+  FULL_SIMP_TAC list_ss []
+) >>
+ASM_SIMP_TAC list_ss [bitstring_split_REWRS]);
+
+
+val bitstring_split_LENGTHS_MODDIV = store_thm ("bitstring_split_LENGTHS_MODDIV",
+  ``!n bs. n <> 0 /\ (LENGTH bs MOD n = 0) ==> (
+      (EVERY (\l. LENGTH l = n) (bitstring_split n bs)) /\
+      (LENGTH (bitstring_split n bs) = LENGTH bs DIV n))``,
+
+REPEAT STRIP_TAC >>
+`0 < n` by DECIDE_TAC >>
+`?m. LENGTH bs = m * n `by METIS_TAC[arithmeticTheory.MOD_EQ_0_DIVISOR] >>
+ASM_SIMP_TAC std_ss [arithmeticTheory.MULT_DIV] >>
+METIS_TAC [bitstring_split_LENGTHS]);
+
+
+val bitstring_split_LENGTHS_b2v = store_thm ("bitstring_split_LENGTHS_b2v",
+  ``!n v vty. (bir_number_of_mem_splits vty (type_of_bir_imm v) = SOME n) ==>
+      (EVERY (\l. LENGTH l = (size_of_bir_immtype vty)) (bitstring_split (size_of_bir_immtype vty) (b2v v)) /\
+      (LENGTH (bitstring_split (size_of_bir_immtype vty) (b2v v)) = n))``,
+
+SIMP_TAC std_ss [bir_number_of_mem_splits_def] >>
+METIS_TAC[bitstring_split_LENGTHS_MODDIV, size_of_bir_immtype_NEQ_0,
+  b2v_LENGTH]);
+
+val bitstring_split_SINGLE = store_thm ("bitstring_split_SINGLE",
+  ``!n bs. n <> 0 ==>
+      (LENGTH bs = n) ==>
+      (bitstring_split n bs = [bs])``,
+
+REPEAT STRIP_TAC >>
+`bs <> []` by (Cases_on `bs` >> FULL_SIMP_TAC list_ss []) >>
+ASM_SIMP_TAC list_ss [bitstring_split_REWRS, listTheory.TAKE_LENGTH_TOO_LONG,
+  listTheory.DROP_LENGTH_TOO_LONG]);
+
+
+val bir_mem_concat_bitstring_split = store_thm ("bir_mem_concat_bitstring_split",
+``!v n rty.
+      (n <> 0) ==>
+      (bir_mem_concat (bitstring_split n (b2v v)) rty = n2bs (b2n v) rty)``,
+
+SIMP_TAC std_ss [bir_mem_concat_def, bitstring_split_FLAT, v2bs_def, v2n_b2v, n2bs_def]);
+
+
+val bitstring_split_num_REWRS = save_thm ("bitstring_split_num_REWRS",
+let
+  val words_sizes = [1,8,16,32,64];
+
+  val combined_sizes = flatten (map (fn sz1 => map (fn sz2 => (sz1, sz2)) words_sizes) words_sizes)
+  val combined_sizes = filter (fn (sz1, sz2) => (sz1 <= sz2) andalso (sz2 mod sz1 = 0)) combined_sizes
+
+  fun mk_sizes_thm (sz1, sz2) = let
+    val sz1_tm = numSyntax.term_of_int sz1
+    val sz2_tm = numSyntax.term_of_int sz2
+    val l_tm = ``l:'a list``
+    val pre = ``LENGTH ^l_tm = ^sz2_tm``
+    val t = ``bitstring_split ^sz1_tm ^l_tm``
+
+    val thm0 = SIMP_CONV list_ss [b2v_def, bitstring_split_REWRS_LENGTH,
+       listTheory.TAKE_LENGTH_TOO_LONG,
+       listTheory.DROP_LENGTH_TOO_LONG, rich_listTheory.DROP_DROP_T,
+       ASSUME pre] t
+    val thm1 = GEN l_tm (DISCH pre thm0)
+  in thm1 end
+
+  val thm0 = LIST_CONJ (map mk_sizes_thm combined_sizes)
+in
+  thm0
+end);
+
+
+(* ================= *)
+(* update_mmap       *)
+(* ================= *)
+
+val bir_update_mmap_def = Define `
+    (!mmap a. (bir_update_mmap mmap a [] = mmap)) /\
+    (!mmap a v vs. (bir_update_mmap mmap a (v::vs) =
+                    bir_update_mmap ((a =+ v2n v) mmap) (SUC a) vs))`;
+
+
+val bir_update_mmap_ALT_DEF = store_thm ("bir_update_mmap_ALT_DEF",
+  ``!mmap a vs a'. (bir_update_mmap mmap a vs) a' =
+      (if (a <= a' /\ a' < a + LENGTH vs) then v2n (EL (a' - a) vs) else mmap a')``,
+
+Induct_on `vs` >> (
+  ASM_SIMP_TAC list_ss [bir_update_mmap_def]
+) >>
+REPEAT GEN_TAC >>
+Cases_on `~(a' < (LENGTH vs) + SUC a) \/ ~(a <= a')` >- (
+  ASM_SIMP_TAC arith_ss [combinTheory.APPLY_UPDATE_THM]
+) >>
+FULL_SIMP_TAC arith_ss [] >>
+Cases_on `SUC a <= a'` >- (
+  `a' - a = SUC (a' - SUC a)` by DECIDE_TAC >>
+  ASM_SIMP_TAC list_ss []
+) >>
+`a' = a` by DECIDE_TAC >>
+ASM_SIMP_TAC list_ss [combinTheory.APPLY_UPDATE_THM]);
+
+
+
+(* ================= *)
+(* bir_store_in_mmap *)
+(* ================= *)
+
+val bir_store_in_mem_def = Define `bir_store_in_mem
+  (value_ty : bir_immtype_t) (result : bir_imm_t) (mmap : num -> num) (en: bir_endian_t) (a:num) =
+
+   let result_ty = type_of_bir_imm result in
+   case (bir_number_of_mem_splits value_ty result_ty) of
+    | NONE => NONE
+    | SOME (n:num) => (
+        let vs = bitstring_split (size_of_bir_immtype value_ty) (b2v result) in
+        let vs' = (case en of BEnd_LittleEndian => SOME (REVERSE vs)
+                          |  BEnd_BigEndian => SOME vs
+                          |  BEnd_NoEndian => if (n = 1) then SOME vs else NONE) in
+
+        case vs' of NONE => NONE
+                 |  SOME vs'' => SOME (bir_update_mmap mmap a vs'')
+   )`;
+
+
+val bir_store_in_mem_SINGLE = store_thm ("bir_store_in_mem_SINGLE",
+  ``!en a vty mmap v.
+     (type_of_bir_imm v = vty) ==>
+     (bir_store_in_mem vty v mmap en a = SOME ((a =+ b2n v) mmap))``,
+
+Cases_on `en` >> (
+  SIMP_TAC (list_ss++bir_endian_ss) [bir_store_in_mem_def, bir_number_of_mem_splits_ID, LET_DEF,
+    bitstring_split_SINGLE, b2v_LENGTH, size_of_bir_immtype_NEQ_0, v2n_b2v,
+    bir_update_mmap_def]
+));
+
+
+val bir_store_in_mem_NO_ENDIAN = store_thm ("bir_store_in_mem_NO_ENDIAN",
+  ``!a vty v mmap. bir_store_in_mem vty v mmap BEnd_NoEndian a =
+    (if vty = (type_of_bir_imm v) then
+      SOME ((a =+ b2n v) mmap)
+     else NONE)``,
+
+REPEAT GEN_TAC >>
+Cases_on `vty = type_of_bir_imm v` >> (
+  ASM_SIMP_TAC std_ss [bir_store_in_mem_SINGLE]
+) >>
+`bir_number_of_mem_splits vty (type_of_bir_imm v) <> SOME 1` by (
+  Cases_on `vty` >> Cases_on `v` >>
+  FULL_SIMP_TAC std_ss [bir_number_of_mem_splits_REWRS, type_of_bir_imm_def]
+) >>
+Cases_on `bir_number_of_mem_splits vty (type_of_bir_imm v)` >> (
+  FULL_SIMP_TAC (std_ss++bir_endian_ss) [bir_store_in_mem_def, LET_DEF]
+));
+
+
+val bir_store_in_mem_EQ_NONE = store_thm ("bir_store_in_mem_EQ_NONE",
+  ``!a en vty v mmap. (bir_store_in_mem vty v mmap en a = NONE) <=>
+      ((bir_number_of_mem_splits vty (type_of_bir_imm v) = NONE) \/
+      ((vty <> (type_of_bir_imm v)) /\ (en = BEnd_NoEndian)))``,
+
+REPEAT GEN_TAC >>
+REWRITE_TAC[GSYM bir_number_of_mem_splits_EQ_SOME1] >>
+Cases_on `bir_number_of_mem_splits vty (type_of_bir_imm v)` >> (
+  ASM_SIMP_TAC std_ss [bir_store_in_mem_def, LET_DEF]
+) >>
+Cases_on `en` >> (
+  ASM_SIMP_TAC (std_ss++bir_endian_ss) []
+) >>
+Cases_on `x=1` >> ASM_SIMP_TAC std_ss []);
+
+
+val bir_store_in_mem_EQ_NONE_IMP = store_thm ("bir_store_in_mem_EQ_NONE_IMP",
+  ``!a en vty v mmap. 
+      ((bir_number_of_mem_splits vty (type_of_bir_imm v) = NONE) \/
+       ((vty <> (type_of_bir_imm v)) /\ (en = BEnd_NoEndian))) ==>
+      (bir_store_in_mem vty v mmap en a = NONE)``,
+METIS_TAC[bir_store_in_mem_EQ_NONE]);
+
+
+val bir_store_in_mem_EQ_SOME = store_thm ("bir_store_in_mem_EQ_SOME",
+  ``!a en vty v mmap res. (bir_store_in_mem vty v mmap en a = SOME res) <=>
+      (?n vs vs'. (bir_number_of_mem_splits vty (type_of_bir_imm v) = SOME n) /\
+                  (vs = (bitstring_split (size_of_bir_immtype vty) (b2v v))) /\
+                  ((en = BEnd_BigEndian) /\ (vs' = vs) \/
+                   (en = BEnd_LittleEndian) /\ (vs' = REVERSE vs) \/
+                   (en = BEnd_NoEndian) /\ (n = 1) /\ (vs' = vs)) /\
+                   (res = bir_update_mmap mmap a vs'))``,
+
+REPEAT GEN_TAC >>
+Cases_on `bir_number_of_mem_splits vty (type_of_bir_imm v)` >> (
+  ASM_SIMP_TAC std_ss [bir_store_in_mem_def, LET_DEF]
+) >>
+Cases_on `en` >> (
+  ASM_SIMP_TAC (std_ss++bir_endian_ss++boolSimps.EQUIV_EXTRACT_ss) []
+) >>
+Cases_on `x=1` >>
+ASM_SIMP_TAC (std_ss++boolSimps.EQUIV_EXTRACT_ss) []);
+
+
+
+val bir_store_in_mem_NONE_REWRS = save_thm ("bir_store_in_mem_NONE_REWRS",
+let
+  val thm0 = bir_store_in_mem_EQ_NONE_IMP
+
+  val thm1 = SIMP_RULE (list_ss++bir_imm_ss++DatatypeSimps.expand_type_quants_ss [``:bir_immtype_t``,
+    ``:bir_imm_t``]) [type_of_bir_imm_def,
+    bir_number_of_mem_splits_REWRS] thm0
+
+  val thm2 = SIMP_RULE list_ss [GSYM CONJ_ASSOC, FORALL_AND_THM] thm1
+in
+  thm2
+end);
+
+
+val bir_store_in_mem_REWRS = save_thm ("bir_store_in_mem_REWRS",
+let
+  val thm0 = bir_store_in_mem_def
+
+  val thm1 = SIMP_RULE (list_ss++DatatypeSimps.expand_type_quants_ss [``:bir_immtype_t``,
+    ``:bir_imm_t``]) [
+    bir_number_of_mem_splits_REWRS, type_of_bir_imm_def, bir_number_of_mem_splits_REWRS, LET_DEF,
+      size_of_bir_immtype_def] thm0
+
+  val thm2 = SIMP_RULE (list_ss++wordsLib.SIZES_ss) [b2v_def, bitstring_split_num_REWRS,
+     bitstringTheory.length_w2v] thm1
+  val thm3 = SIMP_RULE (list_ss++bir_endian_ss++(DatatypeSimps.expand_type_quants_ss [``:bir_endian_t``])) [LET_DEF] thm2
+
+  val thm4 = Ho_Rewrite.REWRITE_RULE [fold_bir_endian_THM] thm3
+
+  val thm5 = SIMP_RULE list_ss [GSYM CONJ_ASSOC, FORALL_AND_THM] thm4
+
+in thm5
+end);
+
+
+val bir_store_in_mem_used_addrs_def = Define `
+  bir_store_in_mem_used_addrs vty v en a =
+  bir_load_from_mem_used_addrs vty (type_of_bir_imm v) en a`;
+
+
+val bir_store_in_mem_used_addrs_THM = store_thm ("bir_store_in_mem_used_addrs_THM",
+  ``!a en vty v mmap mmap'.
+       (bir_store_in_mem vty v mmap en a = SOME mmap') ==>
+       (!addr. ~(addr IN bir_store_in_mem_used_addrs vty v en a) ==>
+               (mmap' addr = mmap addr))``,
+
+SIMP_TAC std_ss [bir_store_in_mem_used_addrs_def, bir_load_from_mem_used_addrs_def,
+  bir_store_in_mem_EQ_SOME, GSYM LEFT_FORALL_IMP_THM] >>
+REPEAT GEN_TAC >>
+
+`!addr. ((!n'. addr <> a + n' \/ ~(n' < n)) <=>
+ (~(a <= addr /\ addr < a + n)))` suffices_by (
+  STRIP_TAC >> STRIP_TAC >> (
+    MP_TAC (Q.SPECL [`n`, `v`, `vty`] bitstring_split_LENGTHS_b2v) >>
+    FULL_SIMP_TAC (list_ss++bir_endian_ss) [bir_update_mmap_ALT_DEF,
+      listTheory.MEM_MAP, rich_listTheory.MEM_COUNT_LIST]
+  )
+) >>
+
+REPEAT STRIP_TAC >> EQ_TAC >> REPEAT STRIP_TAC >| [
+  Q.PAT_X_ASSUM `!n'. _ ` (MP_TAC o Q.SPEC `addr - a`) >>
+  ASM_SIMP_TAC arith_ss [],
+
+  Cases_on `addr = a + n'` >>
+  FULL_SIMP_TAC std_ss []
+]);
+
+
+val bir_store_in_mem_used_addrs_REWRS = save_thm ("bir_store_in_mem_used_addrs_REWRS",
+let
+  val thm0 = bir_store_in_mem_used_addrs_def
+
+  val thm1 = SIMP_RULE (list_ss++DatatypeSimps.expand_type_quants_ss [``:bir_immtype_t``,
+     ``:bir_imm_t``]) [
+     bir_load_from_mem_used_addrs_REWRS, type_of_bir_imm_def] thm0
+in thm1
+end);
+
+val bir_store_in_mem_used_addrs_FINITE = store_thm ("bir_store_in_mem_used_addrs_FINITE",
+  ``!tv v en a.
+      FINITE (bir_store_in_mem_used_addrs tv v en a)``,
+SIMP_TAC std_ss [bir_store_in_mem_used_addrs_def, bir_load_from_mem_used_addrs_FINITE])
+
+
+val bir_store_in_mem_used_addrs_EMPTY = store_thm ("bir_store_in_mem_used_addrs_EMPTY",
+  ``!mmap tv v en a.
+      (bir_store_in_mem_used_addrs tv v en a = {}) <=>
+      (bir_store_in_mem tv v mmap en a = NONE)``,
+
+REPEAT GEN_TAC >>
+SIMP_TAC std_ss [bir_store_in_mem_used_addrs_def, bir_store_in_mem_EQ_NONE,
+  bir_load_from_mem_used_addrs_def, GSYM bir_number_of_mem_splits_EQ_SOME1] >>
+Cases_on `bir_number_of_mem_splits tv (type_of_bir_imm v)` >> ASM_SIMP_TAC std_ss [] >>
+COND_CASES_TAC >> ASM_SIMP_TAC std_ss [] >>
+POP_ASSUM (K ALL_TAC) >>
+Cases_on `x` >- (
+  FULL_SIMP_TAC std_ss [bir_number_of_mem_splits_NEQ_SOME0]
+) >>
+SIMP_TAC list_ss [rich_listTheory.COUNT_LIST_def]);
+
+
+val bir_store_in_mem_used_addrs_NoEndian = store_thm ("bir_store_in_mem_used_addrs_NoEndian",
+  ``!tv v a.
+      (bir_store_in_mem_used_addrs tv v BEnd_NoEndian a = {}) \/
+      (bir_store_in_mem_used_addrs tv v BEnd_NoEndian a = {a})``,
+
+SIMP_TAC std_ss [bir_store_in_mem_used_addrs_def] >>
+METIS_TAC[bir_load_from_mem_used_addrs_NoEndian]);
+
+
+
+(* ------------------------------------------------------------------------- *)
+(*  Loading and storing fit                                                  *)
+(* ------------------------------------------------------------------------- *)
+
+val bir_load_bitstring_from_updated_mmap = store_thm ("bir_load_bitstring_from_updated_mmap",
+  ``!vty vs n mmap a. (LENGTH vs = n) /\
+      (!v. MEM v vs ==> (LENGTH v = (size_of_bir_immtype vty))) ==>
+   (MAP (\n.
+    bir_load_bitstring_from_mmap vty
+             (bir_update_mmap mmap a vs)
+             (a + n)) (COUNT_LIST n) = vs)``,
+GEN_TAC >>
+Induct_on `vs` >- (
+  SIMP_TAC list_ss [rich_listTheory.COUNT_LIST_def]
+) >>
+CONV_TAC (RENAME_VARS_CONV ["v"]) >>
+SIMP_TAC std_ss [listTheory.LENGTH, rich_listTheory.COUNT_LIST_def] >>
+SIMP_TAC list_ss [listTheory.MAP_MAP_o, combinTheory.o_DEF, bir_update_mmap_def,
+  DISJ_IMP_THM, FORALL_AND_THM] >>
+REPEAT STRIP_TAC >- (
+  ASM_SIMP_TAC arith_ss [bir_load_bitstring_from_mmap_def, bir_update_mmap_ALT_DEF,
+    combinTheory.APPLY_UPDATE_THM, n2v_v2n]
+) >>
+Q.PAT_X_ASSUM `!n. _` (MP_TAC o Q.SPECL [`LENGTH (vs:bitstring list)`, ` ((a =+ v2n v) mmap)`,
+  `SUC a`]) >>
+ASM_SIMP_TAC std_ss [arithmeticTheory.ADD_CLAUSES]);
+
+
+
+val bir_store_load_mem_THM = store_thm ("bir_store_load_mem_THM",
+  ``!a en vty v mmap mmap'. (bir_store_in_mem vty v mmap en a = SOME mmap') ==>
+       (bir_load_from_mem vty (type_of_bir_imm v) mmap' en a = SOME v)``,
+
+SIMP_TAC (pure_ss) [bir_store_in_mem_EQ_SOME, GSYM LEFT_FORALL_IMP_THM,
+  bir_load_from_mem_EQ_SOME] >>
+REPEAT GEN_TAC >>
+Q.MATCH_ABBREV_TAC `(_ /\ _ /\ en_COND /\ _) ==> _` >>
+REPEAT STRIP_TAC >>
+Q.EXISTS_TAC `n` >> Q.EXISTS_TAC `vs'` >>
+Tactical.REVERSE (Q.SUBGOAL_THEN `MAP (\n. bir_load_bitstring_from_mmap vty mmap' (a + n))
+     (COUNT_LIST n) = vs'` SUBST1_TAC) >- (
+  UNABBREV_ALL_TAC >> (
+    FULL_SIMP_TAC (list_ss++bir_endian_ss) [bir_mem_concat_bitstring_split,
+      size_of_bir_immtype_NEQ_0, n2bs_b2n]
+  )
+) >>
+
+ASM_SIMP_TAC std_ss [] >>
+MATCH_MP_TAC bir_load_bitstring_from_updated_mmap >>
+`(EVERY (\v. (LENGTH v = size_of_bir_immtype vty)) vs) /\
+ (LENGTH vs = n)` suffices_by (
+    UNABBREV_ALL_TAC >> FULL_SIMP_TAC list_ss [listTheory.EVERY_MEM]
+) >>
+ASM_SIMP_TAC std_ss [bitstring_split_LENGTHS_b2v]);
+
+
+val bir_store_load_mem_disjoint_THM = store_thm ("bir_store_load_mem_disjoint_THM",
+  ``!a en vty v mmap mmap' a' en' vty' rty'.
+       (DISJOINT (bir_store_in_mem_used_addrs vty v en a)
+                 (bir_load_from_mem_used_addrs vty' rty' en' a')) ==>
+       (bir_store_in_mem vty v mmap en a = SOME mmap') ==>
+       (bir_load_from_mem vty' rty' mmap' en' a' =
+        bir_load_from_mem vty' rty' mmap en' a')``,
+
+REPEAT STRIP_TAC >>
+MATCH_MP_TAC (bir_load_from_mem_used_addrs_THM) >>
+REPEAT STRIP_TAC >>
+`~(addr IN (bir_store_in_mem_used_addrs vty v en a))` by (
+  FULL_SIMP_TAC std_ss [pred_setTheory.IN_DISJOINT] >>
+  METIS_TAC[]
+) >>
+METIS_TAC[bir_store_in_mem_used_addrs_THM]);
+
+
+val _ = export_theory();
