bir_programScript.sml
@@ -1,0 +1,1487 @@
+open HolKernel Parse boolLib bossLib;
+open wordsTheory bitstringTheory;
+open bir_auxiliaryTheory bir_immTheory bir_valuesTheory;
+open bir_imm_expTheory bir_mem_expTheory bir_envTheory;
+open bir_expTheory;
+open wordsLib;
+
+val _ = new_theory "bir_program";
+
+
+(* ------------------------------------------------------------------------- *)
+(* Datatypes                                                                 *)
+(* ------------------------------------------------------------------------- *)
+
+val _ = Datatype `bir_label_t =
+    BL_Label string
+  | BL_Address bir_imm_t
+`;
+
+val _ = Datatype `bir_stmt_t =
+  | BStmt_Declare bir_var_t
+  | BStmt_Assign  bir_var_t bir_exp_t
+  | BStmt_Jmp     bir_label_t
+  | BStmt_CJmp    bir_exp_t bir_label_t bir_label_t
+  | BStmt_Halt    bir_exp_t
+  | BStmt_Assert  bir_exp_t
+  | BStmt_Assume  bir_exp_t
+`;
+
+val _ = Datatype `bir_block_t = <| bb_label:bir_label_t ; bb_statements:bir_stmt_t list |>`;
+val _ = Datatype `bir_program_t = BirProgram (bir_block_t list)`;
+val _ = Datatype `bir_programcounter_t = <| bpc_label:bir_label_t; bpc_index:num |>`;
+
+val bir_pc_ss = rewrites (type_rws ``:bir_programcounter_t``);
+
+val _ = Datatype `bir_termcode_t =
+    BTC_Running
+  | BTC_Halted bir_val_t
+  | BTC_ReachedEnd
+  | BTC_ReachedUnknownLabel bir_label_t
+  | BTC_Failed
+  | BTC_AssumptionViolated`
+
+val _ = Datatype `bir_state_t = <|
+  bst_pc       : bir_programcounter_t;
+  bst_environ  : bir_var_environment_t;
+  bst_termcode : bir_termcode_t;
+  bst_debug    : string list;
+  bst_execs    : num
+|>`;
+
+val bir_state_ss = rewrites (type_rws ``:bir_state_t``);
+val bir_termcode_ss = rewrites (type_rws ``:bir_termcode_t``);
+
+
+(* ------------------------------------------------------------------------- *)
+(* Programs                                                                  *)
+(* ------------------------------------------------------------------------- *)
+
+val bir_block_stmts_count_def = Define `bir_block_stmts_count bl = LENGTH bl.bb_statements`;
+val bir_program_stmts_count_def = Define`bir_program_stmts_count (BirProgram p) = SUM (MAP bir_block_stmts_count p)`;
+
+val bir_labels_of_program_def = Define `bir_labels_of_program (BirProgram p) =
+  MAP (\bl. bl.bb_label) p`;
+
+val bir_is_valid_labels_def = Define `bir_is_valid_labels p =
+  ALL_DISTINCT (bir_labels_of_program p) /\ ~(MEM (BL_Label "") (bir_labels_of_program p))`;
+
+val bir_is_valid_program_def = Define `bir_is_valid_program p <=>
+   (bir_is_valid_labels p /\ bir_program_stmts_count p > 0)`;
+
+
+val bir_is_valid_labels_blocks_EQ_EL = store_thm ("bir_is_valid_labels_blocks_EQ_EL",
+  ``!p n1 n2. (bir_is_valid_labels (BirProgram p) /\ n1 < LENGTH p /\ n2 < LENGTH p /\
+                ((EL n1 p).bb_label = (EL n2 p).bb_label)) ==> (n1 = n2)``,
+
+SIMP_TAC list_ss [bir_is_valid_labels_def, bir_labels_of_program_def] >>
+REPEAT STRIP_TAC >>
+MP_TAC (Q.ISPEC `MAP (\bl. bl.bb_label) (p:bir_block_t list)` listTheory.EL_ALL_DISTINCT_EL_EQ) >>
+ASM_SIMP_TAC list_ss [GSYM LEFT_EXISTS_IMP_THM] >>
+Q.EXISTS_TAC `n1` >> Q.EXISTS_TAC `n2` >>
+ASM_SIMP_TAC list_ss [listTheory.EL_MAP]);
+
+
+val bir_is_valid_labels_blocks_EQ = store_thm ("bir_is_valid_labels_blocks_EQ",
+  ``!p bl1 bl2. (bir_is_valid_labels (BirProgram p) /\ MEM bl1 p /\ MEM bl2 p /\
+                (bl1.bb_label = bl2.bb_label)) ==> (bl1 = bl2)``,
+
+METIS_TAC [listTheory.MEM_EL, bir_is_valid_labels_blocks_EQ_EL]);
+
+
+
+val bir_get_program_block_info_by_label_def = Define `bir_get_program_block_info_by_label
+  (BirProgram p) l = INDEX_FIND 0 (\(x:bir_block_t). x.bb_label = l) p
+`;
+
+val bir_get_program_block_info_by_label_THM = store_thm ("bir_get_program_block_info_by_label_THM",
+  ``(!p l. ((bir_get_program_block_info_by_label (BirProgram p) l = NONE) <=> (!bl. MEM bl p ==> (bl.bb_label <> l)))) /\
+
+    (!p l i bl.
+          (bir_get_program_block_info_by_label (BirProgram p) l = SOME (i, bl)) <=>
+          ((((i:num) < LENGTH p) /\ (EL i p = bl) /\ (bl.bb_label = l) /\
+             (!j'. j' < i ==> (EL j' p).bb_label <> l))))``,
+
+SIMP_TAC list_ss [bir_get_program_block_info_by_label_def, INDEX_FIND_EQ_NONE,
+  listTheory.EVERY_MEM, INDEX_FIND_EQ_SOME_0]);
+
+
+val bir_get_program_block_info_by_label_valid_THM = store_thm ("bir_get_program_block_info_by_label_valid_THM",
+  ``(!p l. ((bir_get_program_block_info_by_label (BirProgram p) l = NONE) <=> (!bl. MEM bl p ==> (bl.bb_label <> l)))) /\
+
+    (!p l i bl. bir_is_valid_labels (BirProgram p) ==>
+          ((bir_get_program_block_info_by_label (BirProgram p) l = SOME (i, bl)) <=>
+           ((i:num) < LENGTH p) /\ (EL i p = bl) /\ (bl.bb_label = l)))``,
+
+SIMP_TAC (list_ss++boolSimps.EQUIV_EXTRACT_ss) [bir_get_program_block_info_by_label_def,
+  INDEX_FIND_EQ_NONE, listTheory.EVERY_MEM, INDEX_FIND_EQ_SOME_0] >>
+REPEAT STRIP_TAC >>
+`j' < LENGTH p` by DECIDE_TAC >>
+`j' = i` by METIS_TAC[bir_is_valid_labels_blocks_EQ_EL] >>
+FULL_SIMP_TAC arith_ss []);
+
+
+
+val bir_get_program_block_info_by_label_MEM = store_thm ("bir_get_program_block_info_by_label_MEM",
+  ``!p l. MEM l (bir_labels_of_program p) <=>
+          (?i bl. bir_get_program_block_info_by_label p l = SOME (i, bl))``,
+
+Cases_on `p` >> rename1 `BirProgram p` >>
+REPEAT STRIP_TAC >>
+FULL_SIMP_TAC std_ss [bir_labels_of_program_def, listTheory.MEM_MAP] >>
+Cases_on `bir_get_program_block_info_by_label (BirProgram p) l` >| [
+  FULL_SIMP_TAC std_ss [bir_get_program_block_info_by_label_THM] >>
+  METIS_TAC[],
+
+  rename1 `_ = SOME ibl` >>
+  Cases_on `ibl` >>
+  FULL_SIMP_TAC std_ss [bir_get_program_block_info_by_label_THM, listTheory.MEM_EL,
+    GSYM RIGHT_EXISTS_AND_THM] >>
+  METIS_TAC[]
+]);
+
+
+
+(* ------------------------------------------------------------------------- *)
+(*  Program Counter                                                          *)
+(* ------------------------------------------------------------------------- *)
+
+val bir_is_valid_pc_def = Define `bir_is_valid_pc p pc =
+   (?i bl. (bir_get_program_block_info_by_label p (pc.bpc_label) = SOME (i, bl)) /\
+           (pc.bpc_index < LENGTH bl.bb_statements))`;
+
+val bir_is_end_pc_def = Define `bir_is_end_pc (BirProgram p) pc =
+   (?i bl. (bir_get_program_block_info_by_label (BirProgram p) (pc.bpc_label) = SOME (i, bl)) /\
+           (pc.bpc_index = LENGTH bl.bb_statements) /\
+      (!j. (i < j /\ j < LENGTH p) ==> (((EL j p).bb_statements) = [])))`;
+
+val bir_is_allowed_pc_def = Define `bir_is_allowed_pc p pc =
+   (?i bl. (bir_get_program_block_info_by_label p (pc.bpc_label) = SOME (i, bl)) /\
+           (pc.bpc_index <= LENGTH bl.bb_statements))`;
+
+
+val bir_is_valid_pc_not_end = store_thm ("bir_is_valid_pc_not_end",
+  ``!p pc. bir_is_valid_pc p pc ==> ~(bir_is_end_pc p pc)``,
+Cases >> rename1 `BirProgram p` >>
+SIMP_TAC arith_ss [bir_is_valid_pc_def, bir_is_end_pc_def,
+  GSYM LEFT_FORALL_IMP_THM]);
+
+
+val bir_is_valid_pc_of_valid_blocks = store_thm ("bir_is_valid_pc_of_valid_blocks",
+  ``!p pc. bir_is_valid_labels (BirProgram p) ==>
+           (bir_is_valid_pc (BirProgram p) pc <=> (?bl. MEM bl p /\ (pc.bpc_label = bl.bb_label) /\
+             (pc.bpc_index < LENGTH bl.bb_statements)))``,
+SIMP_TAC std_ss [bir_is_valid_pc_def, bir_get_program_block_info_by_label_valid_THM,
+  listTheory.MEM_EL, GSYM LEFT_EXISTS_AND_THM] >>
+METIS_TAC[]);
+
+
+
+val bir_get_program_block_info_by_label_valid_pc = store_thm ("bir_get_program_block_info_by_label_valid_pc",
+  ``!p pc. bir_is_valid_pc p pc ==> IS_SOME (bir_get_program_block_info_by_label p pc.bpc_label)``,
+
+SIMP_TAC std_ss [bir_is_valid_pc_def, GSYM LEFT_FORALL_IMP_THM]);
+
+val bir_get_current_statement_def = Define `bir_get_current_statement p pc =
+  option_CASE (bir_get_program_block_info_by_label p pc.bpc_label) NONE
+     (\ (_, bl). if (pc.bpc_index < LENGTH bl.bb_statements) then SOME (EL (pc.bpc_index) bl.bb_statements) else NONE) `;
+
+
+val bir_get_current_statement_IS_SOME = store_thm ("bir_get_current_statement_IS_SOME",
+  ``!p pc. IS_SOME (bir_get_current_statement p pc) <=> bir_is_valid_pc p pc``,
+
+REPEAT GEN_TAC >>
+Cases_on `bir_get_program_block_info_by_label p pc.bpc_label` >> (
+  ASM_SIMP_TAC std_ss [bir_get_current_statement_def, bir_is_valid_pc_def]
+) >>
+SIMP_TAC (std_ss++QI_ss++pairSimps.gen_beta_ss++boolSimps.LIFT_COND_ss) []);
+
+
+val bir_pc_normalise_def = Define `
+  (bir_pc_normalise (BirProgram p) pc = case bir_get_program_block_info_by_label (BirProgram p) (pc.bpc_label) of
+        SOME (n, bl) => if (pc.bpc_index < LENGTH bl.bb_statements)
+          then SOME pc
+          else (
+            let p' = FILTER (\bl. bl.bb_statements <> []) (DROP (SUC n) p) in
+            case p' of
+              | [] => NONE
+              | (bl'::_) => SOME <| bpc_label := bl'.bb_label ; bpc_index := 0 |>
+            )
+      | _ => NONE
+  )
+`;
+
+
+val bir_pc_next_def = Define `
+  bir_pc_next p pc = bir_pc_normalise p (pc with bpc_index updated_by SUC)`;
+
+
+val bir_pc_normalise_EQ_SOME = store_thm ("bir_pc_normalise_EQ_SOME",
+``!p pc i bl pc'. (bir_get_program_block_info_by_label (BirProgram p) (pc.bpc_label) = SOME (i, bl)) ==>
+             ((bir_pc_normalise (BirProgram p) pc = SOME pc') <=>
+                (if (pc.bpc_index < LENGTH bl.bb_statements) then (pc' = pc) else
+                (?j. (i < j /\ j < LENGTH p /\ ((EL j p).bb_statements <> []) /\
+                     (pc' = <| bpc_label := (EL j p).bb_label; bpc_index := 0 |>) /\
+                     (!j'. (i < j' /\ j' < j) ==> (((EL j' p).bb_statements) = []))))))``,
+
+SIMP_TAC std_ss [bir_pc_normalise_def, pairTheory.pair_case_thm] >>
+REPEAT STRIP_TAC >>
+Cases_on `pc.bpc_index < LENGTH bl.bb_statements` >- (
+  ASM_SIMP_TAC arith_ss [] >> METIS_TAC[]
+) >>
+ASM_SIMP_TAC std_ss [LET_DEF] >>
+Cases_on `FILTER (\bl. bl.bb_statements <> []) (DROP (SUC i) p)` >| [
+  ASM_SIMP_TAC list_ss [LET_DEF] >>
+  CCONTR_TAC >>
+  FULL_SIMP_TAC std_ss [] >>
+  `MEM (EL j p) (DROP (SUC i) p)` by (
+     SIMP_TAC (list_ss++boolSimps.CONJ_ss) [listTheory.MEM_EL, rich_listTheory.EL_DROP] >>
+     Q.EXISTS_TAC `j - SUC i` >>
+     ASM_SIMP_TAC arith_ss []
+  ) >>
+  `~(MEM (EL j p) (FILTER (\bl. bl.bb_statements <> []) (DROP (SUC i) p)))` by
+    ASM_SIMP_TAC list_ss [] >>
+  FULL_SIMP_TAC list_ss [listTheory.MEM_FILTER] >>
+  FULL_SIMP_TAC std_ss [],
+
+
+  rename1 `FILTER _ _ = bl0::bls` >>
+  ASM_SIMP_TAC list_ss [LET_DEF] >>
+  `?p1 p2. (LENGTH p1 = SUC i) /\ (p = p1 ++ p2)` by (
+     Q.EXISTS_TAC `TAKE (SUC i) p` >>
+     Q.EXISTS_TAC `DROP (SUC i) p` >>
+     FULL_SIMP_TAC list_ss [bir_get_program_block_info_by_label_THM]
+  ) >>
+  FULL_SIMP_TAC list_ss [rich_listTheory.DROP_APPEND1, listTheory.DROP_LENGTH_TOO_LONG] >>
+  Q.PAT_X_ASSUM `p = _ ++ _` (K ALL_TAC) >>
+  Q.PAT_X_ASSUM `_ = SOME _` (K ALL_TAC) >>
+  Induct_on `p2` >- ASM_SIMP_TAC list_ss [] >>
+  CONV_TAC (RENAME_VARS_CONV ["bl1"]) >>
+  REPEAT STRIP_TAC >>
+  Cases_on `(bl1.bb_statements) <> []` >> FULL_SIMP_TAC list_ss [] >| [
+    REPEAT (BasicProvers.VAR_EQ_TAC) >>
+    EQ_TAC >> REPEAT STRIP_TAC >> REPEAT BasicProvers.VAR_EQ_TAC >> ASM_SIMP_TAC list_ss [] >| [
+      Q.EXISTS_TAC `SUC i` >>
+      ASM_SIMP_TAC (list_ss++QI_ss) [rich_listTheory.EL_APPEND2],
+
+      Cases_on `j = SUC i` >- ASM_SIMP_TAC list_ss [rich_listTheory.EL_APPEND2] >>
+      Q.PAT_X_ASSUM `!j'. _` (MP_TAC o Q.SPEC `SUC i`) >>
+      ASM_SIMP_TAC list_ss [rich_listTheory.EL_APPEND2]
+    ],
+
+    EQ_TAC >> STRIP_TAC >> REPEAT BasicProvers.VAR_EQ_TAC >| [
+      Q.EXISTS_TAC `SUC j` >>
+      Q.PAT_X_ASSUM `_ <> []` MP_TAC >>
+      Q.PAT_X_ASSUM `!j. _` MP_TAC >>
+      `j - i = SUC (j - SUC i)` by DECIDE_TAC >>
+      ASM_SIMP_TAC list_ss [rich_listTheory.EL_APPEND2] >>
+      REPEAT STRIP_TAC >>
+      Cases_on `j' = SUC i` >- ASM_SIMP_TAC list_ss [] >>
+      Q.PAT_X_ASSUM `!j. _` (MP_TAC o Q.SPEC `PRE j'`) >>
+      `j' - SUC i = SUC (PRE j' - SUC i)` by DECIDE_TAC >>
+      ASM_SIMP_TAC list_ss [],
+
+      Q.EXISTS_TAC `PRE j` >>
+      Q.PAT_X_ASSUM `_ <> []` MP_TAC >>
+      Q.PAT_X_ASSUM `!j. _` MP_TAC >>
+
+      Cases_on `j = SUC i` >- ASM_SIMP_TAC list_ss [rich_listTheory.EL_APPEND2] >>
+      `j - SUC i = SUC (PRE j - SUC i)` by DECIDE_TAC >>
+      ASM_SIMP_TAC list_ss [rich_listTheory.EL_APPEND2] >>
+      REPEAT STRIP_TAC >>
+      Q.PAT_X_ASSUM `!j. _` (MP_TAC o Q.SPEC `SUC j'`) >>
+      `j' - i = SUC (j' - SUC i)` by DECIDE_TAC >>
+      ASM_SIMP_TAC list_ss []
+    ]
+  ]
+]);
+
+
+val bir_pc_normalise_EQ_NONE = store_thm ("bir_pc_normalise_EQ_NONE",
+``!p pc i bl. (bir_get_program_block_info_by_label (BirProgram p) (pc.bpc_label) = SOME (i, bl)) ==>
+             ((bir_pc_normalise (BirProgram p) pc = NONE) <=> (
+                (LENGTH bl.bb_statements <= pc.bpc_index) /\
+                (!j. (i < j /\ j < LENGTH p) ==> (((EL j p).bb_statements) = []))))``,
+
+SIMP_TAC std_ss [bir_pc_normalise_def, pairTheory.pair_case_thm] >>
+REPEAT STRIP_TAC >>
+Cases_on `pc.bpc_index < LENGTH bl.bb_statements` >> (
+  ASM_SIMP_TAC arith_ss []
+) >>
+Cases_on `FILTER (\bl. bl.bb_statements <> []) (DROP (SUC i) p)` >| [
+  ASM_SIMP_TAC list_ss [LET_DEF] >>
+  REPEAT STRIP_TAC >>
+  `MEM (EL j p) (DROP (SUC i) p)` by (
+     SIMP_TAC (list_ss++boolSimps.CONJ_ss) [listTheory.MEM_EL, rich_listTheory.EL_DROP] >>
+     Q.EXISTS_TAC `j - SUC i` >>
+     ASM_SIMP_TAC arith_ss []
+  ) >>
+  `~(MEM (EL j p) (FILTER (\bl. bl.bb_statements <> []) (DROP (SUC i) p)))` by
+    ASM_SIMP_TAC list_ss [] >>
+  FULL_SIMP_TAC list_ss [listTheory.MEM_FILTER] >>
+  FULL_SIMP_TAC std_ss [],
+
+
+  rename1 `FILTER _ _ = bl0::bls` >>
+  ASM_SIMP_TAC list_ss [LET_DEF] >>
+  `MEM bl0 (FILTER (\bl. bl.bb_statements <> []) (DROP (SUC i) p))` by
+    ASM_SIMP_TAC list_ss [] >>
+  POP_ASSUM MP_TAC >>
+  FULL_SIMP_TAC list_ss [listTheory.MEM_FILTER] >>
+  SIMP_TAC (list_ss++boolSimps.CONJ_ss) [listTheory.MEM_EL, rich_listTheory.EL_DROP] >>
+  REPEAT STRIP_TAC >>
+  rename1 `bl0 = EL (n + SUC i) p` >>
+  Q.EXISTS_TAC `n + SUC i` >>
+  FULL_SIMP_TAC list_ss []
+]);
+
+
+val bir_pc_normalise_EQ_NONE_not_is_valid = store_thm ("bir_pc_normalise_EQ_NONE_not_is_valid",
+``!p pc. (bir_pc_normalise p pc = NONE) ==> (
+         ~(bir_is_valid_pc p pc))``,
+
+Cases_on `p` >> rename1 `BirProgram p` >>
+REPEAT STRIP_TAC >>
+FULL_SIMP_TAC std_ss [bir_is_valid_pc_def, bir_pc_normalise_def] >>
+FULL_SIMP_TAC std_ss [pairTheory.pair_case_thm]);
+
+
+val bir_pc_normalise_EQ_NONE_is_end_pc = store_thm ("bir_pc_normalise_EQ_NONE_is_end_pc",
+``!p pc. bir_is_allowed_pc p pc ==>
+         ((bir_pc_normalise p pc = NONE) <=> (
+           bir_is_end_pc p pc))``,
+
+Cases_on `p` >> rename1 `BirProgram p` >>
+SIMP_TAC std_ss [bir_is_allowed_pc_def, GSYM LEFT_FORALL_IMP_THM] >>
+REPEAT STRIP_TAC >>
+MP_TAC (Q.SPECL [`p`, `pc`] bir_pc_normalise_EQ_NONE) >>
+FULL_SIMP_TAC (arith_ss++boolSimps.EQUIV_EXTRACT_ss) [bir_is_end_pc_def]);
+
+
+
+val bir_is_allowed_pc_inc_valid = store_thm ("bir_is_allowed_pc_inc_valid",
+``!p pc. bir_is_valid_pc p pc ==> bir_is_allowed_pc p (pc with bpc_index updated_by SUC)``,
+
+SIMP_TAC (arith_ss++bir_pc_ss) [bir_is_valid_pc_def, bir_is_allowed_pc_def, GSYM LEFT_FORALL_IMP_THM]);
+
+val bir_is_allowed_pc_jmp = store_thm ("bir_is_allowed_pc_jmp",
+``!l p. MEM l (bir_labels_of_program p) ==>
+        bir_is_allowed_pc p <| bpc_label := l; bpc_index := 0 |>``,
+
+SIMP_TAC (std_ss++bir_pc_ss) [bir_is_allowed_pc_def, GSYM bir_get_program_block_info_by_label_MEM]);
+
+
+val bir_pc_normalise_valid = store_thm ("bir_pc_normalise_valid",
+``!p pc pc'. (bir_is_valid_labels p /\ (MEM pc.bpc_label (bir_labels_of_program p)) /\
+              (bir_pc_normalise p pc = SOME pc')) ==>
+             (bir_is_valid_pc p pc')``,
+
+Cases >> rename1 `BirProgram p` >>
+SIMP_TAC list_ss [bir_labels_of_program_def, bir_pc_normalise_EQ_SOME,
+  listTheory.MEM_MAP, GSYM RIGHT_EXISTS_AND_THM] >>
+REPEAT STRIP_TAC >>
+FULL_SIMP_TAC std_ss [listTheory.MEM_EL] >>
+rename1 `bl = EL i p` >>
+`bir_get_program_block_info_by_label (BirProgram p) pc.bpc_label = SOME (i, bl)` by
+  METIS_TAC[bir_get_program_block_info_by_label_valid_THM] >>
+
+MP_TAC (Q.SPECL [`p`, `pc`, `i`, `bl`, `pc'`] bir_pc_normalise_EQ_SOME) >>
+FULL_SIMP_TAC std_ss [bir_is_valid_pc_def] >>
+Cases_on `pc.bpc_index < LENGTH (EL i p).bb_statements` >| [
+  ASM_SIMP_TAC std_ss [] >> METIS_TAC[],
+
+  ASM_SIMP_TAC (std_ss++bir_pc_ss) [bir_get_program_block_info_by_label_valid_THM,
+    GSYM LEFT_FORALL_IMP_THM] >>
+  REPEAT STRIP_TAC >>
+  Q.EXISTS_TAC `j` >>
+  ASM_SIMP_TAC arith_ss [] >>
+  Cases_on `(EL j p).bb_statements` >> FULL_SIMP_TAC list_ss []
+]);
+
+
+val bir_pc_next_valid = store_thm ("bir_pc_next_valid",
+``!p pc pc'. (bir_is_valid_labels p /\ bir_is_valid_pc p pc /\ (bir_pc_next p pc = SOME pc')) ==>
+             (bir_is_valid_pc p pc')``,
+
+REPEAT STRIP_TAC >>
+MATCH_MP_TAC bir_pc_normalise_valid >>
+Q.EXISTS_TAC `pc with bpc_index updated_by SUC` >>
+Cases_on `p` >>
+FULL_SIMP_TAC (std_ss++bir_pc_ss) [bir_pc_next_def, bir_is_valid_pc_def, bir_labels_of_program_def,
+  listTheory.MEM_MAP] >>
+METIS_TAC[listTheory.MEM_EL, bir_get_program_block_info_by_label_valid_THM]);
+
+
+val bir_pc_first_def = Define
+  `bir_pc_first (BirProgram p) = let bl = HD (FILTER (\bl. (bl.bb_statements) <> []) p) in
+    (<| bpc_label := bl.bb_label; bpc_index := 0 |>):bir_programcounter_t`;
+
+val bir_pc_last_def = Define
+  `bir_pc_last (BirProgram p) = let bl = LAST (FILTER (\bl. (bl.bb_statements) <> []) p) in
+    (<| bpc_label := bl.bb_label; bpc_index := LENGTH bl.bb_statements - 1 |>):bir_programcounter_t`;
+
+
+val bir_program_stmts_count_FILTER_NEQ_NIL = store_thm ("bir_program_stmts_count_FILTER_NEQ_NIL",
+  ``!p. (bir_program_stmts_count (BirProgram p) > 0) ==>
+    (?bl0 bls. (FILTER (\bl. bl.bb_statements <> []) p = bl0 :: bls) /\
+              EVERY (\bl. (bl.bb_statements <> []) /\ MEM bl p) (bl0::bls))``,
+
+Induct_on `p` >> (
+  FULL_SIMP_TAC list_ss [bir_program_stmts_count_def, bir_block_stmts_count_def]
+) >>
+CONV_TAC (RENAME_VARS_CONV ["bl"]) >> GEN_TAC >>
+Cases_on `bl.bb_statements` >| [
+  SIMP_TAC list_ss [] >>
+  REPEAT STRIP_TAC >>
+  FULL_SIMP_TAC list_ss [listTheory.EVERY_MEM],
+
+  SIMP_TAC list_ss [listTheory.EVERY_FILTER] >>
+  ASM_SIMP_TAC list_ss [listTheory.EVERY_MEM]
+]);
+
+
+val bir_pc_first_valid = store_thm ("bir_pc_first_valid",
+  ``!p. bir_is_valid_program p ==> bir_is_valid_pc p (bir_pc_first p)``,
+
+Cases >> rename1 `BirProgram p` >>
+SIMP_TAC (std_ss++bir_pc_ss) [bir_is_valid_pc_of_valid_blocks, bir_is_valid_program_def,
+  bir_pc_first_def, LET_DEF] >>
+ASSUME_TAC (Q.SPEC `p` bir_program_stmts_count_FILTER_NEQ_NIL) >>
+REPEAT STRIP_TAC >>
+FULL_SIMP_TAC list_ss [] >>
+rename1 `bl0.bb_statements <> []` >>
+Q.EXISTS_TAC `bl0` >>
+Cases_on `bl0.bb_statements` >> FULL_SIMP_TAC list_ss []);
+
+
+val bir_pc_last_valid = store_thm ("bir_pc_last_valid",
+  ``!p. bir_is_valid_program p ==> bir_is_valid_pc p (bir_pc_last p)``,
+
+Cases >> rename1 `BirProgram p` >>
+SIMP_TAC (std_ss++bir_pc_ss) [bir_is_valid_pc_of_valid_blocks, bir_is_valid_program_def,
+  bir_pc_last_def, LET_DEF] >>
+ASSUME_TAC (Q.SPEC `p` bir_program_stmts_count_FILTER_NEQ_NIL) >>
+REPEAT STRIP_TAC >>
+FULL_SIMP_TAC list_ss [] >>
+rename1 `FILTER _ p = bl0::bls` >>
+Q.EXISTS_TAC `LAST (bl0::bls)` >>
+`MEM (LAST (bl0::bls)) (bl0::bls)` by MATCH_ACCEPT_TAC rich_listTheory.MEM_LAST >>
+ASM_SIMP_TAC arith_ss [rich_listTheory.LENGTH_NOT_NULL, listTheory.NULL_EQ] >>
+FULL_SIMP_TAC list_ss [listTheory.EVERY_MEM]);
+
+
+
+val bir_is_valid_pc_label_OK = store_thm ("bir_is_valid_pc_label_OK",
+  ``!p pc. bir_is_valid_pc p pc ==> MEM pc.bpc_label (bir_labels_of_program p)``,
+
+Cases_on `p` >> rename1 `BirProgram p` >>
+SIMP_TAC std_ss [bir_is_valid_pc_def, listTheory.MEM_MAP,
+  GSYM LEFT_FORALL_IMP_THM, bir_labels_of_program_def,
+  bir_get_program_block_info_by_label_THM] >>
+SIMP_TAC std_ss [listTheory.MEM_EL, GSYM RIGHT_EXISTS_AND_THM] >>
+METIS_TAC[]);
+
+
+val bir_pc_next_valid_EQ_NONE = store_thm ("bir_pc_next_valid_EQ_NONE",
+``!p pc. (bir_is_valid_labels p /\ bir_is_valid_pc p pc) ==>
+          ((bir_pc_next p pc = NONE) <=> (pc = bir_pc_last p))``,
+
+REPEAT STRIP_TAC >>
+ASM_SIMP_TAC std_ss [bir_pc_next_def,
+  bir_pc_normalise_EQ_NONE_is_end_pc, bir_is_allowed_pc_inc_valid] >>
+
+Cases_on `p` >> rename1 `BirProgram p` >>
+ASM_SIMP_TAC (std_ss++bir_pc_ss) [bir_pc_last_def, LET_THM, bir_is_end_pc_def] >>
+
+`FILTER (\bl. bl.bb_statements <> []) p <> []` by (
+  STRIP_TAC  >>
+  FULL_SIMP_TAC std_ss [bir_is_valid_pc_def, bir_get_program_block_info_by_label_THM] >>
+  `MEM (EL i p) (FILTER (\bl. bl.bb_statements <> []) p)` suffices_by ASM_SIMP_TAC list_ss [] >>
+  SIMP_TAC list_ss [listTheory.MEM_FILTER, listTheory.MEM_EL] >>
+  REPEAT STRIP_TAC >| [
+    Cases_on `(EL i p).bb_statements` >> FULL_SIMP_TAC list_ss [],
+    METIS_TAC[]
+  ]
+) >>
+
+IMP_RES_TAC LAST_FILTER_EL >>
+FULL_SIMP_TAC (list_ss++bir_pc_ss) [DB.fetch "-" "bir_programcounter_t_component_equality",
+  bir_is_valid_pc_def] >>
+REV_FULL_SIMP_TAC std_ss [bir_get_program_block_info_by_label_valid_THM] >>
+EQ_TAC >> STRIP_TAC >| [
+  `~(i < i')` by (
+    STRIP_TAC >>
+    `bl.bb_statements = []` by METIS_TAC[] >>
+    FULL_SIMP_TAC list_ss []
+  ) >>
+  `~(i' < i)` by (
+    STRIP_TAC >>
+    `(EL i p).bb_statements = []` by METIS_TAC[] >>
+    FULL_SIMP_TAC list_ss []
+  ) >>
+  `i' = i` by DECIDE_TAC >>
+  FULL_SIMP_TAC arith_ss [],
+
+  `bl = EL i p` by METIS_TAC [bir_is_valid_labels_blocks_EQ, listTheory.MEM_EL] >>
+  `i' = i` by METIS_TAC [bir_is_valid_labels_blocks_EQ_EL] >>
+  FULL_SIMP_TAC arith_ss [] >>
+  REPEAT STRIP_TAC >>
+  `~(LENGTH (EL j p).bb_statements > 0)` by METIS_TAC[] >>
+  ASM_SIMP_TAC arith_ss []
+]);
+
+
+
+
+
+
+(* ------------------------------------------------------------------------- *)
+(* Auxiliary stuff                                                           *)
+(* ------------------------------------------------------------------------- *)
+
+(* This definition is oriented to give an RX name to registers *)
+val r2s_def = Define `r2s = \(w:bool[5]).STRCAT ("R") (w2s (10:num) HEX w)`;
+
+val r2s_REWRS = store_thm ("r2s_REWRS", ``
+  (r2s  0w = "R0" ) /\ (r2s  1w = "R1" ) /\ (r2s  2w = "R2" ) /\ (r2s  3w = "R3" ) /\
+  (r2s  4w = "R4" ) /\ (r2s  5w = "R5" ) /\ (r2s  6w = "R6" ) /\ (r2s  7w = "R7" ) /\
+  (r2s  8w = "R8" ) /\ (r2s  9w = "R9" ) /\ (r2s 10w = "R10") /\ (r2s 11w = "R11") /\
+  (r2s 12w = "R12") /\ (r2s 13w = "R13") /\ (r2s 14w = "R14") /\ (r2s 15w = "R15") /\
+  (r2s 16w = "R16") /\ (r2s 17w = "R17") /\ (r2s 18w = "R18") /\ (r2s 19w = "R19") /\
+  (r2s 20w = "R20") /\ (r2s 21w = "R21") /\ (r2s 22w = "R22") /\ (r2s 23w = "R23") /\
+  (r2s 24w = "R24") /\ (r2s 25w = "R25") /\ (r2s 26w = "R26") /\ (r2s 27w = "R27") /\
+  (r2s 28w = "R28") /\ (r2s 29w = "R29") /\ (r2s 30w = "R30") /\ (r2s 31w = "R31")``,
+EVAL_TAC);
+
+
+(* Statement to string (useful for debugging purposes) *)
+val bir_stmt_to_string_def = Define `bir_stmt_to_string stmt = case stmt of
+  | BStmt_Declare (BVar s _) => CONCAT ["Declaration of "; s]
+  | BStmt_Assign (BVar s _) _ => CONCAT ["Assignment of "; s]
+  | BStmt_Jmp _ => "Jump"
+  | BStmt_CJmp _ _ _ => "Conditional Jump"
+  | BStmt_Halt _ => "Halt"
+  | BStmt_Assert _ => "Assert"
+  | BStmt_Assume _ => "Assume"
+  | _ => "-- unsupported statement"
+`;
+
+
+(* ------------------------------------------------------------------------- *)
+(*  Program State                                                            *)
+(* ------------------------------------------------------------------------- *)
+
+val bir_state_add_execs_def = Define `bir_state_add_execs st n =
+  st with bst_execs updated_by ($+ n)`;
+
+val bir_state_is_terminated_def = Define `bir_state_is_terminated st =
+  (st.bst_termcode <> BTC_Running)`;
+
+val bir_state_is_terminated_IMP = store_thm ("bir_state_is_terminated_IMP",
+  ``(!st. (st.bst_termcode = BTC_Running) ==> ~(bir_state_is_terminated st)) /\
+    (!st. (st.bst_termcode <> BTC_Running) ==> (bir_state_is_terminated st))``,
+  SIMP_TAC std_ss [bir_state_is_terminated_def]);
+
+val bir_state_is_failed_def = Define `bir_state_is_failed st =
+  (st.bst_termcode = BTC_Failed)`;
+
+val bir_state_set_failed_def = Define `bir_state_set_failed st msg =
+  (st with bst_termcode := BTC_Failed) with bst_debug updated_by (\dbg. msg::dbg)`;
+
+val bir_state_set_failed_is_failed = store_thm ("bir_state_set_failed_is_failed",
+  ``!st msg. bir_state_is_failed (bir_state_set_failed st msg)``,
+SIMP_TAC (std_ss ++ bir_state_ss) [bir_state_set_failed_def, bir_state_is_failed_def]);
+
+val bir_state_normalise_pc_def = Define `bir_state_normalise_pc p (st:bir_state_t) =
+  case bir_pc_normalise p st.bst_pc of
+    | SOME pc' => (st with bst_pc := pc')
+    | NONE => (st with bst_termcode := BTC_ReachedEnd)`;
+
+val bir_state_incr_pc_def = Define `bir_state_incr_pc p (st:bir_state_t) =
+  bir_state_normalise_pc p (st with bst_pc := (st.bst_pc with bpc_index updated_by SUC))`
+
+val bir_state_set_pc_def = Define `bir_state_set_pc p (st:bir_state_t) pc' =
+  bir_state_normalise_pc p (st with bst_pc := pc')`;
+
+val bir_state_init_def = Define `bir_state_init p = <|
+    bst_pc       := bir_pc_first p
+  ; bst_environ  := bir_empty_env
+  ; bst_termcode := BTC_Running
+  ; bst_debug    := []
+  ; bst_execs    := 0
+|>`;
+
+
+(* ------------------------------------------------------------------------- *)
+(*  Semantics of statements                                                  *)
+(* ------------------------------------------------------------------------- *)
+
+(* Execution of Jmp, CJmp, Halt, Assert, Assume doesn't change environment *)
+
+val bir_declare_initial_value_def = Define `
+  (bir_declare_initial_value (BType_Imm _) = NONE) /\
+  (bir_declare_initial_value (BType_Mem at vt) = SOME (BVal_Mem at vt (K 0)))`;
+
+val bir_exec_stmt_declare_def = Define `bir_exec_stmt_declare p v ty (st : bir_state_t) =
+   let env = (
+      let vo = bir_declare_initial_value ty in
+      if bir_env_varname_is_bound st.bst_environ v then BEnv_Irregular else
+      bir_env_update v vo ty st.bst_environ) in
+    if (bir_is_regular_env env) then
+       bir_state_incr_pc p (st with bst_environ := env)
+    else
+       bir_state_set_failed st (CONCAT ["irregular environment after "; bir_stmt_to_string
+          (BStmt_Declare (BVar v ty))])`;
+
+val bir_exec_stmt_assign_def = Define `bir_exec_stmt_assign p v ex (st : bir_state_t) =
+   let env = bir_env_write v (bir_eval_exp ex st.bst_environ) st.bst_environ in
+    if (bir_is_regular_env env) then
+       bir_state_incr_pc p (st with bst_environ := env)
+    else
+       bir_state_set_failed st (CONCAT ["irregular environment after "; bir_stmt_to_string
+          (BStmt_Assign v ex)])`;
+
+val bir_exec_stmt_halt_def = Define `bir_exec_stmt_halt ex (st : bir_state_t) =
+    (st with bst_termcode := BTC_Halted (bir_eval_exp ex st.bst_environ))`;
+
+val bir_exec_stmt_jmp_def = Define `bir_exec_stmt_jmp p l (st : bir_state_t) =
+    if (MEM l (bir_labels_of_program p)) then
+      bir_state_set_pc p st <| bpc_label := l; bpc_index := 0 |>
+    else (st with bst_termcode := (BTC_ReachedUnknownLabel l))`;
+
+val bir_exec_stmt_cjmp_def = Define `bir_exec_stmt_cjmp p ex l1 l2 (st : bir_state_t) =
+  case (bir_dest_bool_val (bir_eval_exp ex st.bst_environ)) of
+    | SOME T => bir_exec_stmt_jmp p l1 st
+    | SOME F => bir_exec_stmt_jmp p l2 st
+    | NONE => bir_state_set_failed st "condition of cjmp failed to evaluate"`;
+
+val bir_exec_stmt_assert_def = Define `bir_exec_stmt_assert p ex (st : bir_state_t) =
+  case (bir_dest_bool_val (bir_eval_exp ex st.bst_environ)) of
+    | SOME T => bir_state_incr_pc p st
+    | SOME F => bir_state_set_failed st "assertion failed"
+    | NONE => bir_state_set_failed st "condition of assert failed to evaluate"`
+
+val bir_exec_stmt_assume_def = Define `bir_exec_stmt_assume p ex (st : bir_state_t) =
+  case (bir_dest_bool_val (bir_eval_exp ex st.bst_environ)) of
+    | SOME T => bir_state_incr_pc p st
+    | SOME F => (st with bst_termcode := BTC_AssumptionViolated)
+    | NONE => bir_state_set_failed st "condition of assume failed to evaluate"`;
+
+
+val bir_exec_stmt_def = Define `
+  (bir_exec_stmt p (BStmt_Jmp l) st = bir_exec_stmt_jmp p l st) /\
+  (bir_exec_stmt p (BStmt_CJmp e l1 l2) st = bir_exec_stmt_cjmp p e l1 l2 st) /\
+  (bir_exec_stmt p (BStmt_Declare v) st = bir_exec_stmt_declare p (bir_var_name v) (bir_var_type v) st) /\
+  (bir_exec_stmt p (BStmt_Assert ex) st = bir_exec_stmt_assert p ex st) /\
+  (bir_exec_stmt p (BStmt_Assume ex) st = bir_exec_stmt_assume p ex st) /\
+  (bir_exec_stmt p (BStmt_Assign v ex) st = bir_exec_stmt_assign p v ex st) /\
+  (bir_exec_stmt p (BStmt_Halt ex) st = bir_exec_stmt_halt ex st)`;
+
+
+val bir_exec_step_def = Define `bir_exec_step p state =
+  if (bir_state_is_terminated state) then state else
+  case (bir_get_current_statement p state.bst_pc) of
+    | NONE => bir_state_set_failed state "invalid program_counter"
+    | SOME stm => (bir_exec_stmt p stm state) with bst_execs updated_by SUC
+`;
+
+
+(* ------------------------------------------------------------------------- *)
+(*  Semantics preserve validity of states                                    *)
+(* ------------------------------------------------------------------------- *)
+
+val bir_is_valid_state_def = Define `bir_is_valid_state p st <=>
+  ((bir_is_well_typed_env st.bst_environ) /\ (if st.bst_termcode = BTC_ReachedEnd then bir_is_end_pc p st.bst_pc else
+      bir_is_valid_pc p st.bst_pc))`;
+
+val bir_state_init_valid = store_thm ("bir_state_init_valid",
+  ``!p. bir_is_valid_program p ==> bir_is_valid_state p (bir_state_init p)``,
+
+SIMP_TAC (std_ss++bir_state_ss++bir_termcode_ss) [bir_is_valid_state_def, bir_state_init_def,
+  bir_pc_first_valid, bir_is_well_typed_env_empty]);
+
+
+val bir_is_valid_state_exec_ignore = store_thm ("bir_is_valid_state_exec_ignore",
+  ``!p st f. bir_is_valid_state p (st with bst_execs updated_by f) =
+             bir_is_valid_state p st``,
+SIMP_TAC (std_ss++bir_state_ss) [bir_is_valid_state_def]);
+
+
+val bir_exec_step_valid_THM = store_thm ("bir_exec_step_valid_THM",
+ ``!p st. bir_is_valid_state p st ==>
+          (if bir_state_is_terminated st then
+             (bir_exec_step p st = st)
+           else
+             (bir_is_valid_pc p st.bst_pc) /\
+             (?stmt. (bir_get_current_statement p st.bst_pc = SOME stmt) /\
+                     (bir_exec_step p st = (bir_exec_stmt p stmt st with bst_execs updated_by SUC))))``,
+
+REPEAT STRIP_TAC >>
+SIMP_TAC std_ss [bir_exec_step_def] >>
+Cases_on `bir_state_is_terminated st` >> ASM_SIMP_TAC (std_ss++boolSimps.CONJ_ss) [] >>
+`st.bst_termcode <> BTC_ReachedEnd` by (
+  STRIP_TAC >> FULL_SIMP_TAC (std_ss++bir_termcode_ss) [bir_state_is_terminated_def]
+) >>
+`?stm. bir_get_current_statement p st.bst_pc = SOME stm` by (
+  `IS_SOME (bir_get_current_statement p st.bst_pc)` suffices_by METIS_TAC[optionTheory.IS_SOME_EXISTS] >>
+  FULL_SIMP_TAC std_ss [bir_get_current_statement_IS_SOME,
+     bir_is_valid_state_def]
+) >>
+FULL_SIMP_TAC std_ss [bir_is_valid_state_def]);
+
+
+val bir_is_valid_state_set_failed = store_thm ("bir_is_valid_state_set_failed",
+  ``!p st msg. bir_is_valid_state p st /\ bir_is_valid_pc p st.bst_pc ==>
+               bir_is_valid_state p (bir_state_set_failed st msg)``,
+SIMP_TAC (std_ss++bir_termcode_ss++bir_state_ss) [bir_is_valid_state_def, bir_state_set_failed_def]);
+
+
+val bir_is_valid_state_incr_pc = store_thm ("bir_is_valid_state_incr_pc",
+  ``!p st. bir_is_valid_program p /\ bir_is_valid_state p st /\ bir_is_valid_pc p st.bst_pc ==>
+           bir_is_valid_state p (bir_state_incr_pc p st)``,
+SIMP_TAC (std_ss++bir_state_ss++boolSimps.CONJ_ss) [bir_state_incr_pc_def, bir_is_valid_state_def,
+  bir_state_normalise_pc_def, bir_is_valid_pc_not_end
+] >>
+REPEAT GEN_TAC >> STRIP_TAC >>
+Cases_on `bir_pc_normalise p (st.bst_pc with bpc_index updated_by SUC)` >- (
+  ASM_SIMP_TAC (std_ss++bir_state_ss) [GSYM bir_pc_normalise_EQ_NONE_is_end_pc,
+    bir_is_allowed_pc_inc_valid]
+) >>
+rename1 `_ = SOME pc'` >>
+ASM_SIMP_TAC (std_ss++bir_pc_ss++bir_state_ss) [] >>
+MATCH_MP_TAC bir_pc_normalise_valid >>
+Q.EXISTS_TAC `st.bst_pc with bpc_index updated_by SUC` >>
+FULL_SIMP_TAC (std_ss++bir_pc_ss) [bir_is_valid_pc_label_OK,
+   bir_is_valid_program_def]);
+
+
+
+val bir_exec_step_valid_state_invar_declare = prove (
+  ``!p st v. (bir_is_valid_program p /\ bir_is_valid_state p st /\ bir_is_valid_pc p st.bst_pc) ==>
+             bir_is_valid_state p (bir_exec_stmt p (BStmt_Declare v) st)``,
+Cases_on `v` >> rename1 `BVar v ty` >>
+SIMP_TAC (std_ss++boolSimps.LIFT_COND_ss) [bir_exec_stmt_def, bir_exec_stmt_declare_def, LET_THM,
+  bir_is_valid_state_set_failed, bir_is_regular_env_def, bir_var_type_def, bir_var_name_def] >>
+REPEAT STRIP_TAC >>
+MATCH_MP_TAC bir_is_valid_state_incr_pc >>
+ASM_SIMP_TAC (std_ss++bir_state_ss) [] >>
+FULL_SIMP_TAC (std_ss++bir_state_ss) [bir_is_valid_state_def] >>
+Q.PAT_X_ASSUM `bir_is_regular_env _` MP_TAC >>
+Cases_on `st.bst_environ` >> SIMP_TAC std_ss [bir_env_update_def, bir_is_regular_env_def] >>
+COND_CASES_TAC >- SIMP_TAC std_ss [bir_is_regular_env_def] >>
+FULL_SIMP_TAC (std_ss) [bir_is_regular_env_def, bir_is_well_typed_env_def] >>
+ConseqConv.CONSEQ_REWRITE_TAC ([finite_mapTheory.FEVERY_STRENGTHEN_THM], [], []) >>
+Cases_on `bir_declare_initial_value ty` >> FULL_SIMP_TAC std_ss []);
+
+
+val bir_exec_step_valid_state_invar_assign = prove (
+  ``!p st v ex. (bir_is_valid_program p /\ bir_is_valid_state p st /\ bir_is_valid_pc p st.bst_pc) ==>
+                 bir_is_valid_state p (bir_exec_stmt p (BStmt_Assign v ex) st)``,
+Cases_on `v` >> rename1 `BVar v ty` >>
+SIMP_TAC (std_ss++boolSimps.LIFT_COND_ss) [bir_exec_stmt_def, bir_exec_stmt_assign_def, LET_THM,
+  bir_is_valid_state_set_failed, bir_is_regular_env_def] >>
+REPEAT STRIP_TAC >>
+MATCH_MP_TAC bir_is_valid_state_incr_pc >>
+ASM_SIMP_TAC (std_ss++bir_state_ss) [] >>
+FULL_SIMP_TAC (std_ss++bir_state_ss) [bir_is_valid_state_def] >>
+Q.PAT_X_ASSUM `bir_is_regular_env _` MP_TAC >>
+SIMP_TAC std_ss [bir_env_write_def] >>
+COND_CASES_TAC >> SIMP_TAC std_ss [bir_is_regular_env_def, bir_var_name_def, bir_var_type_def] >>
+Cases_on `st.bst_environ` >> SIMP_TAC std_ss [bir_env_update_def, bir_is_regular_env_def] >>
+COND_CASES_TAC >> SIMP_TAC std_ss [bir_is_regular_env_def, bir_is_well_typed_env_def] >>
+ConseqConv.CONSEQ_REWRITE_TAC ([finite_mapTheory.FEVERY_STRENGTHEN_THM], [], []) >>
+FULL_SIMP_TAC std_ss [bir_is_well_typed_env_def]);
+
+
+val bir_exec_step_valid_state_invar_jmp' = prove (
+  ``!p st l. (bir_is_valid_program p /\ bir_is_valid_state p st /\ bir_is_valid_pc p st.bst_pc) ==>
+             bir_is_valid_state p (bir_exec_stmt_jmp p l st)``,
+SIMP_TAC std_ss [bir_exec_stmt_jmp_def] >>
+REPEAT STRIP_TAC >>
+COND_CASES_TAC >| [
+  ASM_SIMP_TAC (std_ss++bir_state_ss) [bir_is_valid_state_def, bir_state_set_pc_def,
+    bir_state_normalise_pc_def] >>
+  Cases_on `bir_pc_normalise p <|bpc_label := l; bpc_index := 0|>` >| [
+    FULL_SIMP_TAC (std_ss++bir_state_ss) [bir_is_valid_state_def] >>
+    ASM_SIMP_TAC std_ss [GSYM bir_pc_normalise_EQ_NONE_is_end_pc,
+      bir_is_allowed_pc_jmp],
+
+    rename1 `_ = SOME pc'` >>
+    FULL_SIMP_TAC (std_ss++bir_pc_ss++bir_state_ss) [bir_is_valid_state_def,
+      bir_is_valid_pc_not_end] >>
+    MATCH_MP_TAC bir_pc_normalise_valid >>
+    Q.EXISTS_TAC `<| bpc_label := l; bpc_index := 0|>` >>
+    FULL_SIMP_TAC (std_ss++bir_pc_ss) [bir_is_valid_program_def]
+  ],
+
+  FULL_SIMP_TAC (std_ss++bir_state_ss++bir_termcode_ss) [bir_is_valid_state_def]
+]);
+
+val bir_exec_step_valid_state_invar_jmp = prove (
+  ``!p st l. (bir_is_valid_program p /\ bir_is_valid_state p st /\ bir_is_valid_pc p st.bst_pc) ==>
+             bir_is_valid_state p (bir_exec_stmt p (BStmt_Jmp l) st)``,
+SIMP_TAC std_ss [bir_exec_stmt_def, bir_exec_step_valid_state_invar_jmp']);
+
+
+val bir_exec_step_valid_state_invar_cjmp = prove (
+  ``!p st ex l1 l2.
+       (bir_is_valid_program p /\ bir_is_valid_state p st /\ bir_is_valid_pc p st.bst_pc) ==>
+       bir_is_valid_state p (bir_exec_stmt p (BStmt_CJmp ex l1 l2) st)``,
+SIMP_TAC std_ss [bir_exec_stmt_def, bir_exec_stmt_cjmp_def] >>
+REPEAT STRIP_TAC >>
+Cases_on `bir_dest_bool_val (bir_eval_exp ex st.bst_environ)` >- (
+  ASM_SIMP_TAC std_ss [bir_is_valid_state_set_failed]
+) >>
+rename1 `SOME c` >>
+Cases_on `c` >> (
+  ASM_SIMP_TAC std_ss [bir_exec_step_valid_state_invar_jmp']
+));
+
+
+val bir_exec_step_valid_state_invar_halt = prove (
+  ``!p st ex. (bir_is_valid_program p /\ bir_is_valid_state p st /\ bir_is_valid_pc p st.bst_pc) ==>
+               bir_is_valid_state p (bir_exec_stmt p (BStmt_Halt ex) st)``,
+
+SIMP_TAC (std_ss++bir_state_ss++bir_termcode_ss) [bir_exec_stmt_def, bir_exec_stmt_halt_def,
+  bir_is_valid_state_def]);
+
+
+val bir_exec_step_valid_state_invar_assert = prove (
+  ``!p st ex. (bir_is_valid_program p /\ bir_is_valid_state p st /\ bir_is_valid_pc p st.bst_pc) ==>
+               bir_is_valid_state p (bir_exec_stmt p (BStmt_Assert ex) st)``,
+
+SIMP_TAC (std_ss++bir_state_ss++bir_termcode_ss) [bir_exec_stmt_def, bir_exec_stmt_assert_def] >>
+REPEAT GEN_TAC >> STRIP_TAC >>
+Cases_on `bir_dest_bool_val (bir_eval_exp ex st.bst_environ)` >- (
+  ASM_SIMP_TAC std_ss [bir_is_valid_state_set_failed]
+) >>
+rename1 `SOME c` >>
+Cases_on `c` >| [
+  ASM_SIMP_TAC std_ss [bir_is_valid_state_incr_pc],
+  ASM_SIMP_TAC std_ss [bir_is_valid_state_set_failed]
+]);
+
+
+val bir_exec_step_valid_state_invar_assume = prove (
+  ``!p st ex. (bir_is_valid_program p /\ bir_is_valid_state p st /\ bir_is_valid_pc p st.bst_pc) ==>
+               bir_is_valid_state p (bir_exec_stmt p (BStmt_Assume ex) st)``,
+
+SIMP_TAC (std_ss++bir_state_ss++bir_termcode_ss) [bir_exec_stmt_def, bir_exec_stmt_assume_def] >>
+REPEAT GEN_TAC >> STRIP_TAC >>
+Cases_on `bir_dest_bool_val (bir_eval_exp ex st.bst_environ)` >- (
+  ASM_SIMP_TAC std_ss [bir_is_valid_state_set_failed]
+) >>
+rename1 `SOME c` >>
+Cases_on `c` >| [
+  ASM_SIMP_TAC std_ss [bir_is_valid_state_incr_pc],
+  FULL_SIMP_TAC (std_ss++bir_state_ss++bir_termcode_ss) [bir_is_valid_state_def]
+]);
+
+
+val bir_exec_step_valid_state_invar = store_thm ("bir_exec_step_valid_state_invar",
+``!p st. bir_is_valid_program p /\ bir_is_valid_state p st ==>
+         bir_is_valid_state p (bir_exec_step p st)``,
+
+REPEAT STRIP_TAC >>
+IMP_RES_TAC bir_exec_step_valid_THM >>
+Cases_on `bir_state_is_terminated st` >> FULL_SIMP_TAC std_ss [bir_is_valid_state_exec_ignore] >>
+Cases_on `stmt` >> (
+  ASM_SIMP_TAC std_ss [bir_exec_step_valid_state_invar_declare,
+    bir_exec_step_valid_state_invar_assign,
+    bir_exec_step_valid_state_invar_cjmp,
+    bir_exec_step_valid_state_invar_jmp,
+    bir_exec_step_valid_state_invar_halt,
+    bir_exec_step_valid_state_invar_assume,
+    bir_exec_step_valid_state_invar_assert]
+));
+
+
+
+val bir_exec_step_FUNPOW_valid_state_invar = store_thm ("bir_exec_step_FUNPOW_valid_state_invar",
+``!p st n. bir_is_valid_program p /\ bir_is_valid_state p st ==>
+           bir_is_valid_state p (FUNPOW (bir_exec_step p) n st)``,
+
+Induct_on `n` >> (
+  ASM_SIMP_TAC std_ss [arithmeticTheory.FUNPOW, bir_exec_step_valid_state_invar]
+));
+
+
+
+
+(* ------------------------------------------------------------------------- *)
+(*  The execs field is just a counter                                        *)
+(* ------------------------------------------------------------------------- *)
+
+val bir_state_normalise_pc_execs = store_thm ("bir_state_normalise_pc_execs",
+  ``!p st. (bir_state_normalise_pc p st).bst_execs = st.bst_execs``,
+REPEAT GEN_TAC >>
+SIMP_TAC std_ss [bir_state_normalise_pc_def] >>
+Cases_on `bir_pc_normalise p st.bst_pc` >> (
+  ASM_SIMP_TAC (std_ss++bir_state_ss) []
+));
+
+
+val bir_state_incr_pc_execs = store_thm ("bir_state_incr_pc_execs",
+  ``!p st. (bir_state_incr_pc p st).bst_execs = st.bst_execs``,
+SIMP_TAC (std_ss++bir_state_ss) [bir_state_incr_pc_def, bir_state_normalise_pc_execs]);
+
+
+val bir_state_set_failed_execs = store_thm ("bir_state_set_failed_execs",
+  ``!st msg. (bir_state_set_failed st msg).bst_execs = st.bst_execs``,
+SIMP_TAC (std_ss++bir_state_ss) [bir_state_set_failed_def]);
+
+
+val bir_state_set_pc_execs = store_thm ("bir_state_set_pc_execs",
+  ``!st p pc'. (bir_state_set_pc p st pc').bst_execs = st.bst_execs``,
+SIMP_TAC (std_ss++bir_state_ss) [bir_state_set_pc_def,
+  bir_state_normalise_pc_execs]);
+
+
+val bir_exec_step_execs = store_thm ("bir_exec_step_execs",
+``!p st. bir_is_valid_state p st ==>
+         (if bir_state_is_terminated st then
+           (bir_exec_step p st = st)
+         else ((bir_exec_step p st).bst_execs = SUC (st.bst_execs)))``,
+
+
+REPEAT STRIP_TAC >>
+IMP_RES_TAC bir_exec_step_valid_THM >>
+Cases_on `bir_state_is_terminated st` >> FULL_SIMP_TAC (std_ss++bir_state_ss) [] >>
+Cases_on `stmt` >> (
+  SIMP_TAC (std_ss++boolSimps.LIFT_COND_ss++bir_state_ss) [bir_exec_stmt_def,
+    bir_exec_stmt_declare_def, bir_exec_stmt_cjmp_def,
+    bir_exec_stmt_assume_def, bir_exec_stmt_assign_def, bir_exec_stmt_jmp_def,
+    LET_THM, bir_exec_stmt_halt_def, bir_exec_stmt_assert_def] >>
+  REPEAT CASE_TAC >> (
+    SIMP_TAC (std_ss++bir_state_ss) [bir_state_incr_pc_execs, bir_state_set_failed_execs,
+      bir_state_set_pc_execs]
+  )
+));
+
+
+val bir_state_EQ_EXCEPT_EXECS_def = Define `
+  bir_state_EQ_EXCEPT_EXECS st st' <=>
+  ((st' with bst_execs := 0) = (st with bst_execs := 0))`;
+
+val bir_state_EQ_EXCEPT_EXECS_ALT_DEF = save_thm ("bir_state_EQ_EXCEPT_EXECS_ALT_DEF",
+SIMP_RULE (std_ss++bir_state_ss) [DB.fetch "-" "bir_state_t_component_equality"]
+  bir_state_EQ_EXCEPT_EXECS_def);
+
+val bir_state_EQ_EXCEPT_EXECS_ALT_DEF = save_thm ("bir_state_EQ_EXCEPT_EXECS_ALT_DEF",
+SIMP_RULE (std_ss++bir_state_ss) [DB.fetch "-" "bir_state_t_component_equality"]
+  bir_state_EQ_EXCEPT_EXECS_def);
+
+
+val bir_state_EQ_EXCEPT_EXECS_IMP = save_thm ("bir_state_EQ_EXCEPT_EXECS_IMP",
+GEN_ALL (fst (EQ_IMP_RULE (SPEC_ALL bir_state_EQ_EXCEPT_EXECS_ALT_DEF))));
+
+
+val bir_state_normalise_pc_CHANGE_EXECS = store_thm ("bir_state_normalise_pc_CHANGE_EXECS",
+``!p st1 st2. bir_state_EQ_EXCEPT_EXECS st1 st2 ==>
+              bir_state_EQ_EXCEPT_EXECS (bir_state_normalise_pc p st1) (bir_state_normalise_pc p st2)``,
+
+SIMP_TAC std_ss [bir_state_normalise_pc_def, bir_state_EQ_EXCEPT_EXECS_ALT_DEF] >>
+REPEAT GEN_TAC >> STRIP_TAC >>
+CASE_TAC >> ASM_SIMP_TAC (std_ss++bir_state_ss) []);
+
+
+val bir_state_incr_pc_CHANGE_EXECS = store_thm ("bir_state_incr_pc_CHANGE_EXECS",
+``!p st1 st2. bir_state_EQ_EXCEPT_EXECS st1 st2 ==>
+              bir_state_EQ_EXCEPT_EXECS (bir_state_incr_pc p st1) (bir_state_incr_pc p st2)``,
+
+SIMP_TAC std_ss [bir_state_incr_pc_def, bir_state_normalise_pc_def, bir_state_EQ_EXCEPT_EXECS_ALT_DEF] >>
+REPEAT GEN_TAC >> STRIP_TAC >>
+CASE_TAC >> CASE_TAC >> FULL_SIMP_TAC (std_ss++bir_state_ss) []);
+
+
+val bir_state_set_pc_CHANGE_EXECS = store_thm ("bir_state_set_pc_CHANGE_EXECS",
+``!p st1 st2 l. bir_state_EQ_EXCEPT_EXECS st1 st2 ==>
+                bir_state_EQ_EXCEPT_EXECS (bir_state_set_pc p st1 l) (bir_state_set_pc p st2 l)``,
+
+REPEAT STRIP_TAC >>
+SIMP_TAC std_ss [bir_state_set_pc_def] >>
+MATCH_MP_TAC bir_state_normalise_pc_CHANGE_EXECS >>
+FULL_SIMP_TAC (std_ss++bir_state_ss) [bir_state_EQ_EXCEPT_EXECS_ALT_DEF]);
+
+
+val bir_exec_stmt_CHANGE_EXECS = store_thm ("bir_exec_stmt_CHANGE_EXECS",
+``!p st1 st2. bir_state_EQ_EXCEPT_EXECS st1 st2 ==>
+              (!stmt. bir_state_EQ_EXCEPT_EXECS (bir_exec_stmt p stmt st1) (bir_exec_stmt p stmt st2))``,
+
+Cases_on `p` >> rename1 `BirProgram p` >>
+SIMP_TAC std_ss [Once bir_state_EQ_EXCEPT_EXECS_ALT_DEF] >>
+REPEAT GEN_TAC >> STRIP_TAC >>
+Cases >> ASM_SIMP_TAC std_ss [bir_exec_stmt_def] >| [
+  ASM_SIMP_TAC std_ss [bir_exec_stmt_declare_def, LET_DEF] >>
+  Q.HO_MATCH_ABBREV_TAC `bir_state_EQ_EXCEPT_EXECS (if (bir_is_regular_env env) then _ else _) _` >>
+  CASE_TAC >- (
+    MATCH_MP_TAC bir_state_incr_pc_CHANGE_EXECS >>
+    ASM_SIMP_TAC (std_ss++bir_state_ss) [bir_state_EQ_EXCEPT_EXECS_ALT_DEF]
+  ) >>
+  ASM_SIMP_TAC (std_ss++bir_state_ss) [bir_state_set_failed_def, bir_state_EQ_EXCEPT_EXECS_ALT_DEF],
+
+
+  ASM_SIMP_TAC std_ss [bir_exec_stmt_assign_def, LET_DEF] >>
+  Q.HO_MATCH_ABBREV_TAC `bir_state_EQ_EXCEPT_EXECS (if (bir_is_regular_env env) then _ else _) _` >>
+  CASE_TAC >- (
+    MATCH_MP_TAC bir_state_incr_pc_CHANGE_EXECS >>
+    ASM_SIMP_TAC (std_ss++bir_state_ss) [bir_state_EQ_EXCEPT_EXECS_ALT_DEF]
+  ) >>
+  ASM_SIMP_TAC (std_ss++bir_state_ss) [bir_state_set_failed_def, bir_state_EQ_EXCEPT_EXECS_ALT_DEF],
+
+
+  ASM_SIMP_TAC std_ss [bir_exec_stmt_jmp_def] >>
+  CASE_TAC >- (
+    MATCH_MP_TAC bir_state_set_pc_CHANGE_EXECS >>
+    ASM_SIMP_TAC std_ss [bir_state_EQ_EXCEPT_EXECS_ALT_DEF]
+  ) >>
+  ASM_SIMP_TAC (std_ss++bir_state_ss) [bir_state_EQ_EXCEPT_EXECS_ALT_DEF],
+
+
+  ASM_SIMP_TAC std_ss [bir_exec_stmt_cjmp_def, bir_exec_stmt_jmp_def] >>
+  REPEAT CASE_TAC >> TRY (
+    ASM_SIMP_TAC (std_ss++bir_state_ss) [bir_state_set_failed_def,
+      bir_state_EQ_EXCEPT_EXECS_ALT_DEF] >>
+    NO_TAC
+  ) >> (
+    MATCH_MP_TAC bir_state_set_pc_CHANGE_EXECS >>
+    ASM_SIMP_TAC std_ss [bir_state_EQ_EXCEPT_EXECS_ALT_DEF]
+  ),
+
+
+  ASM_SIMP_TAC (std_ss++bir_state_ss) [bir_exec_stmt_halt_def,
+    bir_state_EQ_EXCEPT_EXECS_ALT_DEF],
+
+  ASM_SIMP_TAC (std_ss++bir_state_ss) [bir_exec_stmt_assert_def] >>
+  REPEAT CASE_TAC >> TRY (
+    ASM_SIMP_TAC (std_ss++bir_state_ss) [bir_state_set_failed_def,
+      bir_state_EQ_EXCEPT_EXECS_ALT_DEF] >>
+    NO_TAC
+  ) >>
+  MATCH_MP_TAC bir_state_incr_pc_CHANGE_EXECS >>
+  ASM_SIMP_TAC std_ss [bir_state_EQ_EXCEPT_EXECS_ALT_DEF],
+
+
+  ASM_SIMP_TAC (std_ss++bir_state_ss) [bir_exec_stmt_assume_def] >>
+  REPEAT CASE_TAC >> TRY (
+    ASM_SIMP_TAC (std_ss++bir_state_ss) [bir_state_set_failed_def,
+      bir_state_EQ_EXCEPT_EXECS_ALT_DEF] >>
+    NO_TAC
+  ) >>
+  MATCH_MP_TAC bir_state_incr_pc_CHANGE_EXECS >>
+  ASM_SIMP_TAC std_ss [bir_state_EQ_EXCEPT_EXECS_ALT_DEF]
+]);
+
+
+
+val bir_exec_step_CHANGE_EXECS = store_thm ("bir_exec_step_CHANGE_EXECS",
+``!p st1 st2. bir_state_EQ_EXCEPT_EXECS st1 st2 ==>
+              bir_state_EQ_EXCEPT_EXECS (bir_exec_step p st1) (bir_exec_step p st2)``,
+
+SIMP_TAC std_ss [bir_exec_step_def, Once bir_state_EQ_EXCEPT_EXECS_ALT_DEF] >>
+REPEAT STRIP_TAC >>
+`bir_state_is_terminated st1 = bir_state_is_terminated st2` by
+  ASM_SIMP_TAC std_ss [bir_state_is_terminated_def] >>
+Cases_on `bir_state_is_terminated st2` >- (
+  ASM_SIMP_TAC std_ss [bir_state_EQ_EXCEPT_EXECS_ALT_DEF]
+) >>
+Cases_on `bir_get_current_statement p st1.bst_pc` >- (
+  ASM_SIMP_TAC (std_ss++bir_state_ss) [bir_state_EQ_EXCEPT_EXECS_ALT_DEF,
+    bir_state_set_failed_def]
+) >>
+rename1 `_ = SOME stmt` >>
+`bir_state_EQ_EXCEPT_EXECS
+   (bir_exec_stmt p stmt st1) (bir_exec_stmt p stmt st2)` suffices_by (
+  ASM_SIMP_TAC (std_ss++bir_state_ss) [bir_state_EQ_EXCEPT_EXECS_ALT_DEF]
+) >>
+MATCH_MP_TAC bir_exec_stmt_CHANGE_EXECS >>
+ASM_SIMP_TAC (std_ss++bir_state_ss) [bir_state_EQ_EXCEPT_EXECS_ALT_DEF]);
+
+
+
+
+(* ------------------------------------------------------------------------- *)
+(*  Executing multiple steps                                                 *)
+(* ------------------------------------------------------------------------- *)
+
+val bir_exec_steps_opt_def = Define `bir_exec_steps_opt p state b max_steps =
+   OWHILE (\ (n, st). option_CASE max_steps T (\m. n < (m:num)) /\
+                      ~(bir_state_is_terminated st)) (\ (n, st).
+     (SUC n, bir_exec_step p st)) (b, state)`;
+
+val bir_exec_step_n_def = Define `
+  bir_exec_step_n p state n = THE (bir_exec_steps_opt p state 0 (SOME n))`;
+
+val bir_exec_steps_def = Define `
+  (bir_exec_steps p state = bir_exec_steps_opt p state 0 NONE)`
+
+
+val bir_exec_steps_opt_NONE_REWRS = store_thm ("bir_exec_steps_opt_NONE_REWRS",
+  ``bir_exec_steps_opt p state b NONE =
+    (if bir_state_is_terminated state then SOME (b, state) else
+       bir_exec_steps_opt p (bir_exec_step p state) (SUC b) NONE)``,
+
+SIMP_TAC std_ss [Once whileTheory.OWHILE_THM, bir_exec_steps_opt_def] >>
+METIS_TAC[]);
+
+
+val bir_exec_steps_opt_SOME_REWRS = store_thm ("bir_exec_steps_opt_SOME_REWRS",
+  ``bir_exec_steps_opt p state b (SOME m) =
+    (if ((m <= b) \/ bir_state_is_terminated state) then SOME (b, state) else
+       bir_exec_steps_opt p (bir_exec_step p state) (SUC b) (SOME m))``,
+
+SIMP_TAC std_ss [Once whileTheory.OWHILE_THM, bir_exec_steps_opt_def] >>
+COND_CASES_TAC >> FULL_SIMP_TAC arith_ss []);
+
+
+val FUNPOW_bir_exec_steps_opt_REWR = store_thm ("FUNPOW_bir_exec_steps_opt_REWR",
+  ``!n b st. (FUNPOW (\(n,st). (SUC n,bir_exec_step p st)) n (b,st)) =
+      (b + n, FUNPOW (bir_exec_step p) n st)``,
+Induct >> ASM_SIMP_TAC arith_ss [arithmeticTheory.FUNPOW]);
+
+
+val bir_exec_steps_opt_EQ_NONE = store_thm ("bir_exec_steps_opt_EQ_NONE",
+  ``(bir_exec_steps_opt p state b mo = NONE) <=>
+    ((mo = NONE) /\ (!n. ~(bir_state_is_terminated (FUNPOW (bir_exec_step p) n state))))``,
+
+SIMP_TAC (std_ss ++ boolSimps.EQUIV_EXTRACT_ss) [bir_exec_steps_opt_def, whileTheory.OWHILE_EQ_NONE,
+  FUNPOW_bir_exec_steps_opt_REWR, FORALL_AND_THM] >>
+DISCH_TAC >> POP_ASSUM (K ALL_TAC) >>
+Cases_on `mo` >> SIMP_TAC std_ss [] >>
+Q.EXISTS_TAC `x` >> DECIDE_TAC);
+
+
+val bir_exec_steps_EQ_NONE = store_thm ("bir_exec_steps_EQ_NONE",
+  ``(bir_exec_steps p state = NONE) <=>
+    (!n. ~(bir_state_is_terminated (FUNPOW (bir_exec_step p) n state)))``,
+
+SIMP_TAC std_ss [bir_exec_steps_def, bir_exec_steps_opt_EQ_NONE]);
+
+
+val bir_exec_steps_opt_EQ_SOME = store_thm ("bir_exec_steps_opt_EQ_SOME",
+  ``(case mo of NONE => T | SOME m => (b <= m)) ==>
+    ((bir_exec_steps_opt p state b mo = SOME (c, state')) <=>
+    ((case mo of NONE => (bir_state_is_terminated state')
+               | SOME m => ((c <= m) /\ ((c < m) ==> (bir_state_is_terminated state')))) /\
+     (b <= c) /\
+     (state' = FUNPOW (bir_exec_step p) (c - b) state) /\
+     (!n. n < c-b ==> ~(bir_state_is_terminated (FUNPOW (bir_exec_step p) n state)))))``,
+
+SIMP_TAC std_ss [whileTheory.OWHILE_def, bir_exec_steps_opt_def, FUNPOW_bir_exec_steps_opt_REWR] >>
+STRIP_TAC >>
+Q.ABBREV_TAC `P = \n. ~(case mo of NONE => T | SOME m => b + n < m) \/
+  bir_state_is_terminated (FUNPOW (bir_exec_step p) n state)` >>
+Tactical.REVERSE (Cases_on `?n. P n`) >- (
+  UNABBREV_ALL_TAC >>
+  FULL_SIMP_TAC std_ss [FORALL_AND_THM] >>
+  Cases_on `mo` >| [
+    SIMP_TAC std_ss [] >> METIS_TAC[],
+
+    rename1 `SOME m` >>
+    FULL_SIMP_TAC arith_ss [] >>
+    Q.PAT_X_ASSUM `!n. b + n < m` (MP_TAC o Q.SPEC `m`) >>
+    SIMP_TAC arith_ss []
+  ]
+) >>
+FULL_SIMP_TAC std_ss [] >>
+Q.SUBGOAL_THEN `$? (P:num->bool)` (fn thm => REWRITE_TAC [thm]) >- (
+  UNABBREV_ALL_TAC >>
+  Q.EXISTS_TAC `n` >> FULL_SIMP_TAC std_ss []
+) >>
+Tactical.REVERSE (Cases_on `b <= c`) >> ASM_SIMP_TAC arith_ss [] >>
+Q.ABBREV_TAC `n' = c - b` >>
+`c = b + n'` by (UNABBREV_ALL_TAC >> DECIDE_TAC) >>
+ASM_SIMP_TAC (std_ss++boolSimps.CONJ_ss++boolSimps.EQUIV_EXTRACT_ss) [] >>
+STRIP_TAC >>
+EQ_TAC >| [
+  STRIP_TAC >>
+  `!n. n < n' ==> ~(P n)` by METIS_TAC [whileTheory.LESS_LEAST] >>
+  `P n'` by METIS_TAC[whileTheory.FULL_LEAST_INTRO] >>
+  NTAC 2 (POP_ASSUM MP_TAC) >>
+  Q.PAT_X_ASSUM `P n` (K ALL_TAC) >>
+  Q.PAT_X_ASSUM `$LEAST P = _` (K ALL_TAC) >>
+  Q.UNABBREV_TAC `P` >>
+  ASM_SIMP_TAC std_ss [] >>
+  Cases_on `mo` >> SIMP_TAC arith_ss [DISJ_IMP_THM] >>
+  Cases_on `b + n' <= x` >> ASM_SIMP_TAC std_ss [] >>
+  FULL_SIMP_TAC arith_ss [] >>
+  Cases_on `n'` >- FULL_SIMP_TAC arith_ss [] >>
+  rename1 `~(b + SUC n'' <= _)` >>
+  Q.EXISTS_TAC `n''` >>
+  ASM_SIMP_TAC arith_ss [],
+
+
+  STRIP_TAC >>
+  MATCH_MP_TAC bitTheory.LEAST_THM >>
+  Q.PAT_X_ASSUM `P n` (K ALL_TAC) >>
+  Q.UNABBREV_TAC `P` >>
+  ASM_SIMP_TAC std_ss [] >>
+  Cases_on `mo` >> FULL_SIMP_TAC arith_ss [] >>
+  METIS_TAC[]
+]);
+
+
+
+val bir_exec_steps_EQ_SOME = store_thm ("bir_exec_steps_EQ_SOME",
+  ``((bir_exec_steps p state = SOME (c, state')) <=>
+    ((bir_state_is_terminated state') /\
+     (state' = FUNPOW (bir_exec_step p) c state) /\
+     (!n. n < c ==> ~(bir_state_is_terminated (FUNPOW (bir_exec_step p) n state)))))``,
+
+SIMP_TAC std_ss [bir_exec_steps_def, bir_exec_steps_opt_EQ_SOME]);
+
+
+val bir_exec_step_n_EQ_THM = store_thm ("bir_exec_step_n_EQ_THM",
+  ``((bir_exec_step_n p state n = (c, state')) <=>
+     ((c <= n) /\ ((c < n) ==> (bir_state_is_terminated state'))) /\
+     (state' = FUNPOW (bir_exec_step p) c state) /\
+     (!n'. n' < c ==> ~(bir_state_is_terminated (FUNPOW (bir_exec_step p) n' state))))``,
+
+SIMP_TAC std_ss [bir_exec_step_n_def] >>
+Cases_on `bir_exec_steps_opt p state 0 (SOME n)` >- (
+  FULL_SIMP_TAC std_ss [bir_exec_steps_opt_EQ_NONE]
+) >>
+FULL_SIMP_TAC std_ss [] >>
+rename1 `x = (c, state')` >>
+Cases_on `x` >>
+rename1 `(c0, state'') = (c, state')` >>
+FULL_SIMP_TAC (std_ss) [bir_exec_steps_opt_EQ_SOME] >>
+EQ_TAC >> STRIP_TAC >- (
+  REPEAT (BasicProvers.VAR_EQ_TAC) >>
+  ASM_SIMP_TAC std_ss []
+) >>
+ASM_SIMP_TAC (std_ss ++ boolSimps.CONJ_ss) [] >>
+Cases_on `c < c0` >- (
+  `c < n` by DECIDE_TAC >>
+  METIS_TAC[]
+) >>
+Cases_on `c0 < c` >- (
+  `c0 < n` by DECIDE_TAC >>
+  METIS_TAC[]
+) >>
+DECIDE_TAC);
+
+
+val bir_exec_step_FUNPOW_EXECS_ADD = store_thm ("bir_exec_step_FUNPOW_EXECS_ADD",
+``!p state n.
+    bir_is_valid_state p state ==> bir_is_valid_program p ==>
+    (!i. i < n ==> ~(bir_state_is_terminated (FUNPOW (bir_exec_step p) i state))) ==>
+    ((FUNPOW (bir_exec_step p) n state).bst_execs = state.bst_execs + n)``,
+
+GEN_TAC >> GEN_TAC >>
+Induct_on `n` >- (
+  SIMP_TAC std_ss [arithmeticTheory.FUNPOW]
+) >>
+REPEAT STRIP_TAC >>
+FULL_SIMP_TAC arith_ss [arithmeticTheory.FUNPOW_SUC] >>
+Q.ABBREV_TAC `state' =  (FUNPOW (bir_exec_step p) n state)` >>
+MP_TAC (Q.SPECL [`p`, `state'`] bir_exec_step_execs) >>
+`bir_is_valid_state p state'` by METIS_TAC[bir_exec_step_FUNPOW_valid_state_invar] >>
+Q.PAT_X_ASSUM `!i. _` (MP_TAC o Q.SPEC `n`) >>
+ASM_SIMP_TAC arith_ss []);
+
+
+
+val bir_exec_steps_opt_EXECS_ADD = store_thm ("bir_exec_steps_opt_EXECS_ADD",
+``!p state state' b mo c.
+    bir_is_valid_state p state ==> bir_is_valid_program p ==>
+    (case mo of NONE => T | SOME m => b <= m) ==>
+    (bir_exec_steps_opt p state b mo = SOME (c, state')) ==>
+    (state'.bst_execs = state.bst_execs + (c - b))``,
+
+SIMP_TAC std_ss [bir_exec_steps_opt_EQ_SOME] >>
+REPEAT STRIP_TAC >>
+MATCH_MP_TAC (SIMP_RULE std_ss [AND_IMP_INTRO] bir_exec_step_FUNPOW_EXECS_ADD) >>
+ASM_SIMP_TAC std_ss []);
+
+
+
+val bir_exec_step_n_EXECS_ADD = store_thm ("bir_exec_step_n_EXECS_ADD",
+``!p state state' n c.
+    bir_is_valid_state p state ==> bir_is_valid_program p ==>
+    (bir_exec_step_n p state n = (c, state')) ==>
+    (state'.bst_execs = state.bst_execs + c)``,
+
+REPEAT STRIP_TAC >>
+FULL_SIMP_TAC std_ss [bir_exec_step_n_EQ_THM] >>
+MATCH_MP_TAC (SIMP_RULE std_ss [AND_IMP_INTRO] bir_exec_step_FUNPOW_EXECS_ADD) >>
+ASM_SIMP_TAC std_ss []);
+
+
+
+val bir_exec_steps_EXECS_ADD = store_thm ("bir_exec_steps_EXECS_ADD",
+``!p state state' c.
+    bir_is_valid_state p state ==> bir_is_valid_program p ==>
+    (bir_exec_steps p state = SOME (c, state')) ==>
+    (state'.bst_execs = state.bst_execs + c)``,
+
+REPEAT STRIP_TAC >>
+MP_TAC (Q.SPECL [`p`, `state`, `state'`, `0`, `NONE`] bir_exec_steps_opt_EXECS_ADD) >>
+FULL_SIMP_TAC std_ss [bir_exec_steps_def]);
+
+
+
+
+(* ------------------------------------------------------------------------- *)
+(*  Environment Order                                                        *)
+(* ------------------------------------------------------------------------- *)
+
+
+val bir_state_set_failed_SAME_ENV = store_thm ("bir_state_set_failed_SAME_ENV",
+  ``!st msg. (bir_state_set_failed st msg).bst_environ = st.bst_environ``,
+SIMP_TAC (std_ss++bir_state_ss) [bir_state_set_failed_def]);
+
+
+val bir_state_normalise_pc_SAME_ENV = store_thm ("bir_state_normalise_pc_SAME_ENV",
+  ``!p st. (bir_state_normalise_pc p st).bst_environ = st.bst_environ``,
+REPEAT STRIP_TAC >>
+SIMP_TAC std_ss [bir_state_normalise_pc_def] >>
+CASE_TAC >> SIMP_TAC (std_ss++bir_state_ss) []);
+
+
+val bir_state_incr_pc_SAME_ENV = store_thm ("bir_state_incr_pc_SAME_ENV",
+  ``!p st. (bir_state_incr_pc p st).bst_environ = st.bst_environ``,
+SIMP_TAC (std_ss++bir_state_ss) [bir_state_incr_pc_def, bir_state_normalise_pc_SAME_ENV]);
+
+val bir_state_set_pc_SAME_ENV = store_thm ("bir_state_set_pc_SAME_ENV",
+  ``!p st l. (bir_state_set_pc p st l).bst_environ = st.bst_environ``,
+SIMP_TAC (std_ss++bir_state_ss) [bir_state_set_pc_def, bir_state_normalise_pc_SAME_ENV]);
+
+
+val bir_exec_stmt_jmp_SAME_ENV = store_thm("bir_exec_stmt_jmp_SAME_ENV",
+  ``!p st l. (bir_exec_stmt_jmp p l st).bst_environ = st.bst_environ``,
+SIMP_TAC std_ss [bir_exec_stmt_jmp_def] >>
+REPEAT STRIP_TAC >>
+COND_CASES_TAC >> SIMP_TAC (std_ss++bir_state_ss) [bir_state_set_pc_SAME_ENV]);
+
+
+
+val bir_exec_stmt_cjmp_SAME_ENV = store_thm("bir_exec_stmt_cjmp_SAME_ENV",
+  ``!p e st l1 l2. (bir_exec_stmt_cjmp p e l1 l2 st).bst_environ = st.bst_environ``,
+SIMP_TAC std_ss [bir_exec_stmt_cjmp_def] >>
+REPEAT STRIP_TAC >>
+REPEAT CASE_TAC >> SIMP_TAC (std_ss++bir_state_ss) [bir_exec_stmt_jmp_SAME_ENV,
+   bir_state_set_failed_SAME_ENV]
+);
+
+
+val bir_exec_stmt_halt_SAME_ENV = store_thm("bir_exec_stmt_halt_SAME_ENV",
+  ``!e st. (bir_exec_stmt_halt e st).bst_environ = st.bst_environ``,
+SIMP_TAC (std_ss++bir_state_ss) [bir_exec_stmt_halt_def]);
+
+
+val bir_exec_stmt_assert_SAME_ENV = store_thm("bir_exec_stmt_assert_SAME_ENV",
+  ``!p e st. (bir_exec_stmt_assert p e st).bst_environ = st.bst_environ``,
+SIMP_TAC (std_ss++bir_state_ss) [bir_exec_stmt_assert_def] >>
+REPEAT STRIP_TAC >>
+REPEAT CASE_TAC >> SIMP_TAC (std_ss++bir_state_ss) [bir_state_incr_pc_SAME_ENV,
+   bir_state_set_failed_SAME_ENV]
+);
+
+
+val bir_exec_stmt_assume_SAME_ENV = store_thm("bir_exec_stmt_assume_SAME_ENV",
+  ``!p e st. (bir_exec_stmt_assume p e st).bst_environ = st.bst_environ``,
+SIMP_TAC (std_ss++bir_state_ss) [bir_exec_stmt_assume_def] >>
+REPEAT STRIP_TAC >>
+REPEAT CASE_TAC >> SIMP_TAC (std_ss++bir_state_ss) [bir_state_incr_pc_SAME_ENV,
+   bir_state_set_failed_SAME_ENV]
+);
+
+
+val bir_exec_stmt_declare_ENV = store_thm("bir_exec_stmt_declare_ENV",
+  ``!p vn vty st. (bir_exec_stmt_declare p vn vty st).bst_environ =
+      if (bir_env_varname_is_bound st.bst_environ vn) then st.bst_environ else
+      (bir_env_update vn (bir_declare_initial_value vty) vty
+            st.bst_environ)``,
+
+SIMP_TAC (std_ss++bir_state_ss) [bir_exec_stmt_declare_def, LET_DEF] >>
+REPEAT STRIP_TAC >>
+REPEAT CASE_TAC >> (
+   FULL_SIMP_TAC (std_ss++bir_state_ss) [bir_state_incr_pc_SAME_ENV,
+     bir_state_set_failed_SAME_ENV, bir_is_regular_env_def]
+) >>
+Cases_on `st.bst_environ` >> FULL_SIMP_TAC std_ss [bir_env_update_def] >>
+Cases_on `vty` >> FULL_SIMP_TAC std_ss [bir_declare_initial_value_def,
+  bir_is_regular_env_def, type_of_bir_val_def]);
+
+
+val bir_exec_stmt_assign_ENV = store_thm("bir_exec_stmt_assign_ENV",
+  ``!p v e st.
+      (bir_exec_stmt_assign p v e st).bst_environ =
+      (if bir_is_regular_env (bir_env_write v (bir_eval_exp e st.bst_environ) st.bst_environ) then
+         (bir_env_write v (bir_eval_exp e st.bst_environ) st.bst_environ)
+       else st.bst_environ)``,
+
+SIMP_TAC (std_ss++bir_state_ss) [bir_exec_stmt_assign_def, LET_DEF] >>
+REPEAT STRIP_TAC >>
+REPEAT CASE_TAC >> (
+   ASM_SIMP_TAC (std_ss++bir_state_ss) [bir_state_incr_pc_SAME_ENV,
+     bir_state_set_failed_SAME_ENV]
+));
+
+
+val bir_exec_stmt_ENV_ORDER = store_thm ("bir_exec_stmt_ENV_ORDER",
+``!p st stmt. bir_env_order st.bst_environ (bir_exec_stmt p stmt st).bst_environ``,
+
+Cases_on `stmt` >> (
+  SIMP_TAC (std_ss++boolSimps.LIFT_COND_ss) [bir_exec_stmt_def, bir_exec_stmt_jmp_SAME_ENV,
+    bir_exec_stmt_cjmp_SAME_ENV, bir_exec_stmt_halt_SAME_ENV,
+    bir_exec_stmt_assert_SAME_ENV, bir_exec_stmt_assume_SAME_ENV,
+    bir_env_order_REFL, bir_exec_stmt_assign_ENV,  bir_exec_stmt_declare_ENV]
+) >- (
+  REPEAT STRIP_TAC >>
+  rename1 `bir_var_name v` >>
+  Cases_on `bir_env_varname_is_bound st.bst_environ (bir_var_name v)` >> ASM_REWRITE_TAC[] >>
+  MATCH_MP_TAC bir_env_order_update >>
+  ASM_REWRITE_TAC[] >>
+  Cases_on `bir_var_type v` >> (
+    ASM_SIMP_TAC std_ss [bir_declare_initial_value_def, type_of_bir_val_def]
+  )
+) >- (
+  REPEAT STRIP_TAC >>
+  MATCH_MP_TAC bir_env_order_write >>
+  ASM_REWRITE_TAC[]
+));
+
+
+val bir_exec_step_ENV_ORDER = store_thm ("bir_exec_step_ENV_ORDER",
+``!p st. bir_env_order st.bst_environ (bir_exec_step p st).bst_environ``,
+
+REPEAT GEN_TAC >>
+SIMP_TAC std_ss [bir_exec_step_def] >>
+REPEAT CASE_TAC >> (
+  SIMP_TAC (std_ss++bir_state_ss) [bir_env_order_REFL, bir_state_set_failed_SAME_ENV,
+    bir_exec_stmt_ENV_ORDER]
+));
+
+
+
+val bir_exec_step_FUNPOW_ENV_ORDER = store_thm ("bir_exec_step_FUNPOW_ENV_ORDER",
+``!p n st. bir_env_order st.bst_environ (FUNPOW (bir_exec_step p) n st).bst_environ``,
+
+GEN_TAC >>
+Induct >> (
+  SIMP_TAC std_ss [arithmeticTheory.FUNPOW, bir_env_order_REFL]
+) >>
+GEN_TAC >>
+MATCH_MP_TAC (SIMP_RULE std_ss [AND_IMP_INTRO] bir_env_order_TRANS) >>
+Q.EXISTS_TAC `(bir_exec_step p st).bst_environ` >>
+ASM_SIMP_TAC std_ss [bir_exec_step_ENV_ORDER]);
+
+
+
+val bir_exec_steps_ENV_ORDER = store_thm ("bir_exec_steps_ENV_ORDER",
+``!p c st st'. (bir_exec_steps p st = SOME (c, st')) ==>
+  bir_env_order st.bst_environ st'.bst_environ``,
+
+SIMP_TAC std_ss [bir_exec_steps_EQ_SOME, bir_exec_step_FUNPOW_ENV_ORDER]);
+
+
+val bir_exec_step_n_ENV_ORDER = store_thm ("bir_exec_step_n_ENV_ORDER",
+``!p c n st st'. (bir_exec_step_n p st n = (c, st')) ==>
+  bir_env_order st.bst_environ st'.bst_environ``,
+
+SIMP_TAC std_ss [bir_exec_step_n_EQ_THM, bir_exec_step_FUNPOW_ENV_ORDER]);
+
+
+val _ = export_theory();
