bir_typingScript.sml
@@ -1,0 +1,362 @@
+open HolKernel Parse boolLib bossLib;
+open wordsTheory bitstringTheory;
+open bir_auxiliaryTheory bir_immTheory bir_valuesTheory;
+open bir_imm_expTheory bir_mem_expTheory bir_envTheory;
+open bir_expTheory bir_programTheory;
+open wordsLib;
+
+val _ = new_theory "bir_typing";
+
+
+(* ------------------------------------------------------------------------- *)
+(*  Expressions                                                              *)
+(* ------------------------------------------------------------------------- *)
+
+val bir_val_ss = rewrites (type_rws ``:bir_val_t``);
+val bir_type_ss = rewrites (type_rws ``:bir_type_t``);
+
+
+val type_of_bir_exp_def = Define `
+  (type_of_bir_exp (BExp_Const i) = SOME (BType_Imm (type_of_bir_imm i))) /\
+
+  (type_of_bir_exp (BExp_Den v) = SOME (bir_var_type v)) /\
+
+  (type_of_bir_exp (BExp_Cast ct e rty) = (case (type_of_bir_exp e) of
+      NONE => NONE
+    | SOME ty => (if (bir_type_is_Imm ty) then SOME (BType_Imm rty) else NONE))) /\
+
+  (type_of_bir_exp (BExp_UnaryExp et e) = (case (type_of_bir_exp e) of
+      NONE => NONE
+    | SOME ty => (if (bir_type_is_Imm ty) then
+        SOME ty else NONE))) /\
+
+  (type_of_bir_exp (BExp_BinExp et e1 e2) = (case (type_of_bir_exp e1,
+       type_of_bir_exp e2) of
+       (SOME ty1, SOME ty2) => (if ((bir_type_is_Imm ty1) /\ (ty2 = ty1)) then SOME ty1 else NONE)
+       | _, _ => NONE)) /\
+
+  (type_of_bir_exp (BExp_BinPred pt e1 e2) = (case (type_of_bir_exp e1,
+       type_of_bir_exp e2) of
+       (SOME ty1, SOME ty2) => (if ((bir_type_is_Imm ty1) /\ (ty2 = ty1)) then SOME BoolType else NONE)
+       | _, _ => NONE)) /\
+
+
+  (type_of_bir_exp (BExp_IfThenElse ec e1 e2) = (case (type_of_bir_exp ec, type_of_bir_exp e1,
+       type_of_bir_exp e2) of
+       (SOME ect, SOME ty1, SOME ty2) => (if ((ect = BoolType) /\ (ty2 = ty1)) then SOME ty1 else NONE)
+       | _, _, _ => NONE)) /\
+
+  (type_of_bir_exp (BExp_Load me ae en rty) = (case (type_of_bir_exp me, type_of_bir_exp ae) of
+       (SOME (BType_Mem aty vty), SOME (BType_Imm aty')) => (if (
+            (aty = aty') /\ (if en = BEnd_NoEndian then (vty = rty) else (bir_number_of_mem_splits vty rty <> NONE))
+           ) then SOME (BType_Imm rty) else NONE)
+       | _, _ => NONE)) /\
+
+  (type_of_bir_exp (BExp_Store me ae en v) = (case (type_of_bir_exp me, type_of_bir_exp ae, type_of_bir_exp v) of
+       (SOME (BType_Mem aty vty), SOME (BType_Imm aty'), SOME (BType_Imm rty)) => (if (
+            (aty = aty') /\ (if en = BEnd_NoEndian then (vty = rty) else (bir_number_of_mem_splits vty rty <> NONE))
+           ) then SOME (BType_Mem aty vty) else NONE)
+       | _, _, _ => NONE))`;
+
+
+
+val type_of_bir_exp_THM = store_thm ("type_of_bir_exp_THM",
+ ``!env. (bir_is_well_typed_env env) ==> !e ty. (type_of_bir_exp e = SOME ty) ==>
+              ((bir_eval_exp e env = BVal_Unknown) \/ (type_of_bir_val (bir_eval_exp e env) = SOME ty))``,
+
+GEN_TAC >> STRIP_TAC >>
+Induct >> (
+  SIMP_TAC (list_ss++bir_val_ss) [bir_eval_exp_def, type_of_bir_exp_def,
+     type_of_bir_val_def] >>
+  REPEAT CASE_TAC
+) >- (
+  METIS_TAC[bir_is_well_typed_env_read]
+) >- (
+  FULL_SIMP_TAC std_ss [bir_eval_cast_REWRS, bir_type_is_Imm_def] >>
+  FULL_SIMP_TAC (std_ss++bir_val_ss) [type_of_bir_val_EQ_ELIMS, bir_eval_cast_REWRS,
+    type_of_bir_gencast]
+) >- (
+  FULL_SIMP_TAC std_ss [bir_eval_unary_exp_REWRS, bir_type_is_Imm_def] >>
+  FULL_SIMP_TAC (std_ss++bir_val_ss) [type_of_bir_val_EQ_ELIMS, bir_eval_unary_exp_REWRS,
+    type_of_bir_unary_exp]
+) >- (
+  FULL_SIMP_TAC std_ss [bir_eval_bin_exp_REWRS, bir_type_is_Imm_def] >>
+  FULL_SIMP_TAC (std_ss++bir_val_ss) [type_of_bir_val_EQ_ELIMS, bir_eval_bin_exp_REWRS,
+    type_of_bir_bin_exp]
+) >- (
+  FULL_SIMP_TAC std_ss [bir_eval_bin_pred_REWRS, bir_type_is_Imm_def] >>
+  FULL_SIMP_TAC (std_ss++bir_val_ss) [type_of_bir_val_EQ_ELIMS, bir_eval_bin_pred_REWRS,
+    type_of_bir_val_def, BoolType_def, type_of_bool2b]
+) >- (
+  Cases_on `bir_eval_exp e env = BVal_Unknown` >- (
+    ASM_SIMP_TAC std_ss [bir_eval_ifthenelse_REWRS]
+  ) >>
+  FULL_SIMP_TAC std_ss [bir_eval_ifthenelse_REWRS, bir_type_is_Imm_def] >> (
+    FULL_SIMP_TAC (std_ss++bir_val_ss) [type_of_bir_val_EQ_ELIMS, bir_eval_ifthenelse_REWRS,
+      BoolType_def] >>
+    CASE_TAC
+  )
+) >- (
+  FULL_SIMP_TAC std_ss [bir_eval_load_Unknown_REWRS] >>
+  FULL_SIMP_TAC std_ss [type_of_bir_val_EQ_ELIMS, bir_eval_load_def] >>
+  REPEAT GEN_TAC >> REPEAT CASE_TAC >> (
+    METIS_TAC[type_of_bir_load_from_mem]
+  )
+) >- (
+  FULL_SIMP_TAC std_ss [bir_eval_store_Unknown_REWRS] >>
+  FULL_SIMP_TAC std_ss [type_of_bir_val_EQ_ELIMS, bir_eval_store_def] >>
+  REPEAT GEN_TAC >> REPEAT CASE_TAC
+));
+
+
+
+val type_of_bir_exp_EQ_SOME_REWRS = store_thm ("type_of_bir_exp_EQ_SOME_REWRS",``
+  (!i ty. (type_of_bir_exp (BExp_Const i) = SOME ty) <=> (ty = BType_Imm (type_of_bir_imm i))) /\
+
+  (!v ty. (type_of_bir_exp (BExp_Den v) = SOME ty) <=> (ty = bir_var_type v)) /\
+
+  (!ct e ty ty'. (type_of_bir_exp (BExp_Cast ct e ty') = SOME ty) <=> (
+     (ty = BType_Imm ty') /\ (?it. (type_of_bir_exp e = SOME (BType_Imm it))))) /\
+
+  (!et e ty. (type_of_bir_exp (BExp_UnaryExp et e) = SOME ty) <=> (
+     (bir_type_is_Imm ty) /\ (type_of_bir_exp e = SOME ty))) /\
+
+  (!et e1 e2 ty. (type_of_bir_exp (BExp_BinExp et e1 e2) = SOME ty) <=> (
+     (bir_type_is_Imm ty) /\ (type_of_bir_exp e1 = SOME ty) /\ (type_of_bir_exp e2 = SOME ty))) /\
+
+  (!pt e1 e2 ty. (type_of_bir_exp (BExp_BinPred pt e1 e2) = SOME ty) <=> (
+     (ty = BoolType) /\ (?it. (type_of_bir_exp e1 = SOME (BType_Imm it)) /\
+                              (type_of_bir_exp e2 = SOME (BType_Imm it))))) /\
+
+  (!ce e1 e2 ty. (type_of_bir_exp (BExp_IfThenElse ce e1 e2) = SOME ty) <=> (
+     (type_of_bir_exp ce = SOME BoolType) /\
+     (type_of_bir_exp e1 = SOME ty) /\
+     (type_of_bir_exp e2 = SOME ty))) /\
+
+  (!rty ty ae en me. (type_of_bir_exp (BExp_Load me ae en rty) = SOME ty) <=> (
+     (ty = BType_Imm rty) /\ (?at vt. (type_of_bir_exp me = SOME (BType_Mem at vt)) /\
+                            (type_of_bir_exp ae = SOME (BType_Imm at)) /\
+                            (if en = BEnd_NoEndian then (vt = rty) else
+                                  (bir_number_of_mem_splits vt rty <> NONE))))) /\
+
+  (!ty ae en me v. (type_of_bir_exp (BExp_Store me ae en v) = SOME ty) <=> (
+     ?at vt rty. (ty = BType_Mem at vt) /\
+             (type_of_bir_exp me = SOME (BType_Mem at vt)) /\
+             (type_of_bir_exp ae = SOME (BType_Imm at)) /\
+             (type_of_bir_exp v = SOME (BType_Imm rty)) /\
+             (if en = BEnd_NoEndian then (vt = rty) else
+                                  (bir_number_of_mem_splits vt rty <> NONE))))
+``,
+
+REPEAT CONJ_TAC >> (
+  SIMP_TAC (std_ss++boolSimps.EQUIV_EXTRACT_ss) [type_of_bir_exp_def]
+) >- (
+  REPEAT GEN_TAC >> REPEAT CASE_TAC >>
+    FULL_SIMP_TAC (std_ss++bir_type_ss) [bir_type_is_Imm_def] >> METIS_TAC[]
+) >- (
+  REPEAT GEN_TAC >> REPEAT CASE_TAC >> METIS_TAC[]
+) >- (
+  REPEAT GEN_TAC >> REPEAT CASE_TAC >> (
+    FULL_SIMP_TAC std_ss [] >> METIS_TAC[]
+  )
+) >- (
+  REPEAT GEN_TAC >> REPEAT CASE_TAC >> (
+    FULL_SIMP_TAC std_ss [bir_type_is_Imm_def] >> METIS_TAC[]
+  )
+) >- (
+  REPEAT GEN_TAC >> REPEAT CASE_TAC >> (
+    FULL_SIMP_TAC std_ss [bir_type_is_Imm_def] >> METIS_TAC[]
+  )
+) >- (
+  REPEAT GEN_TAC >> REPEAT CASE_TAC >> METIS_TAC[]
+) >- (
+  REPEAT GEN_TAC >> REPEAT CASE_TAC >> METIS_TAC[]
+));
+
+
+
+
+val type_of_bir_exp_EQ_NONE_REWRS = store_thm ("type_of_bir_exp_EQ_NONE_REWRS",``
+  (!i. ~(type_of_bir_exp (BExp_Const i) = NONE)) /\
+
+  (!v. ~(type_of_bir_exp (BExp_Den v) = NONE)) /\
+
+  (!ct e ty ty'. (type_of_bir_exp (BExp_Cast ct e ty') = NONE) <=> (
+     (!ity. (type_of_bir_exp e <> SOME (BType_Imm ity))))) /\
+
+  (!et e. (type_of_bir_exp (BExp_UnaryExp et e) = NONE) <=> (
+     (!ity. type_of_bir_exp e <> SOME (BType_Imm ity)))) /\
+
+  (!et e1 e2. (type_of_bir_exp (BExp_BinExp et e1 e2) = NONE) <=> !ity.
+     (type_of_bir_exp e1 <> SOME (BType_Imm ity)) \/
+     (type_of_bir_exp e2 <> SOME (BType_Imm ity))) /\
+
+  (!pt e1 e2. (type_of_bir_exp (BExp_BinPred pt e1 e2) = NONE) <=> !ity.
+     (type_of_bir_exp e1 <> SOME (BType_Imm ity)) \/
+     (type_of_bir_exp e2 <> SOME (BType_Imm ity))) /\
+
+  (!ce e1 e2 ty. (type_of_bir_exp (BExp_IfThenElse ce e1 e2) = NONE) <=> (
+     (type_of_bir_exp ce <> SOME BoolType) \/
+     (type_of_bir_exp e1 = NONE) \/
+     (type_of_bir_exp e2 <> type_of_bir_exp e1))) /\
+
+  (!rty ty ae en me. (type_of_bir_exp (BExp_Load me ae en rty) = NONE) <=> (
+     (!at vt. (type_of_bir_exp me = SOME (BType_Mem at vt)) /\
+              (type_of_bir_exp ae = SOME (BType_Imm at)) ==>
+              (if en = BEnd_NoEndian then (vt <> rty) else
+                   (bir_number_of_mem_splits vt rty = NONE))))) /\
+
+  (!ty ae en me v. (type_of_bir_exp (BExp_Store me ae en v) = NONE) <=> (
+     !at vt rty.
+             (type_of_bir_exp me = SOME (BType_Mem at vt)) /\
+             (type_of_bir_exp ae = SOME (BType_Imm at)) /\
+             (type_of_bir_exp v = SOME (BType_Imm rty)) ==>
+             (if en = BEnd_NoEndian then (vt <> rty) else
+                                  (bir_number_of_mem_splits vt rty = NONE))))
+``,
+
+REPEAT CONJ_TAC >> (
+  SIMP_TAC (std_ss++boolSimps.EQUIV_EXTRACT_ss) [type_of_bir_exp_def]
+) >- (
+  REPEAT GEN_TAC >> REPEAT CASE_TAC >> FULL_SIMP_TAC (std_ss++bir_type_ss) [bir_type_is_Imm_def]
+) >- (
+  REPEAT GEN_TAC >> REPEAT CASE_TAC >> FULL_SIMP_TAC (std_ss++bir_type_ss) [bir_type_is_Imm_def]
+) >- (
+  REPEAT GEN_TAC >> REPEAT CASE_TAC >> (
+    FULL_SIMP_TAC (std_ss++bir_type_ss) [bir_type_is_Imm_def] >>
+    METIS_TAC[]
+  )
+) >- (
+  REPEAT GEN_TAC >> REPEAT CASE_TAC >> (
+    FULL_SIMP_TAC (std_ss++bir_type_ss) [bir_type_is_Imm_def] >>
+    METIS_TAC[]
+  )
+) >- (
+  REPEAT GEN_TAC >> REPEAT CASE_TAC >> (
+    FULL_SIMP_TAC (std_ss) []
+  )
+) >- (
+  REPEAT GEN_TAC >> REPEAT CASE_TAC >> METIS_TAC[]
+) >- (
+  REPEAT GEN_TAC >> REPEAT CASE_TAC >> METIS_TAC[]
+));
+
+
+
+val bir_is_well_typed_exp_def = Define `bir_is_well_typed_exp e <=>  (type_of_bir_exp e <> NONE)`
+
+
+(* ------------------------------------------------------------------------- *)
+(*  Looking at  variables used somewhere in an expression                    *)
+(* ------------------------------------------------------------------------- *)
+
+val bir_vars_of_exp_def = Define `
+  (bir_vars_of_exp (BExp_Const _) = {}) /\
+  (bir_vars_of_exp (BExp_Den v) = {v}) /\
+  (bir_vars_of_exp (BExp_Cast _ e _) = bir_vars_of_exp e) /\
+  (bir_vars_of_exp (BExp_UnaryExp _ e) = bir_vars_of_exp e) /\
+  (bir_vars_of_exp (BExp_BinExp _ e1 e2) = (bir_vars_of_exp e1 UNION bir_vars_of_exp e2)) /\
+  (bir_vars_of_exp (BExp_BinPred _ e1 e2) = (bir_vars_of_exp e1 UNION bir_vars_of_exp e2)) /\
+  (bir_vars_of_exp (BExp_IfThenElse ec e1 e2) = (bir_vars_of_exp ec UNION bir_vars_of_exp e1 UNION bir_vars_of_exp e2)) /\
+  (bir_vars_of_exp (BExp_Load me ae _ _) = (bir_vars_of_exp me UNION bir_vars_of_exp ae)) /\
+  (bir_vars_of_exp (BExp_Store me ae _ ve) = (bir_vars_of_exp me UNION bir_vars_of_exp ae UNION bir_vars_of_exp ve))`
+
+
+val type_of_bir_exp_THM_with_init_vars = store_thm ("type_of_bir_exp_THM_with_init_vars",
+  ``!env. (bir_is_well_typed_env env) ==>
+          (!e ty. (type_of_bir_exp e = SOME ty) ==>
+                  (bir_env_vars_are_initialised env (bir_vars_of_exp e)) ==>
+                  (type_of_bir_val (bir_eval_exp e env) = SOME ty))``,
+
+GEN_TAC >> STRIP_TAC >> Induct >> (
+  SIMP_TAC (std_ss++bir_val_ss) [bir_eval_exp_def, BoolType_def,
+    type_of_bir_exp_EQ_SOME_REWRS, bir_vars_of_exp_def,
+    bir_env_vars_are_initialised_UNION, bir_env_vars_are_initialised_INSERT,
+    bir_env_vars_are_initialised_EMPTY, PULL_EXISTS, PULL_FORALL, bir_type_is_Imm_def] >>
+  REPEAT STRIP_TAC >>
+  FULL_SIMP_TAC (std_ss++bir_val_ss) [type_of_bir_val_EQ_ELIMS, bir_type_is_Imm_def]
+) >- (
+  rename1 `bir_env_read v env` >>
+  Cases_on `v` >>
+  FULL_SIMP_TAC std_ss [bir_env_read_def, bir_env_var_is_initialised_def, bir_var_name_def,
+    bir_var_type_def, pairTheory.pair_case_thm] >>
+  METIS_TAC[bir_is_well_typed_env_lookup]
+) >- (
+  SIMP_TAC (std_ss++bir_val_ss) [bir_eval_cast_REWRS, type_of_bir_gencast]
+) >- (
+  ASM_SIMP_TAC (std_ss++bir_val_ss) [bir_eval_unary_exp_REWRS, type_of_bir_unary_exp]
+) >- (
+  ASM_SIMP_TAC (std_ss++bir_val_ss) [bir_eval_bin_exp_REWRS, type_of_bir_bin_exp]
+) >- (
+  ASM_SIMP_TAC (std_ss++bir_val_ss) [bir_eval_bin_pred_REWRS, type_of_bir_val_def,
+    type_of_bool2b, BoolType_def]
+) >- (
+  ASM_SIMP_TAC (std_ss++bir_val_ss) [bir_eval_ifthenelse_REWRS] >>
+  METIS_TAC[]
+) >- (
+  ASM_SIMP_TAC (std_ss++bir_val_ss) [bir_eval_load_BASIC_REWR] >>
+  rename1 `bir_load_from_mem vt ity mmap en (b2n i)` >>
+  Cases_on `bir_load_from_mem vt ity mmap en (b2n i)` >- (
+    POP_ASSUM MP_TAC >>
+    ASM_SIMP_TAC (std_ss++bir_val_ss) [bir_load_from_mem_EQ_NONE] >>
+    Cases_on `en = BEnd_NoEndian` >> (
+       FULL_SIMP_TAC (std_ss++boolSimps.CONJ_ss) [bir_number_of_mem_splits_ID]
+    )
+  ) >>
+  ASM_SIMP_TAC (std_ss++bir_val_ss) [] >>
+  METIS_TAC [type_of_bir_load_from_mem]
+) >- (
+  ASM_SIMP_TAC (std_ss++bir_val_ss) [bir_eval_store_BASIC_REWR] >>
+  rename1 `bir_store_in_mem vt ity mmap en (b2n i)` >>
+  Cases_on `bir_store_in_mem vt ity mmap en (b2n i)` >- (
+    POP_ASSUM MP_TAC >>
+    ASM_SIMP_TAC (std_ss++bir_val_ss) [bir_store_in_mem_EQ_NONE] >>
+    Cases_on `en = BEnd_NoEndian` >> (
+       FULL_SIMP_TAC (std_ss++boolSimps.CONJ_ss) [bir_number_of_mem_splits_ID]
+    )
+  ) >>
+  ASM_SIMP_TAC (std_ss++bir_val_ss) []
+));
+
+
+
+(* ------------------------------------------------------------------------- *)
+(*  Programs                                                                 *)
+(* ------------------------------------------------------------------------- *)
+
+val bir_is_well_typed_stmt_def = Define `
+  (bir_is_well_typed_stmt (BStmt_Declare _) = T) /\
+  (bir_is_well_typed_stmt (BStmt_Assign v e) = (type_of_bir_exp e = SOME (bir_var_type v))) /\
+  (bir_is_well_typed_stmt (BStmt_Jmp _) = T) /\
+  (bir_is_well_typed_stmt (BStmt_CJmp c _ _) = (type_of_bir_exp c = SOME BoolType)) /\
+  (bir_is_well_typed_stmt (BStmt_Halt e) = (type_of_bir_exp e <> NONE)) /\
+  (bir_is_well_typed_stmt (BStmt_Assert e) = (type_of_bir_exp e = SOME BoolType)) /\
+  (bir_is_well_typed_stmt (BStmt_Assume e) = (type_of_bir_exp e = SOME BoolType))`
+
+
+val bir_is_well_typed_program_def = Define `bir_is_well_typed_program (BirProgram p) <=>
+  (EVERY (\bl. EVERY bir_is_well_typed_stmt bl.bb_statements) p)`;
+
+
+val bir_get_current_statement_well_typed = store_thm ("bir_get_current_statement_well_typed",
+  ``!p pc stmt. (bir_is_well_typed_program p /\
+                (bir_get_current_statement p pc = SOME stmt)) ==>
+                bir_is_well_typed_stmt stmt``,
+
+Cases >> rename1 `BirProgram p` >>
+SIMP_TAC std_ss [bir_is_well_typed_program_def, bir_get_current_statement_def] >>
+REPEAT GEN_TAC >>
+Cases_on `(bir_get_program_block_info_by_label (BirProgram p) pc.bpc_label)` >- (
+  ASM_SIMP_TAC std_ss []
+) >>
+rename1 `_ = SOME xy` >> Cases_on `xy` >>
+rename1 `_ = SOME (i, bl)` >>
+ASM_SIMP_TAC std_ss [] >>
+REPEAT STRIP_TAC >>
+`MEM stmt bl.bb_statements` by METIS_TAC[listTheory.MEM_EL] >>
+`MEM bl p` by METIS_TAC [bir_get_program_block_info_by_label_THM, listTheory.MEM_EL] >>
+FULL_SIMP_TAC std_ss [listTheory.EVERY_MEM] >>
+METIS_TAC[]);
+
+
+val _ = export_theory();
